Update to using wordsTheory.

examples/Crypto/Serpent/Bitslice/Serpent_BitsliceScript.sml
@@ -5,329 +5,276 @@
  http://www.cl.cam.ac.uk/~rja14/serpent.html
 *)
 
-
-open HolKernel Parse boolLib bossLib 
-     listTheory rich_listTheory bitsTheory
-     word32Theory metisLib pairTheory arithmeticTheory
+open HolKernel Parse boolLib bossLib listTheory rich_listTheory bitTheory
+     wordsTheory wordsLib pairTheory arithmeticTheory
      Serpent_Bitslice_UtilityTheory Serpent_Bitslice_SBoxTheory;
 
 val _ = new_theory "Serpent_Bitslice";
 
-val WORD_BITWISE_EQ_PROVE_TAC
-    = SIMP_TAC std_ss [word32Theory.ONE_COMP_EVAL, word32Theory.AND_EVAL,
-                      word32Theory.OR_EVAL, word32Theory.EOR_EVAL] THEN
-     SIMP_TAC std_ss [word32Theory.n2w_11,GSYM word32Theory.EQUIV_def] THEN
-     RW_TAC bool_ss [word32Theory.EOR_def, word32Theory.AND_def, word32Theory.OR_def,
-                     word32Theory.ONE_COMP_BITWISE_THM, GSYM word32Theory.BITWISE_THM2,
-		     BITWISE_THM] THEN
-     tautLib.TAUT_TAC;
-			  
 (*****************TRANSFORMATION*******************************)
 
-val transform_def=Define 
-`transform (x0:word32, x1:word32, x2:word32, x3:word32)=
-	
-	let  y0 =  x0 #>> (32-13)
-	in
-	let  y2 =  x2 #>> (32-3)
-	in
-	let  y1 = ( x1 # y0) # y2
-	
-	in 
-	let  y3 = ( x3 # y2) # ( y0 << 3)
-	in
-	let  y11 =  y1 #>> (32-1)
-	in
-	let  y31 =  y3 #>> (32-7)
-	in
-	let  y01 = ( y0 # y11) # y31
-	in
-	let  y21 = ( y2 # y31) # ( y11 << 7)
-	in 
-	let  y02 = y01 #>> (32-5)
-	in
-	let  y22 = y21 #>>(32-22)
-	in (y02,y11,y22,y31)`;
+val transform_def = Define`
+ transform (x0:word32, x1:word32, x2:word32, x3:word32)=
+   (let y0 = x0 #>> (32 - 13) in
+    let y2 = x2 #>> (32 - 3) in
+    let y1 = (x1 ?? y0) ?? y2 in
+    let y3 = (x3 ?? y2) ?? y0 << 3 in
+    let y11 = y1 #>> (32 - 1) in
+    let y31 = y3 #>> (32 - 7) in
+    let y01 = (y0 ?? y11) ?? y31 in
+    let y21 = (y2 ?? y31) ?? y11 << 7 in
+    let y02 = y01 #>> (32 - 5) in
+    let y22 = y21 #>> (32 - 22) in
+      (y02,y11,y22,y31))`;
 
-val inv_transform_def=Define
-`inv_transform (x0:word32, x1:word32, x2:word32, x3:word32)=
-	let y2 =  x2 #>> 22
-	in 
-	let y0 =  x0 #>> 5
-	in 
-	let y21 = ( y2 # x3) # ( x1 << 7)
-	in 
-	let y01 = ( y0 # x1) # x3
-	in 
-	let y3 = x3 #>> 7
-	in 
-	let y1 =  x1 #>> 1
-	in 
-	let y31 = (y3 # y21) # (y01 << 3)
-	in 
-	let y11 = (y1 # y01) # y21
-	in 
-	let y22 = y21 #>>3
-	in 
-	let y02 = y01 #>> 13
-	in (y02,y11,y22,y31)`;
-				  
-
-val transform_THM=Q.store_thm (
+val inv_transform_def = Define`
+  inv_transform (x0:word32, x1:word32, x2:word32, x3:word32)=
+   (let y2 = x2 #>> 22 in
+    let y0 = x0 #>> 5 in
+    let y21 = (y2 ?? x3) ?? x1 << 7 in
+    let y01 = (y0 ?? x1) ?? x3 in
+    let y3 = x3 #>> 7 in
+    let y1 = x1 #>> 1 in
+    let y31 = (y3 ?? y21) ?? y01 << 3 in
+    let y11 = (y1 ?? y01) ?? y21 in
+    let y22 = y21 #>> 3 in
+    let y02 = y01 #>> 13 in
+      (y02,y11,y22,y31))`;
+                
+val transform_THM = Q.store_thm (
 "transform_THM",
-`!v. 
-	inv_transform (transform v) = v`,
-
-SIMP_TAC std_ss [FORALL_PROD,transform_def,inv_transform_def,
-                 LET_THM,word32Theory.ROR_ADD,ror_32_lem,
-		 WORD_EOR_ID2,WORD_EOR_REDUCTION]);
-
+`!v. inv_transform (transform v) = v`,
+ SIMP_TAC std_ss [FORALL_PROD,transform_def,inv_transform_def,LET_THM] THEN
+ SRW_TAC [] []);
 
 (********************************APPLYING KEYING**************************)
-val keying_def=Define
-`keying (x0:word32, x1:word32, x2:word32, x3:word32) 
+val keying_def = Define
+`keying (x0:word32, x1:word32, x2:word32, x3:word32)
         (subkey0:word32, subkey1:word32, subkey2:word32, subkey3:word32)
- = (x0 # subkey0, x1 # subkey1, x2 # subkey2,x3 # subkey3)`;
-	
-	 
-val keying_THM= Q.store_thm (
+ = (x0 ?? subkey0, x1 ?? subkey1, x2 ?? subkey2,x3 ?? subkey3)`;
+   
+val keying_THM = Q.store_thm (
 "keying_THM",
-`!d sk. 
-	keying (keying d sk) sk = d`,
-	
-SIMP_TAC std_ss [FORALL_PROD,word32Theory.FORALL_WORD,keying_def] THEN  
-RW_TAC std_ss [] THENL [
-	WORD_BITWISE_EQ_PROVE_TAC,
-	WORD_BITWISE_EQ_PROVE_TAC,
-	WORD_BITWISE_EQ_PROVE_TAC,
-	WORD_BITWISE_EQ_PROVE_TAC]);
-	 
+`!d sk.
+    keying (keying d sk) sk = d`,
+  SIMP_TAC std_ss [FORALL_PROD,keying_def] THEN SRW_TAC [] []);
+
 (**************************BLOCK ENCRYPTION******************************)
-val f_def= Define
-	`f a (op,sk) = op a sk`;
+val f_def = Define `f a (op,sk) = op a sk`;
+
+val encryptRnd00_def = Define
+    `encryptRnd00 a b = transform (RND00 (keying a b))`;
+val encryptRnd01_def = Define
+    `encryptRnd01 a b = transform (RND01 (keying a b))`;
+val encryptRnd02_def = Define
+    `encryptRnd02 a b = transform (RND02 (keying a b))`;
+val encryptRnd03_def = Define
+    `encryptRnd03 a b = transform (RND03 (keying a b))`;
+val encryptRnd04_def = Define
+    `encryptRnd04 a b = transform (RND04 (keying a b))`;
+val encryptRnd05_def = Define
+    `encryptRnd05 a b = transform (RND05 (keying a b))`;
+val encryptRnd06_def = Define
+    `encryptRnd06 a b = transform (RND06 (keying a b))`;
+val encryptRnd07_def = Define
+    `encryptRnd07 a b = transform (RND07 (keying a b))`;
+val encryptRnd08_def = Define
+    `encryptRnd08 a b = transform (RND08 (keying a b))`;
+val encryptRnd09_def = Define
+    `encryptRnd09 a b = transform (RND09 (keying a b))`;
+val encryptRnd10_def = Define
+    `encryptRnd10 a b = transform (RND10 (keying a b))`;
+val encryptRnd11_def = Define
+    `encryptRnd11 a b = transform (RND11 (keying a b))`;
+val encryptRnd12_def = Define
+    `encryptRnd12 a b = transform (RND12 (keying a b))`;
+val encryptRnd13_def = Define
+    `encryptRnd13 a b = transform (RND13 (keying a b))`;
+val encryptRnd14_def = Define
+    `encryptRnd14 a b = transform (RND14 (keying a b))`;
+val encryptRnd15_def = Define
+    `encryptRnd15 a b = transform (RND15 (keying a b))`;
+val encryptRnd16_def = Define
+    `encryptRnd16 a b = transform (RND16 (keying a b))`;
+val encryptRnd17_def = Define
+    `encryptRnd17 a b = transform (RND17 (keying a b))`;
+val encryptRnd18_def = Define
+    `encryptRnd18 a b = transform (RND18 (keying a b))`;
+val encryptRnd19_def = Define
+    `encryptRnd19 a b = transform (RND19 (keying a b))`;
+val encryptRnd20_def = Define
+    `encryptRnd20 a b = transform (RND20 (keying a b))`;
+val encryptRnd21_def = Define
+    `encryptRnd21 a b = transform (RND21 (keying a b))`;
+val encryptRnd22_def = Define
+    `encryptRnd22 a b = transform (RND22 (keying a b))`;
+val encryptRnd23_def = Define
+    `encryptRnd23 a b = transform (RND23 (keying a b))`;
+val encryptRnd24_def = Define
+    `encryptRnd24 a b = transform (RND24 (keying a b))`;
+val encryptRnd25_def = Define
+    `encryptRnd25 a b = transform (RND25 (keying a b))`;
+val encryptRnd26_def = Define
+    `encryptRnd26 a b = transform (RND26 (keying a b))`;
+val encryptRnd27_def = Define
+    `encryptRnd27 a b = transform (RND27 (keying a b))`;
+val encryptRnd28_def = Define
+    `encryptRnd28 a b = transform (RND28 (keying a b))`;
+val encryptRnd29_def = Define
+    `encryptRnd29 a b = transform (RND29 (keying a b))`;
+val encryptRnd30_def = Define
+    `encryptRnd30 a b = transform (RND30 (keying a b))`;
+val encryptRnd31_1_def = Define
+    `encryptRnd31_1 a b31 = RND31 (keying a b31)`;
+val encryptRnd31_2_def = Define
+    `encryptRnd31_2 a b32 = keying a b32`;
+
+val decryptRnd00_1_def = Define
+    `decryptRnd00_1 a b32 = keying a b32`;
+val decryptRnd00_2_def = Define
+    `decryptRnd00_2 a b31 = keying (InvRND31 a) b31`;
+val decryptRnd01_def = Define
+    `decryptRnd01 a b = keying (InvRND30 (inv_transform a)) b`;
+val decryptRnd02_def = Define
+    `decryptRnd02 a b = keying (InvRND29 (inv_transform a)) b`;
+val decryptRnd03_def = Define
+    `decryptRnd03 a b = keying (InvRND28 (inv_transform a)) b`;
+val decryptRnd04_def = Define
+    `decryptRnd04 a b = keying (InvRND27 (inv_transform a)) b`;
+val decryptRnd05_def = Define
+    `decryptRnd05 a b = keying (InvRND26 (inv_transform a)) b`;
+val decryptRnd06_def = Define
+    `decryptRnd06 a b = keying (InvRND25 (inv_transform a)) b`;
+val decryptRnd07_def = Define
+    `decryptRnd07 a b = keying (InvRND24 (inv_transform a)) b`;
+val decryptRnd08_def = Define
+    `decryptRnd08 a b = keying (InvRND23 (inv_transform a)) b`;
+val decryptRnd09_def = Define
+    `decryptRnd09 a b = keying (InvRND22 (inv_transform a)) b`;
+val decryptRnd10_def = Define
+    `decryptRnd10 a b = keying (InvRND21 (inv_transform a)) b`;
+val decryptRnd11_def = Define
+    `decryptRnd11 a b = keying (InvRND20 (inv_transform a)) b`;
+val decryptRnd12_def = Define
+    `decryptRnd12 a b = keying (InvRND19 (inv_transform a)) b`;
+val decryptRnd13_def = Define
+    `decryptRnd13 a b = keying (InvRND18 (inv_transform a)) b`;
+val decryptRnd14_def = Define
+    `decryptRnd14 a b = keying (InvRND17 (inv_transform a)) b`;
+val decryptRnd15_def = Define
+    `decryptRnd15 a b = keying (InvRND16 (inv_transform a)) b`;
+val decryptRnd16_def = Define
+    `decryptRnd16 a b = keying (InvRND15 (inv_transform a)) b`;
+val decryptRnd17_def = Define
+    `decryptRnd17 a b = keying (InvRND14 (inv_transform a)) b`;
+val decryptRnd18_def = Define
+    `decryptRnd18 a b = keying (InvRND13 (inv_transform a)) b`;
+val decryptRnd19_def = Define
+    `decryptRnd19 a b = keying (InvRND12 (inv_transform a)) b`;
+val decryptRnd20_def = Define
+    `decryptRnd20 a b = keying (InvRND11 (inv_transform a)) b`;
+val decryptRnd21_def = Define
+    `decryptRnd21 a b = keying (InvRND10 (inv_transform a)) b`;
+val decryptRnd22_def = Define
+    `decryptRnd22 a b = keying (InvRND09 (inv_transform a)) b`;
+val decryptRnd23_def = Define
+    `decryptRnd23 a b = keying (InvRND08 (inv_transform a)) b`;
+val decryptRnd24_def = Define
+    `decryptRnd24 a b = keying (InvRND07 (inv_transform a)) b`;
+val decryptRnd25_def = Define
+    `decryptRnd25 a b = keying (InvRND06 (inv_transform a)) b`;
+val decryptRnd26_def = Define
+    `decryptRnd26 a b = keying (InvRND05 (inv_transform a)) b`;
+val decryptRnd27_def = Define
+    `decryptRnd27 a b = keying (InvRND04 (inv_transform a)) b`;
+val decryptRnd28_def = Define
+    `decryptRnd28 a b = keying (InvRND03 (inv_transform a)) b`;
+val decryptRnd29_def = Define
+    `decryptRnd29 a b = keying (InvRND02 (inv_transform a)) b`;
+val decryptRnd30_def = Define
+    `decryptRnd30 a b = keying (InvRND01 (inv_transform a)) b`;
+val decryptRnd31_def = Define
+    `decryptRnd31 a b = keying (InvRND00 (inv_transform a)) b`;
+
+val encryptSchedule_def = Define
+`encryptSchedule = encryptRnd00::encryptRnd01::encryptRnd02::encryptRnd03::
+    encryptRnd04::encryptRnd05::encryptRnd06::encryptRnd07::
+    encryptRnd08::encryptRnd09::encryptRnd10::encryptRnd11::
+    encryptRnd12::encryptRnd13::encryptRnd14::encryptRnd15::
+    encryptRnd16::encryptRnd17::encryptRnd18::encryptRnd19::
+    encryptRnd20::encryptRnd21::encryptRnd22::encryptRnd23::
+    encryptRnd24::encryptRnd25::encryptRnd26::encryptRnd27::
+    encryptRnd28::encryptRnd29::encryptRnd30::encryptRnd31_1::encryptRnd31_2::[]`;
 
 
-val encryptRnd00_def = Define 
-	`encryptRnd00 a b =transform (RND00 (keying a b))`;
-val encryptRnd01_def = Define 
-	`encryptRnd01 a b =transform (RND01 (keying a b))`;
-val encryptRnd02_def = Define 
-	`encryptRnd02 a b =transform (RND02 (keying a b))`;
-val encryptRnd03_def = Define 
-	`encryptRnd03 a b =transform (RND03 (keying a b))`;
-val encryptRnd04_def = Define 
-	`encryptRnd04 a b =transform (RND04 (keying a b))`;
-val encryptRnd05_def = Define 
-	`encryptRnd05 a b =transform (RND05 (keying a b))`;
-val encryptRnd06_def = Define 
-	`encryptRnd06 a b =transform (RND06 (keying a b))`;
-val encryptRnd07_def = Define 
-	`encryptRnd07 a b =transform (RND07 (keying a b))`;
-val encryptRnd08_def = Define 
-	`encryptRnd08 a b =transform (RND08 (keying a b))`;
-val encryptRnd09_def = Define 
-	`encryptRnd09 a b =transform (RND09 (keying a b))`;
-val encryptRnd10_def = Define 
-	`encryptRnd10 a b =transform (RND10 (keying a b))`;
-val encryptRnd11_def = Define 
-	`encryptRnd11 a b =transform (RND11 (keying a b))`;
-val encryptRnd12_def = Define 
-	`encryptRnd12 a b =transform (RND12 (keying a b))`;
-val encryptRnd13_def = Define 
-	`encryptRnd13 a b =transform (RND13 (keying a b))`;
-val encryptRnd14_def = Define 
-	`encryptRnd14 a b =transform (RND14 (keying a b))`;
-val encryptRnd15_def = Define 
-	`encryptRnd15 a b =transform (RND15 (keying a b))`;
-val encryptRnd16_def = Define 
-	`encryptRnd16 a b =transform (RND16 (keying a b))`;
-val encryptRnd17_def = Define 
-	`encryptRnd17 a b =transform (RND17 (keying a b))`;
-val encryptRnd18_def = Define 
-	`encryptRnd18 a b =transform (RND18 (keying a b))`;
-val encryptRnd19_def = Define 
-	`encryptRnd19 a b =transform (RND19 (keying a b))`;
-val encryptRnd20_def = Define 
-	`encryptRnd20 a b =transform (RND20 (keying a b))`;
-val encryptRnd21_def = Define 
-	`encryptRnd21 a b =transform (RND21 (keying a b))`;
-val encryptRnd22_def = Define 
-	`encryptRnd22 a b =transform (RND22 (keying a b))`;
-val encryptRnd23_def = Define 
-	`encryptRnd23 a b =transform (RND23 (keying a b))`;
-val encryptRnd24_def = Define 
-	`encryptRnd24 a b =transform (RND24 (keying a b))`;
-val encryptRnd25_def = Define 
-	`encryptRnd25 a b =transform (RND25 (keying a b))`;
-val encryptRnd26_def = Define 
-	`encryptRnd26 a b =transform (RND26 (keying a b))`;
-val encryptRnd27_def = Define 
-	`encryptRnd27 a b =transform (RND27 (keying a b))`;
-val encryptRnd28_def = Define 
-	`encryptRnd28 a b =transform (RND28 (keying a b))`;
-val encryptRnd29_def = Define 
-	`encryptRnd29 a b =transform (RND29 (keying a b))`;
-val encryptRnd30_def = Define 
-	`encryptRnd30 a b =transform (RND30 (keying a b))`;
-val encryptRnd31_1_def = Define 
-	`encryptRnd31_1 a b31 =RND31 (keying a b31)`;
-val encryptRnd31_2_def = Define 
-	`encryptRnd31_2 a b32 =keying a b32`;
+val decryptSchedule_def = Define
+`decryptSchedule = decryptRnd00_1::decryptRnd00_2::decryptRnd01::
+    decryptRnd02::decryptRnd03::
+    decryptRnd04::decryptRnd05::decryptRnd06::decryptRnd07::
+    decryptRnd08::decryptRnd09::decryptRnd10::decryptRnd11::
+    decryptRnd12::decryptRnd13::decryptRnd14::decryptRnd15::
+    decryptRnd16::decryptRnd17::decryptRnd18::decryptRnd19::
+    decryptRnd20::decryptRnd21::decryptRnd22::decryptRnd23::
+    decryptRnd24::decryptRnd25::decryptRnd26::decryptRnd27::
+    decryptRnd28::decryptRnd29::decryptRnd30::decryptRnd31::[]`;
 
-val decryptRnd00_1_def = Define 
-	`decryptRnd00_1 a b32 = keying a b32`;
-val decryptRnd00_2_def = Define 
-	`decryptRnd00_2 a b31 = keying (InvRND31 a) b31`;
-val decryptRnd01_def = Define 
-	`decryptRnd01 a b = keying (InvRND30 (inv_transform a)) b`;  
-val decryptRnd02_def = Define 
-	`decryptRnd02 a b = keying (InvRND29 (inv_transform a)) b`;  
-val decryptRnd03_def = Define 
-	`decryptRnd03 a b = keying (InvRND28 (inv_transform a)) b`;  
-val decryptRnd04_def = Define 
-	`decryptRnd04 a b = keying (InvRND27 (inv_transform a)) b`;  
-val decryptRnd05_def = Define 
-	`decryptRnd05 a b = keying (InvRND26 (inv_transform a)) b`;  
-val decryptRnd06_def = Define 
-	`decryptRnd06 a b = keying (InvRND25 (inv_transform a)) b`;
-val decryptRnd07_def = Define 
-	`decryptRnd07 a b = keying (InvRND24 (inv_transform a)) b`;  
-val decryptRnd08_def = Define 
-	`decryptRnd08 a b = keying (InvRND23 (inv_transform a)) b`;  
-val decryptRnd09_def = Define 
-	`decryptRnd09 a b = keying (InvRND22 (inv_transform a)) b`;  
-val decryptRnd10_def = Define 
-	`decryptRnd10 a b = keying (InvRND21 (inv_transform a)) b`;  
-val decryptRnd11_def = Define 
-	`decryptRnd11 a b = keying (InvRND20 (inv_transform a)) b`;  
-val decryptRnd12_def = Define 
-	`decryptRnd12 a b = keying (InvRND19 (inv_transform a)) b`;  
-val decryptRnd13_def = Define 
-	`decryptRnd13 a b = keying (InvRND18 (inv_transform a)) b`;  
-val decryptRnd14_def = Define 
-	`decryptRnd14 a b = keying (InvRND17 (inv_transform a)) b`;  
-val decryptRnd15_def = Define 
-	`decryptRnd15 a b = keying (InvRND16 (inv_transform a)) b`;  
-val decryptRnd16_def = Define 
-	`decryptRnd16 a b = keying (InvRND15 (inv_transform a)) b`;
-val decryptRnd17_def = Define 
-	`decryptRnd17 a b = keying (InvRND14 (inv_transform a)) b`;  
-val decryptRnd18_def = Define 
-	`decryptRnd18 a b = keying (InvRND13 (inv_transform a)) b`;  
-val decryptRnd19_def = Define 
-	`decryptRnd19 a b = keying (InvRND12 (inv_transform a)) b`;  
-val decryptRnd20_def = Define 
-	`decryptRnd20 a b = keying (InvRND11 (inv_transform a)) b`;  
-val decryptRnd21_def = Define 
-	`decryptRnd21 a b = keying (InvRND10 (inv_transform a)) b`;
-val decryptRnd22_def = Define 
-	`decryptRnd22 a b = keying (InvRND09 (inv_transform a)) b`;  
-val decryptRnd23_def = Define 
-	`decryptRnd23 a b = keying (InvRND08 (inv_transform a)) b`;  
-val decryptRnd24_def = Define 
-	`decryptRnd24 a b = keying (InvRND07 (inv_transform a)) b`;  
-val decryptRnd25_def = Define 
-	`decryptRnd25 a b = keying (InvRND06 (inv_transform a)) b`;  
-val decryptRnd26_def = Define 
-	`decryptRnd26 a b = keying (InvRND05 (inv_transform a)) b`;
-val decryptRnd27_def = Define 
-	`decryptRnd27 a b = keying (InvRND04 (inv_transform a)) b`;  
-val decryptRnd28_def = Define 
-	`decryptRnd28 a b = keying (InvRND03 (inv_transform a)) b`;  
-val decryptRnd29_def = Define 
-	`decryptRnd29 a b = keying (InvRND02 (inv_transform a)) b`;  
-val decryptRnd30_def = Define 
-	`decryptRnd30 a b = keying (InvRND01 (inv_transform a)) b`;  
-val decryptRnd31_def = Define 
-	`decryptRnd31 a b = keying (InvRND00 (inv_transform a)) b`;  
-
-
-val encryptSchedule_def =Define
-`encryptSchedule=encryptRnd00::encryptRnd01::encryptRnd02::encryptRnd03::
-	encryptRnd04::encryptRnd05::encryptRnd06::encryptRnd07::
-	encryptRnd08::encryptRnd09::encryptRnd10::encryptRnd11::
-	encryptRnd12::encryptRnd13::encryptRnd14::encryptRnd15::
-	encryptRnd16::encryptRnd17::encryptRnd18::encryptRnd19::
-	encryptRnd20::encryptRnd21::encryptRnd22::encryptRnd23::
-	encryptRnd24::encryptRnd25::encryptRnd26::encryptRnd27::
-	encryptRnd28::encryptRnd29::encryptRnd30::encryptRnd31_1::encryptRnd31_2::[]`;
-
-
-
-val decryptSchedule_def=Define
-`decryptSchedule=decryptRnd00_1::decryptRnd00_2::decryptRnd01::decryptRnd02::decryptRnd03::
-	decryptRnd04::decryptRnd05::decryptRnd06::decryptRnd07::
-	decryptRnd08::decryptRnd09::decryptRnd10::decryptRnd11::
-	decryptRnd12::decryptRnd13::decryptRnd14::decryptRnd15::
-	decryptRnd16::decryptRnd17::decryptRnd18::decryptRnd19::
-	decryptRnd20::decryptRnd21::decryptRnd22::decryptRnd23::
-	decryptRnd24::decryptRnd25::decryptRnd26::decryptRnd27::
-	decryptRnd28::decryptRnd29::decryptRnd30::decryptRnd31::[]`;
-
-
-
-			 
+           
 val serpent_encrypt_def = Define
-	`serpent_encrypt plaintext subkeys=
-	let opKey =ZIP (encryptSchedule, subkeys)
-	in 
-	FOLDL f plaintext opKey`;
-
-
-
+    `serpent_encrypt plaintext subkeys =
+    let opKey = ZIP (encryptSchedule, subkeys)
+    in
+    FOLDL f plaintext opKey`;
 
 val serpent_decrypt_def = Define
-	`serpent_decrypt ciphertext subkeys=
-	let opKey =ZIP (decryptSchedule, REVERSE subkeys)
-	in 
-	FOLDL f ciphertext opKey`;
+    `serpent_decrypt ciphertext subkeys =
+    let opKey = ZIP (decryptSchedule, REVERSE subkeys)
+    in
+    FOLDL f ciphertext opKey`;
 
 (*********************FUNCTIONAL CORRECTNESS********************)
-	 
-
-val serpent_THM=Q.store_thm(
+   
+val serpent_THM = Q.store_thm(
 "serpent_THM",
-`!pt sk. 
-	(LENGTH sk=33)
-	==>
-	(serpent_decrypt (serpent_encrypt pt sk) sk =pt)`,
-
-RW_TAC list_ss [serpent_decrypt_def,serpent_encrypt_def,LET_THM] THEN
-`?v_0 v_1 v_2 v_3 v_4 v_5 v_6 v_7 v_8 v_9 v_10 v_11
-  v_12 v_13 v_14 v_15 v_16 v_17 v_18 v_19 v_20 v_21 v_22 
-  v_23 v_24 v_25 v_26 v_27 v_28 v_29 v_30 v_31 v_32.
- sk=[v_0; v_1; v_2; v_3; v_4; v_5; v_6; v_7; v_8; v_9; v_10; v_11; 
-     v_12; v_13; v_14; v_15; v_16; v_17; v_18; v_19; v_20; v_21; v_22; 
-     v_23; v_24; v_25; v_26; v_27; v_28; v_29; v_30; v_31; v_32]` 
+`!pt sk.
+    (LENGTH sk = 33)
+    ==>
+    (serpent_decrypt (serpent_encrypt pt sk) sk = pt)`,
+ RW_TAC list_ss [serpent_decrypt_def,serpent_encrypt_def,LET_THM] THEN
+  `?v_0 v_1 v_2 v_3 v_4 v_5 v_6 v_7 v_8 v_9 v_10 v_11
+    v_12 v_13 v_14 v_15 v_16 v_17 v_18 v_19 v_20 v_21 v_22
+    v_23 v_24 v_25 v_26 v_27 v_28 v_29 v_30 v_31 v_32.
+   sk =[v_0; v_1; v_2; v_3; v_4; v_5; v_6; v_7; v_8; v_9; v_10; v_11;
+        v_12; v_13; v_14; v_15; v_16; v_17; v_18; v_19; v_20; v_21; v_22;
+        v_23; v_24; v_25; v_26; v_27; v_28; v_29; v_30; v_31; v_32]`
      by METIS_TAC [listInstEq33] THEN
-RW_TAC list_ss [encryptSchedule_def, decryptSchedule_def,f_def,
-	encryptRnd00_def,encryptRnd01_def,encryptRnd02_def,encryptRnd03_def,
-	encryptRnd04_def,encryptRnd05_def,encryptRnd06_def,encryptRnd07_def,
-	encryptRnd08_def,encryptRnd09_def,encryptRnd10_def,encryptRnd11_def,
-	encryptRnd12_def,encryptRnd13_def,encryptRnd14_def,encryptRnd15_def,
-	encryptRnd16_def,encryptRnd17_def,encryptRnd18_def,encryptRnd19_def,
-	encryptRnd20_def,encryptRnd21_def,encryptRnd22_def,encryptRnd23_def,
-	encryptRnd24_def,encryptRnd25_def,encryptRnd26_def,encryptRnd27_def,
-	encryptRnd28_def,encryptRnd29_def,encryptRnd30_def,encryptRnd31_1_def,
-	encryptRnd31_2_def,
-	decryptRnd00_1_def,decryptRnd00_2_def,decryptRnd01_def,decryptRnd02_def,
-	decryptRnd03_def,decryptRnd04_def,decryptRnd05_def,decryptRnd06_def,
-	decryptRnd07_def,decryptRnd08_def,decryptRnd09_def,decryptRnd10_def,
-	decryptRnd11_def,decryptRnd12_def,decryptRnd13_def,decryptRnd14_def,
-	decryptRnd15_def,decryptRnd16_def,decryptRnd17_def,decryptRnd18_def,
-	decryptRnd19_def,decryptRnd20_def,decryptRnd21_def,decryptRnd22_def,
-	decryptRnd23_def,decryptRnd24_def,decryptRnd25_def,decryptRnd26_def,
-	decryptRnd27_def,decryptRnd28_def,decryptRnd29_def,decryptRnd30_def,
-	decryptRnd31_def,
-	
-	RND00_THM,RND01_THM,RND02_THM,RND03_THM,
-	RND04_THM,RND05_THM,RND06_THM,RND07_THM,
-	RND08_THM,RND09_THM,RND10_THM,RND11_THM,
-	RND12_THM,RND13_THM,RND14_THM,RND15_THM,
-	RND16_THM,RND17_THM,RND18_THM,RND19_THM,
-	RND20_THM,RND21_THM,RND22_THM,RND23_THM,
-	RND24_THM,RND25_THM,RND26_THM,RND27_THM,
-	RND28_THM,RND29_THM,RND30_THM,RND31_THM,
-	keying_THM,transform_THM]);  
-	
+ RW_TAC list_ss [encryptSchedule_def, decryptSchedule_def,f_def,
+    encryptRnd00_def,encryptRnd01_def,encryptRnd02_def,encryptRnd03_def,
+    encryptRnd04_def,encryptRnd05_def,encryptRnd06_def,encryptRnd07_def,
+    encryptRnd08_def,encryptRnd09_def,encryptRnd10_def,encryptRnd11_def,
+    encryptRnd12_def,encryptRnd13_def,encryptRnd14_def,encryptRnd15_def,
+    encryptRnd16_def,encryptRnd17_def,encryptRnd18_def,encryptRnd19_def,
+    encryptRnd20_def,encryptRnd21_def,encryptRnd22_def,encryptRnd23_def,
+    encryptRnd24_def,encryptRnd25_def,encryptRnd26_def,encryptRnd27_def,
+    encryptRnd28_def,encryptRnd29_def,encryptRnd30_def,encryptRnd31_1_def,
+    encryptRnd31_2_def,
+    decryptRnd00_1_def,decryptRnd00_2_def,decryptRnd01_def,decryptRnd02_def,
+    decryptRnd03_def,decryptRnd04_def,decryptRnd05_def,decryptRnd06_def,
+    decryptRnd07_def,decryptRnd08_def,decryptRnd09_def,decryptRnd10_def,
+    decryptRnd11_def,decryptRnd12_def,decryptRnd13_def,decryptRnd14_def,
+    decryptRnd15_def,decryptRnd16_def,decryptRnd17_def,decryptRnd18_def,
+    decryptRnd19_def,decryptRnd20_def,decryptRnd21_def,decryptRnd22_def,
+    decryptRnd23_def,decryptRnd24_def,decryptRnd25_def,decryptRnd26_def,
+    decryptRnd27_def,decryptRnd28_def,decryptRnd29_def,decryptRnd30_def,
+    decryptRnd31_def,
+  
+    RND00_THM,RND01_THM,RND02_THM,RND03_THM,
+    RND04_THM,RND05_THM,RND06_THM,RND07_THM,
+    RND08_THM,RND09_THM,RND10_THM,RND11_THM,
+    RND12_THM,RND13_THM,RND14_THM,RND15_THM,
+    RND16_THM,RND17_THM,RND18_THM,RND19_THM,
+    RND20_THM,RND21_THM,RND22_THM,RND23_THM,
+    RND24_THM,RND25_THM,RND26_THM,RND27_THM,
+    RND28_THM,RND29_THM,RND30_THM,RND31_THM,
+    keying_THM,transform_THM]);
+  
 val _ = export_theory();
