examples/Crypto/Serpent/Bitslice/Serpent_Bitslice_SBoxScript.sml
@@ -1,1045 +1,463 @@
-open HolKernel Parse boolLib bossLib bitsTheory
-     markerTheory metisLib pairTheory arithmeticTheory 
-     word32Theory word32Lib metisLib
-     Serpent_Bitslice_UtilityTheory ;
+open HolKernel Parse boolLib bossLib bitTheory
+     markerTheory pairTheory arithmeticTheory wordsTheory wordsLib
+     Serpent_Bitslice_UtilityTheory;
 
 val _ = new_theory "Serpent_Bitslice_SBox";
 
-(*RNDxxx is the SBox in xxx round,
-invRNDxxx is the invSBox in xxx round*)
-val RND00_def = Define 
-	`RND00  (a:word32,b:word32,c:word32,d:word32)= 
-	let t01 =  b # c
-	in
-	let t02 =  a   | d 
-	in
-	let t03 =   a  #  b 
-	in
-	let z =   t02  # t01
-	in
-	let t05 =  c   | z
-	in
-	let t06 =  a   # d  
-	in
-	let t07 =  b   |  c 
-	in
-	let t08 =  d   & t05
-	in
-	let t09 =  t03 & t07
-	in 
-	let y =     t09 # t08
-	in
-	let t11 = t09 & y  
-	in
-	let t12 =  c # d 
-	in
-	let t13=  t07 # t11
-	in 
-	let t14= b &  t06
-	in
-	let t15= t06 #  t13
-	in
-	let w = NOT  t15
-	in
-	let t17= w  #  t14
-	in
-	let  x=  t12 # t17
-	in
-	
-	(w,x,y,z)`;
-
-
-
-val InvRND00_def = Define 
-	`InvRND00  (a:word32,b:word32,c:word32,d:word32)=  
-	
-	let t01 =    c # d
-	in 
-	let t02 =   a  |  b 
-	in 
-	let t03 =   b | c 
-	in
-	let t04 =   c & t01
-	in 
-	let t05 =   t02 # t01
-	in
-	let t06 =   a | t04
-	in
-	let y   =   NOT  t05
-	in
-	let t08 =   b # d
-	in
-	let t09 =  t03  & t08
-	in 
-	let t10 =  d | y  
-	in 
-	let x   =    t09 # t06
-	in 
-	let t12 =    a  | t05
-	in 
-	let t13 =    x # t12
-	in 
-	let t14 =    t03 # t10
-	in 
-	let t15 =    a # c  
-	in 
-	let z   =    t14 # t13
-	in 
-	let t17 =   t05 & t13
-	in 
-	let t18 =  t14 | t17
-	in 
-	let w   = t15 # t18
-	in
-	
-	(w,x,y,z)`;
-
-
-val RND01_def= Define
-	`RND01  (a:word32,b:word32,c:word32,d:word32)=  
-	
-	let t01 =  a | d  
-	in
-	let t02 =  c # d  
-	in 
-	let t03 =  NOT b  
-	in 
-	let t04 =  a # c 
-	in 
-	let t05 =  a | t03
-	in 
-	let t06 = d & t04
-	in
-	let t07 = t01 & t02
-	in 
-	let t08 =  b | t06
-	in
-	let y   =  t02 # t05
-	in
-	let t10 = t07 # t08
-	in 
-	let t11 = t01 # t10
-	in 
-	let t12 =  y # t11
-	in 
-	let t13 =  b & d  
-	in 
-	let z   =  NOT  t10
-	in 
-	let x   = t13 # t12
-	in 
-	let t16 = t10 | x  
-	in 
-	let t17 =  t05 & t16
-	in 
-	let w   =  c # t17
-	in (w,x,y,z)`;
-
-val InvRND01_def = Define
-	`InvRND01  (a:word32,b:word32,c:word32,d:word32)=  
-	let t01 =     a # b  
-	in 
-	let t02 =   b  | d  
-	in 
-	let t03 =   a & c  
-	in 
-	let t04 =   c # t02
-	in 
-	let t05 =   a  | t04
-	in 
-	let t06 =   t01 & t05
-	in 
-	let t07 =  d  | t03
-	in 
-	let t08 =  b  # t06
-	in 
-	let t09 =  t07 # t06
-	in 
-	let t10 =  t04  | t03
-	in 
-	let t11 =  d  &  t08
-	in 
-	let y   =  NOT t09
-	in 
-	let x   =  t10 # t11
-	in 
-	let t14 =   a | y  
-	in 
-	let t15 =   t06 # x  
-	in 
-	let z   =   t01 # t04
-	in 
-	let t17 =   c  # t15
-	in 
-	let w   =  t14  # t17
-	in (w,x,y,z)`;
-
-
-val  RND02_def = Define 
-	`RND02  (a:word32,b:word32,c:word32,d:word32)=  
-	
-	let t01 =   a | c  
-	in 
-	let t02 =    a # b  
-	in 
-	let t03 =   d # t01
-	in 
-	let w   =   t02  # t03
-	in 
-	let t05 =   c # w  
-	in 
-	let t06 =   b # t05
-	in 
-	let t07 =   b | t05
-	in 
-	let t08 =   t01 & t06
-	in 
-	let t09 =   t03 # t07
-	in 
-	let t10 =   t02 | t09
-	in 
-	let x   =   t10 # t08
-	in 
-	let t12 =   a | d  
-	in 
-	let t13 =  t09  # x  
-	in 
-	let t14 =  b # t13
-	in 
-	let z   =  NOT t09
-	in 
-	let y   =  t12 # t14
-	in (w,x,y,z)`;
-
-
-val InvRND02_def = Define
-	`InvRND02  (a:word32,b:word32,c:word32,d:word32)=  
-	
-	let t01 =  a # d  
-	in 
-	let t02 =  c # d  
-	in 
-	let t03 =  a & c  
-	in 
-	let t04 =  b | t02
-	in 
-	let w   =  t01 # t04
-	in 
-	let t06 = a  |  c  
-	in 
-	let t07 = d | w  
-	in 
-	let t08 =     NOT d  
-	in 
-	let t09 =   b  & t06
-	in 
-	let t10 =  t08 | t03
-	in 
-	let t11 =   b & t07
-	in 
-	let t12 =   t06 & t02
-	in 
-	let z   =   t09 # t10
-	in 
-	let x   =   t12 # t11
-	in 
-	let t15 =   c & z  
-	in 
-	let t16 =   w # x  
-	in 
-	let t17 =   t10 # t15
-	in 
-	let y   =   t16 # t17
-	in (w,x,y,z)`;
-
-
-val  RND03_def = Define 
-	`RND03  (a:word32,b:word32,c:word32,d:word32)=  
-	let  t01 =  a   #  c  
-	in 
-	let   t02 = a | d  
-	in 
-	let   t03 = a & d  
-	in 
-	let   t04 =t01  & t02
-	in 
-	let t05 =   b | t03
-	in 
-	let   t06 = a & b  
-	in 
-	let   t07 = d # t04
-	in 
-	let   t08 = c | t06
-	in 
-	let   t09 = b #  t07
-	in 
-	let   t10 = d  & t05
-	in 
-	let   t11 = t02 # t10
-	in 
-	let   z   = t08 # t09
-	in 
-	let   t13 = d | z  
-	in 
-	let   t14 = a | t07
-	in 
-	let   t15 = b & t13
-	in 
-	let   y   =t08  # t11
-	in 
-	let   w   = t14 # t15
-	in 
-	let   x   = t05 # t04
-	in (w,x,y,z)`;
-
-val  InvRND03_def = Define
-	`InvRND03  (a:word32,b:word32,c:word32,d:word32)=  
-		
-	let  t01 =   c | d  
-	in 
-	let   t02 =a | d  
-	in 
-	let   t03 = c # t02
-	in 
-	let   t04 = b # t02
-	in 
-	let   t05 = a  # d  
-	in 
-	let   t06 =  t04 & t03
-	in 
-	let   t07 = b & t01
-	in 
-	let   y   = t05 # t06
-	in 
-	let   t09 = a # t03
-	in 
-	let   w   = t07 # t03
-	in 
-	let   t11 = w | t05
-	in 
-	let   t12 = t09 & t11
-	in 
-	let   t13 = a & y  
-	in 
-	let   t14 = t01 # t05
-	in 
-	let   x   =b # t12
-	in 
-	let   t16 = b | t13
-	in 
-	let   z   =t14 # t16
-	in (w,x,y,z)`;
-
-
-
-
-val  RND04_def = Define
-	`RND04  (a:word32,b:word32,c:word32,d:word32)=  
-	let t01 =  a | b  
-	in 
-	let t02 =   b | c  
-	in 
-	let t03 =   a # t02
-	in 
-	let   t04 = b #  d  
-	in 
-	let   t05 = d  | t03
-	in 
-	let   t06 = d  & t01
-	in 
-	let   z   = t03 # t06
-	in 
-	let   t08 = z &  t04
-	in 
-	let   t09 =t04 & t05
-	in 
-	let   t10 = c  # t06
-	in 
-	let   t11 = b & c  
-	in 
-	let   t12 = t04  # t08
-	in 
-	let   t13 = t11 | t03
-	in 
-	let   t14 =t10 # t09
-	in 
-	let   t15 = a & t05
-	in 
-	let   t16 = t11 | t12
-	in 
-	let   y   = t13 # t08
-	in 
-	let   x   = t15 # t16
-	in 
-	let   w   =NOT t14
-	in (w,x,y,z)`;
-
-val  InvRND04_def = Define 
-	`InvRND04  (a:word32,b:word32,c:word32,d:word32)=  
-	let  t01 =  b | d  
-	in 
-	let   t02 =  c | d  
-	in 
-	let   t03 =  a & t01
-	in 
-	let   t04 =  b # t02
-	in 
-	let   t05 =  c # d  
-	in 
-	let   t06 =  NOT t03
-	in 
-	let   t07 =  a & t04
-	in 
-	let   x   =  t05 # t07
-	in 
-	let   t09 =  x | t06
-	in 
-	let   t10 =  a # t07
-	in 
-	let   t11 =  t01 # t09
-	in 
-	let   t12 =  d # t04
-	in 
-	let   t13 =  c | t10
-	in 
-	let   z   =  t03 # t12
-	in 
-	let   t15 =  a # t04
-	in 
-	let   y   =  t11 # t13
-	in 
-	let   w   =  t15 # t09
-	in (w,x,y,z)`;
-
-val  RND05_def = Define
-	`RND05  (a:word32,b:word32,c:word32,d:word32)=  
-	let  t01 =   b #  d  
-	in 
-	let   t02 = b  | d  
-	in 
-	let   t03 =  a & t01
-	in 
-	let   t04 =  c # t02
-	in 
-	let   t05 =   t03 # t04
-	in 
-	let   w   =   NOT  t05
-	in 
-	let   t07 =   a  # t01
-	in 
-	let   t08 =   d | w  
-	in 
-	let   t09 =  b | t05
-	in 
-	let   t10 =   d #t08
-	in 
-	let   t11 =   b | t07
-	in 
-	let   t12 =  t03 | w  
-	in 
-	let   t13 =   t07 | t10
-	in 
-	let   t14 =   t01 # t11
-	in 
-	let   y   =  t09 # t13
-	in 
-	let   x   =  t07 # t08
-	in 
-	let   z   =  t12 # t14
-	in (w,x,y,z)`;
-
-
-val  InvRND05_def = Define
-	`InvRND05  (a:word32,b:word32,c:word32,d:word32)=  
-	let  t01 = a & d  
-	in 
-	let   t02 =   c  #  t01
-	in 
-	let   t03 =   a # d  
-	in 
-	let   t04 =   b  & t02
-	in 
-	let   t05 =   a & c  
-	in 
-	let   w   =   t03 # t04
-	in 
-	let   t07 =  a &  w  
-	in 
-	let   t08 =    t01 # w  
-	in 
-	let   t09 =    b | t05
-	in 
-	let   t10 =    NOT b  
-	in 
-	let   x   =  t08 # t09
-	in 
-	let   t12 =  t10 | t07
-	in 
-	let   t13 =  w | x  
-	in 
-	let   z   =  t02 # t12
-	in 
-	let   t15 =  t02 # t13
-	in 
-	let   t16 =  b # d  
-	in 
-	let   y   = t16 # t15
-	in 
-	(w,x,y,z)`;
-
-val  RND06_def = Define
-	`RND06  (a:word32,b:word32,c:word32,d:word32)=  
-	let  t01 =  a & d  
-	in 
-	let   t02 =  b # c  
-	in 
-	let   t03 =  a  # d  
-	in 
-	let   t04 = t01  # t02
-	in 
-	let   t05 =  b | c  
-	in 
-	let   x   =  NOT t04
-	in 
-	let   t07 =  t03 & t05
-	in 
-	let   t08 =  b & x  
-	in 
-	let   t09 =  a | c  
-	in 
-	let   t10 =  t07  # t08
-	in 
-	let   t11 =  b |  d  
-	in 
-	let   t12 =  c # t11
-	in 
-	let   t13 = t09 # t10
-	in 
-	let   y   =  NOT t13
-	in 
-	let   t15 =  x  &  t03
-	in 
-	let   z   = t12 # t07
-	in 
-	let   t17 =  a # b  
-	in 
-	let   t18 =  y # t15
-	in 
-	let   w   =   t17 # t18
-	in (w,x,y,z)`;
-
-val InvRND06_def= Define 
-	`InvRND06  (a:word32,b:word32,c:word32,d:word32)=  
-	let  t01 =   a # c  
-	in 
-	let   t02 = NOT c  
-	in 
-	let   t03 =  b &  t01
-	in 
-	let   t04 = b  | t02
-	in 
-	let   t05 =  d | t03
-	in 
-	let   t06 =  b # d  
-	in 
-	let   t07 =  a & t04
-	in 
-	let   t08 =  a | t02
-	in 
-	let   t09 =  t07 # t05
-	in 
-	let   x   =  t06  # t08
-	in 
-	let   w   =  NOT t09
-	in 
-	let   t12 =  b & w  
-	in 
-	let   t13 =  t01 & t05
-	in 
-	let   t14 = t01 # t12
-	in 
-	let   t15 =   t07 # t13
-	in 
-	let   t16 =   d | t02
-	in 
-	let   t17 =   a # x  
-	in 
-	let   z   =    t17 # t15
-	in 
-	let   y   =   t16 # t14
-	in (w,x,y,z)`;
-	
-
-val RND07_def=Define
-	`RND07  (a:word32,b:word32,c:word32,d:word32)=  
-	
-	let  t01 = a & c  
-	in 
-	let   t02 = NOT d  
-	in 
-	let   t03 = a &  t02
-	in 
-	let   t04 = b | t01
-	in 
-	let   t05 = a &  b  
-	in 
-	let   t06 =  c  # t04
-	in 
-	let   z   =  t03 # t06
-	in 
-	let   t08 =  c | z  
-	in 
-	let   t09 =  d  | t05
-	in 
-	let   t10 =  a  # t08
-	in 
-	let   t11 =  t04 & z  
-	in 
-	let   x   =  t09 # t10
-	in 
-	let   t13 =  b  # x  
-	in
-	let  t14 =  t01 # x  
-	in 
-	let   t15 =  c # t05
-	in 
-	let   t16 = t11 | t13
-	in 
-	let   t17 = t02 | t14
-	in 
-	let   w   = t15  # t17
-	in 
-	let   y   = a # t16
-	in 
-	(w,x,y,z)`;
-
-val InvRND07_def= Define
-	`InvRND07  (a:word32,b:word32,c:word32,d:word32)=  
-	
-	let  t01 =  a &  b  
-	in 
-	let  t02 =  a   | b  
-	in 
-	let  t03 = c | t01
-	in 
-	let   t04 = d & t02
-	in 
-	let   z   = t03 # t04
-	in 
-	let   t06 =b # t04
-	in 
-	let   t07 = d  # z  
-	in 
-	let   t08 = NOT t07
-	in 
-	let   t09 =  t06 | t08
-	in 
-	let   t10 = b #  d 
-	in 
-	let   t11 = a | d 
-	in 
-	let   x   =  a # t09
-	in 
-	let   t13 =  c # t06
-	in 
-	let   t14 =  c & t11
-	in 
-	let   t15 =  d  | x  
-	in 
-	let   t16 = t01 | t10
-	in 
-	let   w   =   t13 # t15
-	in 
-	let   y   =   t14  # t16
-	in (w,x,y,z)`;
-
-
-val RND08_def = Define 
-	`RND08  b128=RND00  b128`;
-val RND09_def = Define 
-	`RND09  b128=RND01  b128`;
-val RND10_def = Define 
-	`RND10  b128=RND02  b128`;
-val RND11_def = Define 
-	`RND11  b128=RND03  b128`;
-val RND12_def = Define 
-	`RND12  b128=RND04  b128`;
-val RND13_def = Define 
-	`RND13  b128=RND05  b128`;
-val RND14_def = Define 
-	`RND14  b128=RND06  b128`;
-val RND15_def = Define 
-	`RND15  b128=RND07  b128`;
-val RND16_def = Define 
-	`RND16  b128=RND00  b128`;
-val RND17_def = Define 
-	`RND17  b128=RND01  b128`;
-val RND18_def = Define 
-	`RND18  b128=RND02  b128`;
-val RND19_def = Define 
-	`RND19  b128=RND03  b128`;
-val RND20_def = Define 
-	`RND20  b128=RND04  b128`;
-val RND21_def = Define 
-	`RND21  b128=RND05  b128`;
-val RND22_def = Define 
-	`RND22  b128=RND06  b128`;
-val RND23_def = Define 
-	`RND23  b128=RND07  b128`;
-val RND24_def = Define 
-	`RND24  b128=RND00  b128`;
-val RND25_def = Define 
-	`RND25  b128=RND01  b128`;
-val RND26_def = Define 
-	`RND26  b128=RND02  b128`;
-val RND27_def = Define 
-	`RND27  b128=RND03  b128`;
-val RND28_def = Define 
-	`RND28  b128=RND04  b128`;
-val RND29_def = Define 
-	`RND29  b128=RND05  b128`;
-val RND30_def = Define 
-	`RND30  b128=RND06  b128`;
-val RND31_def = Define 
-	`RND31  b128=RND07  b128`;
-
-val InvRND08_def = Define
-	`InvRND08  b128=InvRND00  b128`;
-val InvRND09_def = Define
-	`InvRND09  b128=InvRND01  b128`;
-val InvRND10_def = Define
-	`InvRND10  b128=InvRND02  b128`;
-val InvRND11_def = Define
-	`InvRND11  b128=InvRND03  b128`;
-val InvRND12_def = Define
-	`InvRND12  b128=InvRND04  b128`;
-val InvRND13_def = Define
-	`InvRND13  b128=InvRND05  b128`;
-val InvRND14_def = Define
-	`InvRND14  b128=InvRND06  b128`;
-val InvRND15_def = Define
-	`InvRND15  b128=InvRND07  b128`;
-val InvRND16_def = Define
-	`InvRND16  b128=InvRND00  b128`;
-val InvRND17_def = Define
-	`InvRND17  b128=InvRND01  b128`;
-val InvRND18_def = Define
-	`InvRND18  b128=InvRND02  b128`;
-val InvRND19_def = Define
-	`InvRND19  b128=InvRND03  b128`;
-val InvRND20_def = Define
-	`InvRND20  b128=InvRND04  b128`;
-val InvRND21_def = Define
-	`InvRND21  b128=InvRND05  b128`;
-val InvRND22_def = Define
-	`InvRND22  b128=InvRND06  b128`;
-val InvRND23_def = Define
-	`InvRND23  b128=InvRND07  b128`;
-val InvRND24_def = Define
-	`InvRND24  b128=InvRND00  b128`;
-val InvRND25_def = Define
-	`InvRND25  b128=InvRND01  b128`;
-val InvRND26_def = Define
-	`InvRND26  b128=InvRND02  b128`;
-val InvRND27_def = Define
-	`InvRND27  b128=InvRND03  b128`;
-val InvRND28_def = Define
-	`InvRND28  b128=InvRND04  b128`;
-val InvRND29_def = Define
-	`InvRND29  b128=InvRND05  b128`;
-val InvRND30_def = Define
-	`InvRND30  b128=InvRND06  b128`;
-val InvRND31_def = Define
-	`InvRND31  b128=InvRND07  b128`;
-
-val WORD_BITWISE_EQ_PROVE_TAC
-    =SIMP_TAC std_ss [word32Theory.ONE_COMP_EVAL, word32Theory.AND_EVAL,
-                      word32Theory.OR_EVAL, word32Theory.EOR_EVAL] THEN
-     SIMP_TAC std_ss [word32Theory.n2w_11,GSYM word32Theory.EQUIV_def] THEN
-     RW_TAC bool_ss [word32Theory.EOR_def, word32Theory.AND_def, word32Theory.OR_def,
-                     word32Theory.ONE_COMP_BITWISE_THM, GSYM word32Theory.BITWISE_THM2,
-		     BITWISE_THM] THEN
-     tautLib.TAUT_TAC;
-			  
-		
-val RND00_THM=Q.store_thm(
-"RND00_THM",
-`!v. 
-	InvRND00 (RND00 v) = v`,
-
-SIMP_TAC std_ss [FORALL_PROD,word32Theory.FORALL_WORD,RND00_def,
-                 InvRND00_def,LET_THM] THEN
-RW_TAC std_ss [] THENL [ 
-	WORD_BITWISE_EQ_PROVE_TAC,
-	WORD_BITWISE_EQ_PROVE_TAC,
-	WORD_BITWISE_EQ_PROVE_TAC,
-	WORD_BITWISE_EQ_PROVE_TAC]);
-
-	
-val RND01_THM=Q.store_thm(
-"RND01_THM",
-`!v. 
-	InvRND01 (RND01 v) = v`,
-
-SIMP_TAC std_ss [FORALL_PROD,word32Theory.FORALL_WORD,RND01_def,
-                 InvRND01_def,LET_THM] THEN
-RW_TAC std_ss [] THENL [ 
-	WORD_BITWISE_EQ_PROVE_TAC,
-	WORD_BITWISE_EQ_PROVE_TAC,
-	WORD_BITWISE_EQ_PROVE_TAC,
-	WORD_BITWISE_EQ_PROVE_TAC]);	
-			  
-val RND02_THM=Q.store_thm(
-"RND02_THM",
-`!v. 
-	InvRND02 (RND02 v) = v`,
-
-SIMP_TAC std_ss [FORALL_PROD,word32Theory.FORALL_WORD,RND02_def,
-                 InvRND02_def,LET_THM] THEN
-RW_TAC std_ss [] THENL [ 
-	WORD_BITWISE_EQ_PROVE_TAC,
-	WORD_BITWISE_EQ_PROVE_TAC,
-	WORD_BITWISE_EQ_PROVE_TAC,
-	WORD_BITWISE_EQ_PROVE_TAC]);
-
-val RND03_THM=Q.store_thm(
-"RND03_THM",
-`!v. 
-	InvRND03 (RND03 v) = v`,
-
-SIMP_TAC std_ss [FORALL_PROD,word32Theory.FORALL_WORD,RND03_def,
-                 InvRND03_def,LET_THM] THEN
-RW_TAC std_ss [] THENL [ 
-	WORD_BITWISE_EQ_PROVE_TAC,
-	WORD_BITWISE_EQ_PROVE_TAC,
-	WORD_BITWISE_EQ_PROVE_TAC,
-	WORD_BITWISE_EQ_PROVE_TAC]);
-
-val RND04_THM=Q.store_thm(
-"RND04_THM",
-`!v. 
-	InvRND04 (RND04 v) = v`,
-
-SIMP_TAC std_ss [FORALL_PROD,word32Theory.FORALL_WORD,RND04_def,
-                 InvRND04_def,LET_THM] THEN
-RW_TAC std_ss [] THENL [ 
-	WORD_BITWISE_EQ_PROVE_TAC,
-	WORD_BITWISE_EQ_PROVE_TAC,
-	WORD_BITWISE_EQ_PROVE_TAC,
-	WORD_BITWISE_EQ_PROVE_TAC]);
-
-val RND05_THM=Q.store_thm(
-"RND05_THM",
-`!v. 
-	InvRND05 (RND05 v) = v`,
-
-SIMP_TAC std_ss [FORALL_PROD,word32Theory.FORALL_WORD,RND05_def,
-                 InvRND05_def,LET_THM] THEN
-RW_TAC std_ss [] THENL [ 
-	WORD_BITWISE_EQ_PROVE_TAC,
-	WORD_BITWISE_EQ_PROVE_TAC,
-	WORD_BITWISE_EQ_PROVE_TAC,
-	WORD_BITWISE_EQ_PROVE_TAC]);
-
-val RND06_THM=Q.store_thm(
-"RND06_THM",
-`!v. 
-	InvRND06 (RND06 v) = v`,
-
-SIMP_TAC std_ss [FORALL_PROD,word32Theory.FORALL_WORD,RND06_def,
-                 InvRND06_def,LET_THM] THEN
-RW_TAC std_ss [] THENL [ 
-	WORD_BITWISE_EQ_PROVE_TAC,
-	WORD_BITWISE_EQ_PROVE_TAC,
-	WORD_BITWISE_EQ_PROVE_TAC,
-	WORD_BITWISE_EQ_PROVE_TAC]);
-
-val RND07_THM=Q.store_thm(
-"RND07_THM",
-`!v. 
-	InvRND07 (RND07 v) = v`,
-
-SIMP_TAC std_ss [FORALL_PROD,word32Theory.FORALL_WORD,RND07_def,
-                 InvRND07_def,LET_THM] THEN
-RW_TAC std_ss [] THENL [ 
-	WORD_BITWISE_EQ_PROVE_TAC,
-	WORD_BITWISE_EQ_PROVE_TAC,
-	WORD_BITWISE_EQ_PROVE_TAC,
-	WORD_BITWISE_EQ_PROVE_TAC]);
-
-									  
-val RND08_THM=Q.store_thm (
-"RND08_THM",
-`!v. 
-	InvRND08 (RND08 v)= v`,
-
-METIS_TAC [RND08_def,InvRND08_def,RND00_THM]);			  
-			  
-val RND09_THM=Q.store_thm (
-"RND09_THM",
-`!v. 
-	InvRND09 (RND09 v)= v`,
-
-METIS_TAC [RND09_def,InvRND09_def,RND01_THM]);			  
-			  
-val RND10_THM=Q.store_thm (
-"RND10_THM",
-`!v. 
-	InvRND10 (RND10 v)= v`,
-
-METIS_TAC [RND10_def,InvRND10_def,RND02_THM]);		
-   	  
-val RND11_THM=Q.store_thm (
-"RND11_THM",
-`!v. 
-	InvRND11 (RND11 v)= v`,
-
-METIS_TAC [RND11_def,InvRND11_def,RND03_THM]);	
-   		  
-val RND12_THM=Q.store_thm (
-"RND12_THM",
-`!v. 
-	InvRND12 (RND12 v)= v`,
-
-METIS_TAC [RND12_def,InvRND12_def,RND04_THM]);	
-
-val RND13_THM=Q.store_thm (
-"RND13_THM",
-`!v. 
-	InvRND13 (RND13 v)= v`,
-
-METIS_TAC [RND13_def,InvRND13_def,RND05_THM]);	
-
-val RND14_THM=Q.store_thm (
-"RND14_THM",
-`!v. 
-	InvRND14 (RND14 v)= v`,
-
-METIS_TAC [RND14_def,InvRND14_def,RND06_THM]);	
-
-val RND15_THM=Q.store_thm (
-"RND15_THM",
-`!v. 
-	InvRND15 (RND15 v)= v`,
-
-METIS_TAC [RND15_def,InvRND15_def,RND07_THM]);	
-
-			  
-val RND16_THM=Q.store_thm (
-"RND16_THM",
-`!v. 
-	InvRND16 (RND16 v)= v`,
-
-METIS_TAC [RND16_def,InvRND16_def,RND00_THM]);			  
-			  
-val RND17_THM=Q.store_thm (
-"RND17_THM",
-`!v. 
-	InvRND17 (RND17 v)= v`,
-
-METIS_TAC [RND17_def,InvRND17_def,RND01_THM]);			  
-			  
-val RND18_THM=Q.store_thm (
-"RND18_THM",
-`!v. 
-	InvRND18 (RND18 v)= v`,
-
-METIS_TAC [RND18_def,InvRND18_def,RND02_THM]);		
-   	  
-val RND19_THM=Q.store_thm (
-"RND19_THM",
-`!v. 
-	InvRND19 (RND19 v)= v`,
-
-METIS_TAC [RND19_def,InvRND19_def,RND03_THM]);	
-   		  
-val RND20_THM=Q.store_thm (
-"RND20_THM",
-`!v. 
-	InvRND20 (RND20 v)= v`,
-
-METIS_TAC [RND20_def,InvRND20_def,RND04_THM]);	
-
-val RND21_THM=Q.store_thm (
-"RND21_THM",
-`!v. 
-	InvRND21 (RND21 v)= v`,
-
-METIS_TAC [RND21_def,InvRND21_def,RND05_THM]);	
-
-val RND22_THM=Q.store_thm (
-"RND22_THM",
-`!v. 
-	InvRND22 (RND22 v)= v`,
-
-METIS_TAC [RND22_def,InvRND22_def,RND06_THM]);	
-
-val RND23_THM=Q.store_thm (
-"RND23_THM",
-`!v. 
-	InvRND23 (RND23 v)= v`,
-
-METIS_TAC [RND23_def,InvRND23_def,RND07_THM]);	
-   		  
-			  
-val RND24_THM=Q.store_thm (
-"RND24_THM",
-`!v. 
-	InvRND24 (RND24 v)= v`,
-
-METIS_TAC [RND24_def,InvRND24_def,RND00_THM]);			  
-			  
-val RND25_THM=Q.store_thm (
-"RND25_THM",
-`!v. 
-	InvRND25 (RND25 v)= v`,
-
-METIS_TAC [RND25_def,InvRND25_def,RND01_THM]);			  
-			  
-val RND26_THM=Q.store_thm (
-"RND26_THM",
-`!v. 
-	InvRND26 (RND26 v)= v`,
-
-METIS_TAC [RND26_def,InvRND26_def,RND02_THM]);		
-   	  
-val RND27_THM=Q.store_thm (
-"RND27_THM",
-`!v. 
-	InvRND27 (RND27 v)= v`,
-METIS_TAC [RND27_def,InvRND27_def,RND03_THM]);	
-   		  
-val RND28_THM=Q.store_thm (
-"RND28_THM",
-`!v. 
-	InvRND28 (RND28 v)= v`,
-
-METIS_TAC [RND28_def,InvRND28_def,RND04_THM]);	
-
-val RND29_THM=Q.store_thm (
-"RND29_THM",
-
-`!v. 
-	InvRND29 (RND29 v)= v`,
-
-METIS_TAC [RND29_def,InvRND29_def,RND05_THM]);	
-
-val RND30_THM=Q.store_thm (
-"RND30_THM",
-
-`!v. 
-	InvRND30 (RND30 v)= v`,
-
-METIS_TAC [RND30_def,InvRND30_def,RND06_THM]);	
-
-val RND31_THM=Q.store_thm (
-"RND31_THM",
-
-`!v. 
-	InvRND31 (RND31 v)= v`,
-
-METIS_TAC [RND31_def,InvRND31_def,RND07_THM]);	
-
-
+(* RNDxxx is the SBox in xxx round, invRNDxxx is the invSBox in xxx round *)
+
+val RND00_def = Define`
+  RND00  (a:word32,b:word32,c:word32,d:word32) =
+   (let t01 = b ?? c in
+    let t02 = a !! d in
+    let t03 = a ?? b in
+    let z = t02 ?? t01 in
+    let t05 = c !! z in
+    let t06 = a ?? d in
+    let t07 = b !! c in
+    let t08 = d && t05 in
+    let t09 = t03 && t07 in
+    let y = t09 ?? t08 in
+    let t11 = t09 && y in
+    let t12 = c ?? d in
+    let t13 = t07 ?? t11 in
+    let t14 = b && t06 in
+    let t15 = t06 ?? t13 in
+    let w = ~t15 in
+    let t17 = w ?? t14 in
+    let x = t12 ?? t17 in
+      (w,x,y,z))`;
+
+val InvRND00_def = Define`
+  InvRND00  (a:word32,b:word32,c:word32,d:word32) =
+   (let t01 = c ?? d in
+    let t02 = a !! b in
+    let t03 = b !! c in
+    let t04 = c && t01 in
+    let t05 = t02 ?? t01 in
+    let t06 = a !! t04 in
+    let y = ~t05 in
+    let t08 = b ?? d in
+    let t09 = t03 && t08 in
+    let t10 = d !! y in
+    let x = t09 ?? t06 in
+    let t12 = a !! t05 in
+    let t13 = x ?? t12 in
+    let t14 = t03 ?? t10 in
+    let t15 = a ?? c in
+    let z = t14 ?? t13 in
+    let t17 = t05 && t13 in
+    let t18 = t14 !! t17 in
+    let w = t15 ?? t18 in
+      (w,x,y,z))`;
+
+val RND01_def = Define`
+  RND01  (a:word32,b:word32,c:word32,d:word32) =
+   (let t01 = a !! d in
+    let t02 = c ?? d in
+    let t03 = ~b in
+    let t04 = a ?? c in
+    let t05 = a !! t03 in
+    let t06 = d && t04 in
+    let t07 = t01 && t02 in
+    let t08 = b !! t06 in
+    let y = t02 ?? t05 in
+    let t10 = t07 ?? t08 in
+    let t11 = t01 ?? t10 in
+    let t12 = y ?? t11 in
+    let t13 = b && d in
+    let z = ~t10 in
+    let x = t13 ?? t12 in
+    let t16 = t10 !! x in
+    let t17 = t05 && t16 in
+    let w = c ?? t17 in
+      (w,x,y,z))`;
+
+val InvRND01_def = Define`
+  InvRND01  (a:word32,b:word32,c:word32,d:word32) =
+   (let t01 = a ?? b in
+    let t02 = b !! d in
+    let t03 = a && c in
+    let t04 = c ?? t02 in
+    let t05 = a !! t04 in
+    let t06 = t01 && t05 in
+    let t07 = d !! t03 in
+    let t08 = b ?? t06 in
+    let t09 = t07 ?? t06 in
+    let t10 = t04 !! t03 in
+    let t11 = d && t08 in
+    let y = ~t09 in
+    let x = t10 ?? t11 in
+    let t14 = a !! y in
+    let t15 = t06 ?? x in
+    let z = t01 ?? t04 in
+    let t17 = c ?? t15 in
+    let w = t14 ?? t17 in
+      (w,x,y,z))`;
+
+val  RND02_def = Define`
+    RND02  (a:word32,b:word32,c:word32,d:word32) =
+   (let t01 = a !! c in
+    let t02 = a ?? b in
+    let t03 = d ?? t01 in
+    let w = t02 ?? t03 in
+    let t05 = c ?? w in
+    let t06 = b ?? t05 in
+    let t07 = b !! t05 in
+    let t08 = t01 && t06 in
+    let t09 = t03 ?? t07 in
+    let t10 = t02 !! t09 in
+    let x = t10 ?? t08 in
+    let t12 = a !! d in
+    let t13 = t09 ?? x in
+    let t14 = b ?? t13 in
+    let z = ~t09 in
+    let y = t12 ?? t14 in
+      (w,x,y,z))`;
+
+val InvRND02_def = Define`
+  InvRND02  (a:word32,b:word32,c:word32,d:word32) =
+   (let t01 = a ?? d in
+    let t02 = c ?? d in
+    let t03 = a && c in
+    let t04 = b !! t02 in
+    let w = t01 ?? t04 in
+    let t06 = a !! c in
+    let t07 = d !! w in
+    let t08 = ~d in
+    let t09 = b && t06 in
+    let t10 = t08 !! t03 in
+    let t11 = b && t07 in
+    let t12 = t06 && t02 in
+    let z = t09 ?? t10 in
+    let x = t12 ?? t11 in
+    let t15 = c && z in
+    let t16 = w ?? x in
+    let t17 = t10 ?? t15 in
+    let y = t16 ?? t17 in
+      (w,x,y,z))`;
+
+val  RND03_def = Define`
+  RND03  (a:word32,b:word32,c:word32,d:word32) =
+   (let t01 = a ?? c in
+    let t02 = a !! d in
+    let t03 = a && d in
+    let t04 = t01 && t02 in
+    let t05 = b !! t03 in
+    let t06 = a && b in
+    let t07 = d ?? t04 in
+    let t08 = c !! t06 in
+    let t09 = b ?? t07 in
+    let t10 = d && t05 in
+    let t11 = t02 ?? t10 in
+    let z = t08 ?? t09 in
+    let t13 = d !! z in
+    let t14 = a !! t07 in
+    let t15 = b && t13 in
+    let y = t08 ?? t11 in
+    let w = t14 ?? t15 in
+    let x = t05 ?? t04 in
+      (w,x,y,z))`;
+
+val  InvRND03_def = Define`
+  InvRND03  (a:word32,b:word32,c:word32,d:word32) =
+   (let t01 = c !! d in
+    let t02 = a !! d in
+    let t03 = c ?? t02 in
+    let t04 = b ?? t02 in
+    let t05 = a ?? d in
+    let t06 = t04 && t03 in
+    let t07 = b && t01 in
+    let y = t05 ?? t06 in
+    let t09 = a ?? t03 in
+    let w = t07 ?? t03 in
+    let t11 = w !! t05 in
+    let t12 = t09 && t11 in
+    let t13 = a && y in
+    let t14 = t01 ?? t05 in
+    let x = b ?? t12 in
+    let t16 = b !! t13 in
+    let z = t14 ?? t16 in
+      (w,x,y,z))`;
+
+val  RND04_def = Define`
+  RND04  (a:word32,b:word32,c:word32,d:word32) =
+   (let t01 = a !! b in
+    let t02 = b !! c in
+    let t03 = a ?? t02 in
+    let t04 = b ?? d in
+    let t05 = d !! t03 in
+    let t06 = d && t01 in
+    let z = t03 ?? t06 in
+    let t08 = z && t04 in
+    let t09 = t04 && t05 in
+    let t10 = c ?? t06 in
+    let t11 = b && c in
+    let t12 = t04 ?? t08 in
+    let t13 = t11 !! t03 in
+    let t14 = t10 ?? t09 in
+    let t15 = a && t05 in
+    let t16 = t11 !! t12 in
+    let y = t13 ?? t08 in
+    let x = t15 ?? t16 in
+    let w = ~t14 in
+      (w,x,y,z))`;
+
+val  InvRND04_def = Define`
+  InvRND04  (a:word32,b:word32,c:word32,d:word32) =
+   (let t01 = b !! d in
+    let t02 = c !! d in
+    let t03 = a && t01 in
+    let t04 = b ?? t02 in
+    let t05 = c ?? d in
+    let t06 = ~t03 in
+    let t07 = a && t04 in
+    let x = t05 ?? t07 in
+    let t09 = x !! t06 in
+    let t10 = a ?? t07 in
+    let t11 = t01 ?? t09 in
+    let t12 = d ?? t04 in
+    let t13 = c !! t10 in
+    let z = t03 ?? t12 in
+    let t15 = a ?? t04 in
+    let y = t11 ?? t13 in
+    let w = t15 ?? t09 in
+      (w,x,y,z))`;
+
+val  RND05_def = Define`
+  RND05  (a:word32,b:word32,c:word32,d:word32) =
+   (let t01 = b ?? d in
+    let t02 = b !! d in
+    let t03 = a && t01 in
+    let t04 = c ?? t02 in
+    let t05 = t03 ?? t04 in
+    let w = ~t05 in
+    let t07 = a ?? t01 in
+    let t08 = d !! w in
+    let t09 = b !! t05 in
+    let t10 = d ?? t08 in
+    let t11 = b !! t07 in
+    let t12 = t03 !! w in
+    let t13 = t07 !! t10 in
+    let t14 = t01 ?? t11 in
+    let y = t09 ?? t13 in
+    let x = t07 ?? t08 in
+    let z = t12 ?? t14 in
+      (w,x,y,z))`;
+
+val  InvRND05_def = Define`
+  InvRND05  (a:word32,b:word32,c:word32,d:word32) =
+   (let t01 = a && d in
+    let t02 = c ?? t01 in
+    let t03 = a ?? d in
+    let t04 = b && t02 in
+    let t05 = a && c in
+    let w = t03 ?? t04 in
+    let t07 = a && w in
+    let t08 = t01 ?? w in
+    let t09 = b !! t05 in
+    let t10 = ~b in
+    let x = t08 ?? t09 in
+    let t12 = t10 !! t07 in
+    let t13 = w !! x in
+    let z = t02 ?? t12 in
+    let t15 = t02 ?? t13 in
+    let t16 = b ?? d in
+    let y = t16 ?? t15 in
+      (w,x,y,z))`;
+
+val  RND06_def = Define`
+  RND06  (a:word32,b:word32,c:word32,d:word32) =
+   (let t01 = a && d in
+    let t02 = b ?? c in
+    let t03 = a ?? d in
+    let t04 = t01 ?? t02 in
+    let t05 = b !! c in
+    let x = ~t04 in
+    let t07 = t03 && t05 in
+    let t08 = b && x in
+    let t09 = a !! c in
+    let t10 = t07 ?? t08 in
+    let t11 = b !! d in
+    let t12 = c ?? t11 in
+    let t13 = t09 ?? t10 in
+    let y = ~t13 in
+    let t15 = x && t03 in
+    let z = t12 ?? t07 in
+    let t17 = a ?? b in
+    let t18 = y ?? t15 in
+    let w = t17 ?? t18 in
+      (w,x,y,z))`;
+
+val InvRND06_def = Define`
+  InvRND06  (a:word32,b:word32,c:word32,d:word32) =
+   (let t01 = a ?? c in
+    let t02 = ~c in
+    let t03 = b && t01 in
+    let t04 = b !! t02 in
+    let t05 = d !! t03 in
+    let t06 = b ?? d in
+    let t07 = a && t04 in
+    let t08 = a !! t02 in
+    let t09 = t07 ?? t05 in
+    let x = t06 ?? t08 in
+    let w = ~t09 in
+    let t12 = b && w in
+    let t13 = t01 && t05 in
+    let t14 = t01 ?? t12 in
+    let t15 = t07 ?? t13 in
+    let t16 = d !! t02 in
+    let t17 = a ?? x in
+    let z = t17 ?? t15 in
+    let y = t16 ?? t14 in
+      (w,x,y,z))`;
+
+val RND07_def = Define`
+  RND07  (a:word32,b:word32,c:word32,d:word32) =
+   (let t01 = a && c in
+    let t02 = ~d in
+    let t03 = a && t02 in
+    let t04 = b !! t01 in
+    let t05 = a && b in
+    let t06 = c ?? t04 in
+    let z = t03 ?? t06 in
+    let t08 = c !! z in
+    let t09 = d !! t05 in
+    let t10 = a ?? t08 in
+    let t11 = t04 && z in
+    let x = t09 ?? t10 in
+    let t13 = b ?? x in
+    let t14 = t01 ?? x in
+    let t15 = c ?? t05 in
+    let t16 = t11 !! t13 in
+    let t17 = t02 !! t14 in
+    let w = t15 ?? t17 in
+    let y = a ?? t16 in
+      (w,x,y,z))`;
+
+val InvRND07_def = Define`
+  InvRND07  (a:word32,b:word32,c:word32,d:word32) =
+   (let t01 = a && b in
+    let t02 = a !! b in
+    let t03 = c !! t01 in
+    let t04 = d && t02 in
+    let z = t03 ?? t04 in
+    let t06 = b ?? t04 in
+    let t07 = d ?? z in
+    let t08 = ~t07 in
+    let t09 = t06 !! t08 in
+    let t10 = b ?? d in
+    let t11 = a !! d in
+    let x = a ?? t09 in
+    let t13 = c ?? t06 in
+    let t14 = c && t11 in
+    let t15 = d !! x in
+    let t16 = t01 !! t10 in
+    let w = t13 ?? t15 in
+    let y = t14 ?? t16 in
+      (w,x,y,z))`;
+
+val RND08_def = Define `RND08 b128 = RND00 b128`;
+val RND09_def = Define `RND09 b128 = RND01 b128`;
+val RND10_def = Define `RND10 b128 = RND02 b128`;
+val RND11_def = Define `RND11 b128 = RND03 b128`;
+val RND12_def = Define `RND12 b128 = RND04 b128`;
+val RND13_def = Define `RND13 b128 = RND05 b128`;
+val RND14_def = Define `RND14 b128 = RND06 b128`;
+val RND15_def = Define `RND15 b128 = RND07 b128`;
+val RND16_def = Define `RND16 b128 = RND00 b128`;
+val RND17_def = Define `RND17 b128 = RND01 b128`;
+val RND18_def = Define `RND18 b128 = RND02 b128`;
+val RND19_def = Define `RND19 b128 = RND03 b128`;
+val RND20_def = Define `RND20 b128 = RND04 b128`;
+val RND21_def = Define `RND21 b128 = RND05 b128`;
+val RND22_def = Define `RND22 b128 = RND06 b128`;
+val RND23_def = Define `RND23 b128 = RND07 b128`;
+val RND24_def = Define `RND24 b128 = RND00 b128`;
+val RND25_def = Define `RND25 b128 = RND01 b128`;
+val RND26_def = Define `RND26 b128 = RND02 b128`;
+val RND27_def = Define `RND27 b128 = RND03 b128`;
+val RND28_def = Define `RND28 b128 = RND04 b128`;
+val RND29_def = Define `RND29 b128 = RND05 b128`;
+val RND30_def = Define `RND30 b128 = RND06 b128`;
+val RND31_def = Define `RND31 b128 = RND07 b128`;
+
+val InvRND08_def = Define `InvRND08 b128 = InvRND00 b128`;
+val InvRND09_def = Define `InvRND09 b128 = InvRND01 b128`;
+val InvRND10_def = Define `InvRND10 b128 = InvRND02 b128`;
+val InvRND11_def = Define `InvRND11 b128 = InvRND03 b128`;
+val InvRND12_def = Define `InvRND12 b128 = InvRND04 b128`;
+val InvRND13_def = Define `InvRND13 b128 = InvRND05 b128`;
+val InvRND14_def = Define `InvRND14 b128 = InvRND06 b128`;
+val InvRND15_def = Define `InvRND15 b128 = InvRND07 b128`;
+val InvRND16_def = Define `InvRND16 b128 = InvRND00 b128`;
+val InvRND17_def = Define `InvRND17 b128 = InvRND01 b128`;
+val InvRND18_def = Define `InvRND18 b128 = InvRND02 b128`;
+val InvRND19_def = Define `InvRND19 b128 = InvRND03 b128`;
+val InvRND20_def = Define `InvRND20 b128 = InvRND04 b128`;
+val InvRND21_def = Define `InvRND21 b128 = InvRND05 b128`;
+val InvRND22_def = Define `InvRND22 b128 = InvRND06 b128`;
+val InvRND23_def = Define `InvRND23 b128 = InvRND07 b128`;
+val InvRND24_def = Define `InvRND24 b128 = InvRND00 b128`;
+val InvRND25_def = Define `InvRND25 b128 = InvRND01 b128`;
+val InvRND26_def = Define `InvRND26 b128 = InvRND02 b128`;
+val InvRND27_def = Define `InvRND27 b128 = InvRND03 b128`;
+val InvRND28_def = Define `InvRND28 b128 = InvRND04 b128`;
+val InvRND29_def = Define `InvRND29 b128 = InvRND05 b128`;
+val InvRND30_def = Define `InvRND30 b128 = InvRND06 b128`;
+val InvRND31_def = Define `InvRND31 b128 = InvRND07 b128`;
+
+val tac =
+  SIMP_TAC std_ss [FORALL_PROD,LET_THM,
+    RND00_def,InvRND00_def,RND01_def,InvRND01_def,RND02_def,InvRND02_def,
+    RND03_def,InvRND03_def,RND04_def,InvRND04_def,RND05_def,InvRND05_def,
+    RND06_def,InvRND06_def,RND07_def,InvRND07_def] THEN
+  SRW_TAC [] [] THEN WORD_DECIDE_TAC;
+      
+val RND00_THM = Q.store_thm("RND00_THM", `!v. InvRND00 (RND00 v) = v`, tac);
+val RND01_THM = Q.store_thm("RND01_THM", `!v. InvRND01 (RND01 v) = v`, tac);
+val RND02_THM = Q.store_thm("RND02_THM", `!v. InvRND02 (RND02 v) = v`, tac);
+val RND03_THM = Q.store_thm("RND03_THM", `!v. InvRND03 (RND03 v) = v`, tac);
+val RND04_THM = Q.store_thm("RND04_THM", `!v. InvRND04 (RND04 v) = v`, tac);
+val RND05_THM = Q.store_thm("RND05_THM", `!v. InvRND05 (RND05 v) = v`, tac);
+val RND06_THM = Q.store_thm("RND06_THM", `!v. InvRND06 (RND06 v) = v`, tac);
+val RND07_THM = Q.store_thm("RND07_THM", `!v. InvRND07 (RND07 v) = v`, tac);
+
+val tac = METIS_TAC
+  [RND08_def,InvRND08_def,RND09_def,InvRND09_def,RND10_def,InvRND10_def,
+   RND11_def,InvRND11_def,RND12_def,InvRND12_def,RND13_def,InvRND13_def,
+   RND14_def,InvRND14_def,RND15_def,InvRND15_def,RND16_def,InvRND16_def,
+   RND17_def,InvRND17_def,RND18_def,InvRND18_def,RND19_def,InvRND19_def,
+   RND20_def,InvRND20_def,RND21_def,InvRND21_def,RND22_def,InvRND22_def,
+   RND23_def,InvRND23_def,RND24_def,InvRND24_def,RND25_def,InvRND25_def,
+   RND26_def,InvRND26_def,RND27_def,InvRND27_def,RND28_def,InvRND28_def,
+   RND29_def,InvRND29_def,RND30_def,InvRND30_def,RND31_def,InvRND31_def,
+   RND00_THM,RND01_THM,RND02_THM,RND03_THM,RND04_THM,RND05_THM,RND06_THM,
+   RND07_THM];
+
+val RND08_THM = Q.store_thm ("RND08_THM", `!v. InvRND08 (RND08 v) = v`, tac);
+val RND09_THM = Q.store_thm ("RND09_THM", `!v. InvRND09 (RND09 v) = v`, tac);
+val RND10_THM = Q.store_thm ("RND10_THM", `!v. InvRND10 (RND10 v) = v`, tac);
+val RND11_THM = Q.store_thm ("RND11_THM", `!v. InvRND11 (RND11 v) = v`, tac);
+val RND12_THM = Q.store_thm ("RND12_THM", `!v. InvRND12 (RND12 v) = v`, tac);
+val RND13_THM = Q.store_thm ("RND13_THM", `!v. InvRND13 (RND13 v) = v`, tac);
+val RND14_THM = Q.store_thm ("RND14_THM", `!v. InvRND14 (RND14 v) = v`, tac);
+val RND15_THM = Q.store_thm ("RND15_THM", `!v. InvRND15 (RND15 v) = v`, tac);
+val RND16_THM = Q.store_thm ("RND16_THM", `!v. InvRND16 (RND16 v) = v`, tac);
+val RND17_THM = Q.store_thm ("RND17_THM", `!v. InvRND17 (RND17 v) = v`, tac);
+val RND18_THM = Q.store_thm ("RND18_THM", `!v. InvRND18 (RND18 v) = v`, tac);
+val RND19_THM = Q.store_thm ("RND19_THM", `!v. InvRND19 (RND19 v) = v`, tac);
+val RND20_THM = Q.store_thm ("RND20_THM", `!v. InvRND20 (RND20 v) = v`, tac);
+val RND21_THM = Q.store_thm ("RND21_THM", `!v. InvRND21 (RND21 v) = v`, tac);
+val RND22_THM = Q.store_thm ("RND22_THM", `!v. InvRND22 (RND22 v) = v`, tac);
+val RND23_THM = Q.store_thm ("RND23_THM", `!v. InvRND23 (RND23 v) = v`, tac);
+val RND24_THM = Q.store_thm ("RND24_THM", `!v. InvRND24 (RND24 v) = v`, tac);
+val RND25_THM = Q.store_thm ("RND25_THM", `!v. InvRND25 (RND25 v) = v`, tac);
+val RND26_THM = Q.store_thm ("RND26_THM", `!v. InvRND26 (RND26 v) = v`, tac);
+val RND27_THM = Q.store_thm ("RND27_THM", `!v. InvRND27 (RND27 v) = v`, tac);
+val RND28_THM = Q.store_thm ("RND28_THM", `!v. InvRND28 (RND28 v) = v`, tac);
+val RND29_THM = Q.store_thm ("RND29_THM", `!v. InvRND29 (RND29 v) = v`, tac);
+val RND30_THM = Q.store_thm ("RND30_THM", `!v. InvRND30 (RND30 v) = v`, tac);
+val RND31_THM = Q.store_thm ("RND31_THM", `!v. InvRND31 (RND31 v) = v`, tac);
 
 val _ = export_theory();
