examples/Crypto/Serpent/Reference/Serpent_Reference_TransformationScript.sml
@@ -1,7 +1,7 @@
 
-open HolKernel Parse boolLib bossLib listTheory rich_listTheory bitsTheory
-     markerTheory metisLib pairTheory arithmeticTheory numSyntax word128Theory
-     Serpent_Reference_UtilityTheory word128Lib;
+open HolKernel Parse boolLib bossLib listTheory rich_listTheory bitTheory
+     markerTheory pairTheory arithmeticTheory numSyntax wordsTheory
+     Serpent_Reference_UtilityTheory wordsLib;
 
 val _ = new_theory "Serpent_Reference_Transformation";
 
@@ -13,11 +13,11 @@ val _ = new_theory "Serpent_Reference_Transformation";
 (* for efficient evaluation in the place of BOUNDED_FORALL_THM               *)
 (*---------------------------------------------------------------------------*)
 
-val row_conv = 
-  REPEATC (numLib.BOUNDED_FORALL_CONV EVAL) THENC REWRITE_CONV [];      
+val row_conv =
+  REPEATC (numLib.BOUNDED_FORALL_CONV EVAL) THENC REWRITE_CONV [];     
 
-val LTTable_def=Define
-`LTTable= 
+val LTTable_def = Define
+`LTTable =
 [
 [16;52;56;70;83;94;105];
 [72;114;125];
@@ -147,13 +147,12 @@ val LTTable_def=Define
 [68;110;121];
 [5;11;26;80;122;126];
 [32;86;99]
-]`;      
+]`;     
 
-(*linear transformation table 
-used in decryption
-*)
-val InvLTTable_def=Define
-`InvLTTable= 
+(* linear transformation table used in decryption *)
+
+val InvLTTable_def = Define
+`InvLTTable =
 [
 [53;55;72];
 [1;5;20;90];
@@ -285,1033 +284,762 @@ val InvLTTable_def=Define
 [4;27;86;97;113;115;127]
 ]`;
 
-val LTFun_def = Define
-`LTFun x = EL x LTTable`;
+val LTFun_def = Define `LTFun x = EL x LTTable`;
 
-val invLTFun_def = Define
-`invLTFun x = EL x InvLTTable`;
+val invLTFun_def = Define `invLTFun x = EL x InvLTTable`;
 
-val LTFunVal=Q.store_thm(
+val LTFunVal = Q.store_thm(
 "LTFunVal",
 `
-(LTFun 0= [ 16;52;56;70;83;94;105])  /\
-(LTFun 1= [ 72;114;125])  /\
-(LTFun 2= [ 2;9;15;30;76;84;126])  /\
-(LTFun 3= [ 36;90;103])  /\
-(LTFun 4= [ 20;56;60;74;87;98;109])  /\
-(LTFun 5= [ 1;76;118])  /\
-(LTFun 6= [ 2;6;13;19;34;80;88])  /\
-(LTFun 7= [ 40;94;107])  /\
-(LTFun 8= [ 24;60;64;78;91;102;113])  /\
-(LTFun 9= [ 5;80;122])  /\
-(LTFun 10= [ 6;10;17;23;38;84;92])  /\
-(LTFun 11= [ 44;98;111])  /\
-(LTFun 12= [ 28;64;68;82;95;106;117])  /\
-(LTFun 13= [ 9;84;126])  /\
-(LTFun 14= [ 10;14;21;27;42;88;96])  /\
-(LTFun 15= [ 48;102;115])  /\
-(LTFun 16= [ 32;68;72;86;99;110;121])  /\
-(LTFun 17= [ 2;13;88])  /\
-(LTFun 18= [ 14;18;25;31;46;92;100])  /\
-(LTFun 19= [ 52;106;119])  /\
-(LTFun 20= [ 36;72;76;90;103;114;125])  /\
-(LTFun 21= [ 6;17;92])  /\
-(LTFun 22= [ 18;22;29;35;50;96;104])  /\
-(LTFun 23= [ 56;110;123])  /\
-(LTFun 24= [ 1;40;76;80;94;107;118])  /\
-(LTFun 25= [ 10;21;96])  /\
-(LTFun 26= [ 22;26;33;39;54;100;108])  /\
-(LTFun 27= [ 60;114;127])  /\
-(LTFun 28= [ 5;44;80;84;98;111;122])  /\
-(LTFun 29= [ 14;25;100])  /\
-(LTFun 30= [ 26;30;37;43;58;104;112])  /\
-(LTFun 31= [ 3;118])  /\
-(LTFun 32= [ 9;48;84;88;102;115;126])  /\
-(LTFun 33= [ 18;29;104])  /\
-(LTFun 34= [ 30;34;41;47;62;108;116])  /\
-(LTFun 35= [ 7;122])  /\
-(LTFun 36= [ 2;13;52;88;92;106;119])  /\
-(LTFun 37= [ 22;33;108])  /\
-(LTFun 38= [ 34;38;45;51;66;112;120])  /\
-(LTFun 39= [ 11;126])  /\
-(LTFun 40= [ 6;17;56;92;96;110;123])  /\
-(LTFun 41= [ 26;37;112])  /\
-(LTFun 42= [ 38;42;49;55;70;116;124])  /\
-(LTFun 43= [ 2;15;76])  /\
-(LTFun 44= [ 10;21;60;96;100;114;127])  /\
-(LTFun 45= [ 30;41;116])  /\
-(LTFun 46= [ 0;42;46;53;59;74;120])  /\
-(LTFun 47= [ 6;19;80])  /\
-(LTFun 48= [ 3;14;25;100;104;118])  /\
-(LTFun 49= [ 34;45;120])  /\
-(LTFun 50= [ 4;46;50;57;63;78;124])  /\
-(LTFun 51= [ 10;23;84])  /\
-(LTFun 52= [ 7;18;29;104;108;122])  /\
-(LTFun 53= [ 38;49;124])  /\
-(LTFun 54= [ 0;8;50;54;61;67;82])  /\
-(LTFun 55= [ 14;27;88])  /\
-(LTFun 56= [ 11;22;33;108;112;126])  /\
-(LTFun 57= [ 0;42;53])  /\
-(LTFun 58= [ 4;12;54;58;65;71;86])  /\
-(LTFun 59= [ 18;31;92])  /\
-(LTFun 60= [ 2;15;26;37;76;112;116])  /\
-(LTFun 61= [ 4;46;57])  /\
-(LTFun 62= [ 8;16;58;62;69;75;90])  /\
-(LTFun 63= [ 22;35;96])  /\
-(LTFun 64= [ 6;19;30;41;80;116;120])  /\
-(LTFun 65= [ 8;50;61])  /\
-(LTFun 66= [ 12;20;62;66;73;79;94])  /\
-(LTFun 67= [ 26;39;100])  /\
-(LTFun 68= [ 10;23;34;45;84;120;124])  /\
-(LTFun 69= [ 12;54;65])  /\
-(LTFun 70= [ 16;24;66;70;77;83;98])  /\
-(LTFun 71= [ 30;43;104])  /\
-(LTFun 72= [ 0;14;27;38;49;88;124])  /\
-(LTFun 73= [ 16;58;69])  /\
-(LTFun 74= [ 20;28;70;74;81;87;102])  /\
-(LTFun 75= [ 34;47;108])  /\
-(LTFun 76= [ 0;4;18;31;42;53;92])  /\
-(LTFun 77= [ 20;62;73])  /\
-(LTFun 78= [ 24;32;74;78;85;91;106])  /\
-(LTFun 79= [ 38;51;112])  /\
-(LTFun 80= [ 4;8;22;35;46;57;96])  /\
-(LTFun 81= [ 24;66;77])  /\
-(LTFun 82= [ 28;36;78;82;89;95;110])  /\
-(LTFun 83= [ 42;55;116])  /\
-(LTFun 84= [ 8;12;26;39;50;61;100])  /\
-(LTFun 85= [ 28;70;81])  /\
-(LTFun 86= [ 32;40;82;86;93;99;114])  /\
-(LTFun 87= [ 46;59;120])  /\
-(LTFun 88= [ 12;16;30;43;54;65;104])  /\
-(LTFun 89= [ 32;74;85])  /\
-(LTFun 90= [ 36;90;103;118])  /\
-(LTFun 91= [ 50;63;124])  /\
-(LTFun 92= [ 16;20;34;47;58;69;108])  /\
-(LTFun 93= [ 36;78;89])  /\
-(LTFun 94= [ 40;94;107;122])  /\
-(LTFun 95= [ 0;54;67])  /\
-(LTFun 96= [ 20;24;38;51;62;73;112])  /\
-(LTFun 97= [ 40;82;93])  /\
-(LTFun 98= [ 44;98;111;126])  /\
-(LTFun 99= [ 4;58;71])  /\
-(LTFun 100= [ 24;28;42;55;66;77;116])  /\
-(LTFun 101= [ 44;86;97])  /\
-(LTFun 102= [ 2;48;102;115])  /\
-(LTFun 103= [ 8;62;75])  /\
-(LTFun 104= [ 28;32;46;59;70;81;120])  /\
-(LTFun 105= [ 48;90;101])  /\
-(LTFun 106= [ 6;52;106;119])  /\
-(LTFun 107= [ 12;66;79])  /\
-(LTFun 108= [ 32;36;50;63;74;85;124])  /\
-(LTFun 109= [ 52;94;105])  /\
-(LTFun 110= [ 10;56;110;123])  /\
-(LTFun 111= [ 16;70;83])  /\
-(LTFun 112= [ 0;36;40;54;67;78;89])  /\
-(LTFun 113= [ 56;98;109])  /\
-(LTFun 114= [ 14;60;114;127])  /\
-(LTFun 115= [ 20;74;87])  /\
-(LTFun 116= [ 4;40;44;58;71;82;93])  /\
-(LTFun 117= [ 60;102;113])  /\
-(LTFun 118= [ 3;18;72;114;118;125])  /\
-(LTFun 119= [ 24;78;91])  /\
-(LTFun 120= [ 8;44;48;62;75;86;97])  /\
-(LTFun 121= [ 64;106;117])  /\
-(LTFun 122= [ 1;7;22;76;118;122])  /\
-(LTFun 123= [ 28;82;95])  /\
-(LTFun 124= [ 12;48;52;66;79;90;101])  /\
-(LTFun 125= [ 68;110;121])  /\
-(LTFun 126= [ 5;11;26;80;122;126])  /\
-(LTFun 127= [ 32;86;99])`,
+(LTFun 0 = [ 16;52;56;70;83;94;105])  /\
+(LTFun 1 = [ 72;114;125])  /\
+(LTFun 2 = [ 2;9;15;30;76;84;126])  /\
+(LTFun 3 = [ 36;90;103])  /\
+(LTFun 4 = [ 20;56;60;74;87;98;109])  /\
+(LTFun 5 = [ 1;76;118])  /\
+(LTFun 6 = [ 2;6;13;19;34;80;88])  /\
+(LTFun 7 = [ 40;94;107])  /\
+(LTFun 8 = [ 24;60;64;78;91;102;113])  /\
+(LTFun 9 = [ 5;80;122])  /\
+(LTFun 10 = [ 6;10;17;23;38;84;92])  /\
+(LTFun 11 = [ 44;98;111])  /\
+(LTFun 12 = [ 28;64;68;82;95;106;117])  /\
+(LTFun 13 = [ 9;84;126])  /\
+(LTFun 14 = [ 10;14;21;27;42;88;96])  /\
+(LTFun 15 = [ 48;102;115])  /\
+(LTFun 16 = [ 32;68;72;86;99;110;121])  /\
+(LTFun 17 = [ 2;13;88])  /\
+(LTFun 18 = [ 14;18;25;31;46;92;100])  /\
+(LTFun 19 = [ 52;106;119])  /\
+(LTFun 20 = [ 36;72;76;90;103;114;125])  /\
+(LTFun 21 = [ 6;17;92])  /\
+(LTFun 22 = [ 18;22;29;35;50;96;104])  /\
+(LTFun 23 = [ 56;110;123])  /\
+(LTFun 24 = [ 1;40;76;80;94;107;118])  /\
+(LTFun 25 = [ 10;21;96])  /\
+(LTFun 26 = [ 22;26;33;39;54;100;108])  /\
+(LTFun 27 = [ 60;114;127])  /\
+(LTFun 28 = [ 5;44;80;84;98;111;122])  /\
+(LTFun 29 = [ 14;25;100])  /\
+(LTFun 30 = [ 26;30;37;43;58;104;112])  /\
+(LTFun 31 = [ 3;118])  /\
+(LTFun 32 = [ 9;48;84;88;102;115;126])  /\
+(LTFun 33 = [ 18;29;104])  /\
+(LTFun 34 = [ 30;34;41;47;62;108;116])  /\
+(LTFun 35 = [ 7;122])  /\
+(LTFun 36 = [ 2;13;52;88;92;106;119])  /\
+(LTFun 37 = [ 22;33;108])  /\
+(LTFun 38 = [ 34;38;45;51;66;112;120])  /\
+(LTFun 39 = [ 11;126])  /\
+(LTFun 40 = [ 6;17;56;92;96;110;123])  /\
+(LTFun 41 = [ 26;37;112])  /\
+(LTFun 42 = [ 38;42;49;55;70;116;124])  /\
+(LTFun 43 = [ 2;15;76])  /\
+(LTFun 44 = [ 10;21;60;96;100;114;127])  /\
+(LTFun 45 = [ 30;41;116])  /\
+(LTFun 46 = [ 0;42;46;53;59;74;120])  /\
+(LTFun 47 = [ 6;19;80])  /\
+(LTFun 48 = [ 3;14;25;100;104;118])  /\
+(LTFun 49 = [ 34;45;120])  /\
+(LTFun 50 = [ 4;46;50;57;63;78;124])  /\
+(LTFun 51 = [ 10;23;84])  /\
+(LTFun 52 = [ 7;18;29;104;108;122])  /\
+(LTFun 53 = [ 38;49;124])  /\
+(LTFun 54 = [ 0;8;50;54;61;67;82])  /\
+(LTFun 55 = [ 14;27;88])  /\
+(LTFun 56 = [ 11;22;33;108;112;126])  /\
+(LTFun 57 = [ 0;42;53])  /\
+(LTFun 58 = [ 4;12;54;58;65;71;86])  /\
+(LTFun 59 = [ 18;31;92])  /\
+(LTFun 60 = [ 2;15;26;37;76;112;116])  /\
+(LTFun 61 = [ 4;46;57])  /\
+(LTFun 62 = [ 8;16;58;62;69;75;90])  /\
+(LTFun 63 = [ 22;35;96])  /\
+(LTFun 64 = [ 6;19;30;41;80;116;120])  /\
+(LTFun 65 = [ 8;50;61])  /\
+(LTFun 66 = [ 12;20;62;66;73;79;94])  /\
+(LTFun 67 = [ 26;39;100])  /\
+(LTFun 68 = [ 10;23;34;45;84;120;124])  /\
+(LTFun 69 = [ 12;54;65])  /\
+(LTFun 70 = [ 16;24;66;70;77;83;98])  /\
+(LTFun 71 = [ 30;43;104])  /\
+(LTFun 72 = [ 0;14;27;38;49;88;124])  /\
+(LTFun 73 = [ 16;58;69])  /\
+(LTFun 74 = [ 20;28;70;74;81;87;102])  /\
+(LTFun 75 = [ 34;47;108])  /\
+(LTFun 76 = [ 0;4;18;31;42;53;92])  /\
+(LTFun 77 = [ 20;62;73])  /\
+(LTFun 78 = [ 24;32;74;78;85;91;106])  /\
+(LTFun 79 = [ 38;51;112])  /\
+(LTFun 80 = [ 4;8;22;35;46;57;96])  /\
+(LTFun 81 = [ 24;66;77])  /\
+(LTFun 82 = [ 28;36;78;82;89;95;110])  /\
+(LTFun 83 = [ 42;55;116])  /\
+(LTFun 84 = [ 8;12;26;39;50;61;100])  /\
+(LTFun 85 = [ 28;70;81])  /\
+(LTFun 86 = [ 32;40;82;86;93;99;114])  /\
+(LTFun 87 = [ 46;59;120])  /\
+(LTFun 88 = [ 12;16;30;43;54;65;104])  /\
+(LTFun 89 = [ 32;74;85])  /\
+(LTFun 90 = [ 36;90;103;118])  /\
+(LTFun 91 = [ 50;63;124])  /\
+(LTFun 92 = [ 16;20;34;47;58;69;108])  /\
+(LTFun 93 = [ 36;78;89])  /\
+(LTFun 94 = [ 40;94;107;122])  /\
+(LTFun 95 = [ 0;54;67])  /\
+(LTFun 96 = [ 20;24;38;51;62;73;112])  /\
+(LTFun 97 = [ 40;82;93])  /\
+(LTFun 98 = [ 44;98;111;126])  /\
+(LTFun 99 = [ 4;58;71])  /\
+(LTFun 100 = [ 24;28;42;55;66;77;116])  /\
+(LTFun 101 = [ 44;86;97])  /\
+(LTFun 102 = [ 2;48;102;115])  /\
+(LTFun 103 = [ 8;62;75])  /\
+(LTFun 104 = [ 28;32;46;59;70;81;120])  /\
+(LTFun 105 = [ 48;90;101])  /\
+(LTFun 106 = [ 6;52;106;119])  /\
+(LTFun 107 = [ 12;66;79])  /\
+(LTFun 108 = [ 32;36;50;63;74;85;124])  /\
+(LTFun 109 = [ 52;94;105])  /\
+(LTFun 110 = [ 10;56;110;123])  /\
+(LTFun 111 = [ 16;70;83])  /\
+(LTFun 112 = [ 0;36;40;54;67;78;89])  /\
+(LTFun 113 = [ 56;98;109])  /\
+(LTFun 114 = [ 14;60;114;127])  /\
+(LTFun 115 = [ 20;74;87])  /\
+(LTFun 116 = [ 4;40;44;58;71;82;93])  /\
+(LTFun 117 = [ 60;102;113])  /\
+(LTFun 118 = [ 3;18;72;114;118;125])  /\
+(LTFun 119 = [ 24;78;91])  /\
+(LTFun 120 = [ 8;44;48;62;75;86;97])  /\
+(LTFun 121 = [ 64;106;117])  /\
+(LTFun 122 = [ 1;7;22;76;118;122])  /\
+(LTFun 123 = [ 28;82;95])  /\
+(LTFun 124 = [ 12;48;52;66;79;90;101])  /\
+(LTFun 125 = [ 68;110;121])  /\
+(LTFun 126 = [ 5;11;26;80;122;126])  /\
+(LTFun 127 = [ 32;86;99])`,
+EVAL_TAC);     
 
-EVAL_TAC);      
+(* linear transformation table used in decryption *)
 
-(*linear transformation table 
-used in decryption
-*)
-val invLTFunVal=Q.store_thm(
+val invLTFunVal = Q.store_thm(
 "invLTFunVal",
 `
-(invLTFun 0= [53;55;72])  /\
-(invLTFun 1= [1;5;20;90])  /\
-(invLTFun 2= [15;102])  /\
-(invLTFun 3= [3;31;90])  /\
-(invLTFun 4= [57;59;76])  /\
-(invLTFun 5= [5;9;24;94])  /\
-(invLTFun 6= [19;106])  /\
-(invLTFun 7= [7;35;94])  /\
-(invLTFun 8= [61;63;80])  /\
-(invLTFun 9= [9;13;28;98])  /\
-(invLTFun 10= [23;110])  /\
-(invLTFun 11= [11;39;98])  /\
-(invLTFun 12= [65;67;84])  /\
-(invLTFun 13= [13;17;32;102])  /\
-(invLTFun 14= [27;114])  /\
-(invLTFun 15= [1;3;15;20;43;102])  /\
-(invLTFun 16= [69;71;88])  /\
-(invLTFun 17= [17;21;36;106])  /\
-(invLTFun 18= [1;31;118])  /\
-(invLTFun 19= [5;7;19;24;47;106])  /\
-(invLTFun 20= [73;75;92])  /\
-(invLTFun 21= [21;25;40;110])  /\
-(invLTFun 22= [5;35;122])  /\
-(invLTFun 23= [9;11;23;28;51;110])  /\
-(invLTFun 24= [77;79;96])  /\
-(invLTFun 25= [25;29;44;114])  /\
-(invLTFun 26= [9;39;126])  /\
-(invLTFun 27= [13;15;27;32;55;114])  /\
-(invLTFun 28= [81;83;100])  /\
-(invLTFun 29= [1;29;33;48;118])  /\
-(invLTFun 30= [2;13;43])  /\
-(invLTFun 31= [1;17;19;31;36;59;118])  /\
-(invLTFun 32= [85;87;104])  /\
-(invLTFun 33= [5;33;37;52;122])  /\
-(invLTFun 34= [6;17;47])  /\
-(invLTFun 35= [5;21;23;35;40;63;122])  /\
-(invLTFun 36= [89;91;108])  /\
-(invLTFun 37= [9;37;41;56;126])  /\
-(invLTFun 38= [10;21;51])  /\
-(invLTFun 39= [9;25;27;39;44;67;126])  /\
-(invLTFun 40= [93;95;112])  /\
-(invLTFun 41= [2;13;41;45;60])  /\
-(invLTFun 42= [14;25;55])  /\
-(invLTFun 43= [2;13;29;31;43;48;71])  /\
-(invLTFun 44= [97;99;116])  /\
-(invLTFun 45= [6;17;45;49;64])  /\
-(invLTFun 46= [18;29;59])  /\
-(invLTFun 47= [6;17;33;35;47;52;75])  /\
-(invLTFun 48= [101;103;120])  /\
-(invLTFun 49= [10;21;49;53;68])  /\
-(invLTFun 50= [22;33;63])  /\
-(invLTFun 51= [10;21;37;39;51;56;79])  /\
-(invLTFun 52= [105;107;124])  /\
-(invLTFun 53= [14;25;53;57;72])  /\
-(invLTFun 54= [26;37;67])  /\
-(invLTFun 55= [14;25;41;43;55;60;83])  /\
-(invLTFun 56= [0;109;111])  /\
-(invLTFun 57= [18;29;57;61;76])  /\
-(invLTFun 58= [30;41;71])  /\
-(invLTFun 59= [18;29;45;47;59;64;87])  /\
-(invLTFun 60= [4;113;115])  /\
-(invLTFun 61= [22;33;61;65;80])  /\
-(invLTFun 62= [34;45;75])  /\
-(invLTFun 63= [22;33;49;51;63;68;91])  /\
-(invLTFun 64= [8;117;119])  /\
-(invLTFun 65= [26;37;65;69;84])  /\
-(invLTFun 66= [38;49;79])  /\
-(invLTFun 67= [26;37;53;55;67;72;95])  /\
-(invLTFun 68= [12;121;123])  /\
-(invLTFun 69= [30;41;69;73;88])  /\
-(invLTFun 70= [42;53;83])  /\
-(invLTFun 71= [30;41;57;59;71;76;99])  /\
-(invLTFun 72= [16;125;127])  /\
-(invLTFun 73= [34;45;73;77;92])  /\
-(invLTFun 74= [46;57;87])  /\
-(invLTFun 75= [34;45;61;63;75;80;103])  /\
-(invLTFun 76= [1;3;20])  /\
-(invLTFun 77= [38;49;77;81;96])  /\
-(invLTFun 78= [50;61;91])  /\
-(invLTFun 79= [38;49;65;67;79;84;107])  /\
-(invLTFun 80= [5;7;24])  /\
-(invLTFun 81= [42;53;81;85;100])  /\
-(invLTFun 82= [54;65;95])  /\
-(invLTFun 83= [42;53;69;71;83;88;111])  /\
-(invLTFun 84= [9;11;28])  /\
-(invLTFun 85= [46;57;85;89;104])  /\
-(invLTFun 86= [58;69;99])  /\
-(invLTFun 87= [46;57;73;75;87;92;115])  /\
-(invLTFun 88= [13;15;32])  /\
-(invLTFun 89= [50;61;89;93;108])  /\
-(invLTFun 90= [62;73;103])  /\
-(invLTFun 91= [50;61;77;79;91;96;119])  /\
-(invLTFun 92= [17;19;36])  /\
-(invLTFun 93= [54;65;93;97;112])  /\
-(invLTFun 94= [66;77;107])  /\
-(invLTFun 95= [54;65;81;83;95;100;123])  /\
-(invLTFun 96= [21;23;40])  /\
-(invLTFun 97= [58;69;97;101;116])  /\
-(invLTFun 98= [70;81;111])  /\
-(invLTFun 99= [58;69;85;87;99;104;127])  /\
-(invLTFun 100= [25;27;44])  /\
-(invLTFun 101= [62;73;101;105;120])  /\
-(invLTFun 102= [74;85;115])  /\
-(invLTFun 103= [3;62;73;89;91;103;108])  /\
-(invLTFun 104= [29;31;48])  /\
-(invLTFun 105= [66;77;105;109;124])  /\
-(invLTFun 106= [78;89;119])  /\
-(invLTFun 107= [7;66;77;93;95;107;112])  /\
-(invLTFun 108= [33;35;52])  /\
-(invLTFun 109= [0;70;81;109;113])  /\
-(invLTFun 110= [82;93;123])  /\
-(invLTFun 111= [11;70;81;97;99;111;116])  /\
-(invLTFun 112= [37;39;56])  /\
-(invLTFun 113= [4;74;85;113;117])  /\
-(invLTFun 114= [86;97;127])  /\
-(invLTFun 115= [15;74;85;101;103;115;120])  /\
-(invLTFun 116= [41;43;60])  /\
-(invLTFun 117= [8;78;89;117;121])  /\
-(invLTFun 118= [3;90])  /\
-(invLTFun 119= [19;78;89;105;107;119;124])  /\
-(invLTFun 120= [45;47;64])  /\
-(invLTFun 121= [12;82;93;121;125])  /\
-(invLTFun 122= [7;94])  /\
-(invLTFun 123= [0;23;82;93;109;111;123])  /\
-(invLTFun 124= [49;51;68])  /\
-(invLTFun 125= [1;16;86;97;125])  /\
-(invLTFun 126= [11;98])  /\
-(invLTFun 127= [4;27;86;97;113;115;127])`,
-
+(invLTFun 0 = [53;55;72])  /\
+(invLTFun 1 = [1;5;20;90])  /\
+(invLTFun 2 = [15;102])  /\
+(invLTFun 3 = [3;31;90])  /\
+(invLTFun 4 = [57;59;76])  /\
+(invLTFun 5 = [5;9;24;94])  /\
+(invLTFun 6 = [19;106])  /\
+(invLTFun 7 = [7;35;94])  /\
+(invLTFun 8 = [61;63;80])  /\
+(invLTFun 9 = [9;13;28;98])  /\
+(invLTFun 10 = [23;110])  /\
+(invLTFun 11 = [11;39;98])  /\
+(invLTFun 12 = [65;67;84])  /\
+(invLTFun 13 = [13;17;32;102])  /\
+(invLTFun 14 = [27;114])  /\
+(invLTFun 15 = [1;3;15;20;43;102])  /\
+(invLTFun 16 = [69;71;88])  /\
+(invLTFun 17 = [17;21;36;106])  /\
+(invLTFun 18 = [1;31;118])  /\
+(invLTFun 19 = [5;7;19;24;47;106])  /\
+(invLTFun 20 = [73;75;92])  /\
+(invLTFun 21 = [21;25;40;110])  /\
+(invLTFun 22 = [5;35;122])  /\
+(invLTFun 23 = [9;11;23;28;51;110])  /\
+(invLTFun 24 = [77;79;96])  /\
+(invLTFun 25 = [25;29;44;114])  /\
+(invLTFun 26 = [9;39;126])  /\
+(invLTFun 27 = [13;15;27;32;55;114])  /\
+(invLTFun 28 = [81;83;100])  /\
+(invLTFun 29 = [1;29;33;48;118])  /\
+(invLTFun 30 = [2;13;43])  /\
+(invLTFun 31 = [1;17;19;31;36;59;118])  /\
+(invLTFun 32 = [85;87;104])  /\
+(invLTFun 33 = [5;33;37;52;122])  /\
+(invLTFun 34 = [6;17;47])  /\
+(invLTFun 35 = [5;21;23;35;40;63;122])  /\
+(invLTFun 36 = [89;91;108])  /\
+(invLTFun 37 = [9;37;41;56;126])  /\
+(invLTFun 38 = [10;21;51])  /\
+(invLTFun 39 = [9;25;27;39;44;67;126])  /\
+(invLTFun 40 = [93;95;112])  /\
+(invLTFun 41 = [2;13;41;45;60])  /\
+(invLTFun 42 = [14;25;55])  /\
+(invLTFun 43 = [2;13;29;31;43;48;71])  /\
+(invLTFun 44 = [97;99;116])  /\
+(invLTFun 45 = [6;17;45;49;64])  /\
+(invLTFun 46 = [18;29;59])  /\
+(invLTFun 47 = [6;17;33;35;47;52;75])  /\
+(invLTFun 48 = [101;103;120])  /\
+(invLTFun 49 = [10;21;49;53;68])  /\
+(invLTFun 50 = [22;33;63])  /\
+(invLTFun 51 = [10;21;37;39;51;56;79])  /\
+(invLTFun 52 = [105;107;124])  /\
+(invLTFun 53 = [14;25;53;57;72])  /\
+(invLTFun 54 = [26;37;67])  /\
+(invLTFun 55 = [14;25;41;43;55;60;83])  /\
+(invLTFun 56 = [0;109;111])  /\
+(invLTFun 57 = [18;29;57;61;76])  /\
+(invLTFun 58 = [30;41;71])  /\
+(invLTFun 59 = [18;29;45;47;59;64;87])  /\
+(invLTFun 60 = [4;113;115])  /\
+(invLTFun 61 = [22;33;61;65;80])  /\
+(invLTFun 62 = [34;45;75])  /\
+(invLTFun 63 = [22;33;49;51;63;68;91])  /\
+(invLTFun 64 = [8;117;119])  /\
+(invLTFun 65 = [26;37;65;69;84])  /\
+(invLTFun 66 = [38;49;79])  /\
+(invLTFun 67 = [26;37;53;55;67;72;95])  /\
+(invLTFun 68 = [12;121;123])  /\
+(invLTFun 69 = [30;41;69;73;88])  /\
+(invLTFun 70 = [42;53;83])  /\
+(invLTFun 71 = [30;41;57;59;71;76;99])  /\
+(invLTFun 72 = [16;125;127])  /\
+(invLTFun 73 = [34;45;73;77;92])  /\
+(invLTFun 74 = [46;57;87])  /\
+(invLTFun 75 = [34;45;61;63;75;80;103])  /\
+(invLTFun 76 = [1;3;20])  /\
+(invLTFun 77 = [38;49;77;81;96])  /\
+(invLTFun 78 = [50;61;91])  /\
+(invLTFun 79 = [38;49;65;67;79;84;107])  /\
+(invLTFun 80 = [5;7;24])  /\
+(invLTFun 81 = [42;53;81;85;100])  /\
+(invLTFun 82 = [54;65;95])  /\
+(invLTFun 83 = [42;53;69;71;83;88;111])  /\
+(invLTFun 84 = [9;11;28])  /\
+(invLTFun 85 = [46;57;85;89;104])  /\
+(invLTFun 86 = [58;69;99])  /\
+(invLTFun 87 = [46;57;73;75;87;92;115])  /\
+(invLTFun 88 = [13;15;32])  /\
+(invLTFun 89 = [50;61;89;93;108])  /\
+(invLTFun 90 = [62;73;103])  /\
+(invLTFun 91 = [50;61;77;79;91;96;119])  /\
+(invLTFun 92 = [17;19;36])  /\
+(invLTFun 93 = [54;65;93;97;112])  /\
+(invLTFun 94 = [66;77;107])  /\
+(invLTFun 95 = [54;65;81;83;95;100;123])  /\
+(invLTFun 96 = [21;23;40])  /\
+(invLTFun 97 = [58;69;97;101;116])  /\
+(invLTFun 98 = [70;81;111])  /\
+(invLTFun 99 = [58;69;85;87;99;104;127])  /\
+(invLTFun 100 = [25;27;44])  /\
+(invLTFun 101 = [62;73;101;105;120])  /\
+(invLTFun 102 = [74;85;115])  /\
+(invLTFun 103 = [3;62;73;89;91;103;108])  /\
+(invLTFun 104 = [29;31;48])  /\
+(invLTFun 105 = [66;77;105;109;124])  /\
+(invLTFun 106 = [78;89;119])  /\
+(invLTFun 107 = [7;66;77;93;95;107;112])  /\
+(invLTFun 108 = [33;35;52])  /\
+(invLTFun 109 = [0;70;81;109;113])  /\
+(invLTFun 110 = [82;93;123])  /\
+(invLTFun 111 = [11;70;81;97;99;111;116])  /\
+(invLTFun 112 = [37;39;56])  /\
+(invLTFun 113 = [4;74;85;113;117])  /\
+(invLTFun 114 = [86;97;127])  /\
+(invLTFun 115 = [15;74;85;101;103;115;120])  /\
+(invLTFun 116 = [41;43;60])  /\
+(invLTFun 117 = [8;78;89;117;121])  /\
+(invLTFun 118 = [3;90])  /\
+(invLTFun 119 = [19;78;89;105;107;119;124])  /\
+(invLTFun 120 = [45;47;64])  /\
+(invLTFun 121 = [12;82;93;121;125])  /\
+(invLTFun 122 = [7;94])  /\
+(invLTFun 123 = [0;23;82;93;109;111;123])  /\
+(invLTFun 124 = [49;51;68])  /\
+(invLTFun 125 = [1;16;86;97;125])  /\
+(invLTFun 126 = [11;98])  /\
+(invLTFun 127 = [4;27;86;97;113;115;127])`,
 EVAL_TAC);
 
 
-(*compute the parity on select bits*)
+(* compute the parity on select bits *)
 
 val selParity_def = Define
-`(selParity (w:word128)[]=F) /\
- (selParity w (pos::t) = boolXor (word128$WORD_BIT pos w) (selParity w t))`;
+`(selParity (w:word128) [] = F) /\
+ (selParity w (pos::t) = boolXor (w ' pos) (selParity w t))`;
 
-val selParityAppend=Q.store_thm(
-"selParityAppend",
-`!w l1 l2.
-	selParity w (l1++l2) =boolXor (selParity w l1) (selParity w l2)`,
-
-Induct_on `l1` THEN 
-RW_TAC list_ss [selParity_def] THENL [
-	METIS_TAC [boolXorFacts,boolXorComm],
-	METIS_TAC [boolXorAssoc,selParity_def]]);
-	
+val selParityAppend = Q.store_thm(
+ "selParityAppend",
+ `!w l1 l2. selParity w (l1++l2) = boolXor (selParity w l1) (selParity w l2)`,
+ Induct_on `l1` THEN
+ RW_TAC list_ss [selParity_def] THEN
+ METIS_TAC [boolXorFacts,boolXorComm,boolXorAssoc,selParity_def]);
 
 (*linear transform*)
+
 val transform_def = Define
-`(transform transFun 0 (w:word128) 
-  = let newBit=selParity w (transFun 0) 
+`(transform transFun 0 (w:word128)
+  = let newBit = selParity w (transFun 0)
     in
-    if newBit 
-       then (1w:word128) 
+    if newBit
+       then (1w:word128)
        else (0w:word128))
  /\
- (transform transFun (SUC i) w 
- = let newBit=selParity w (transFun (SUC i)) 
+ (transform transFun (SUC i) w
+ = let newBit = selParity w (transFun (SUC i))
    in
-   let newWord=if newBit 
+   let newWord = if newBit
                   then ((1w:word128)<<(SUC i))
-		  else (0w:word128)
+          else (0w:word128)
    in
-   newWord | transform transFun i w)`;
-		 
-
+   newWord !! transform transFun i w)`;
 
 val transformEval = Q.store_thm(
-"transformEval",
-`!n transFun (w:word128). 
-	transform transFun n w = 
-		if n=0 
-		   then let newBit=selParity w (transFun 0) 
-		        in
-			if newBit 
-			   then (1w:word128) 
-			   else (0w:word128)
-		   else	let newBit=selParity w (transFun n) 
-		        in
- 		 	let newWord=if newBit 
-			               then ((1w:word128)<<n)
-		 	               else (0w:word128)
-	  	 	in
-		 	newWord | transform transFun (n-1) w`,
+ "transformEval",
+ `!n transFun (w:word128).
+    transform transFun n w =
+        if n = 0
+           then let newBit = selParity w (transFun 0)
+                in
+            if newBit
+               then (1w:word128)
+               else (0w:word128)
+           else    let newBit = selParity w (transFun n)
+                in
+              let newWord = if newBit
+                           then ((1w:word128)<<n)
+                            else (0w:word128)
+               in
+             newWord !! transform transFun (n-1) w`,
+  RW_TAC std_ss [transform_def,LET_THM] THEN
+  (Cases_on `n` THENL [
+     METIS_TAC [],
+     FULL_SIMP_TAC arith_ss [transform_def,LET_THM]]));
 
-RW_TAC std_ss [transform_def,LET_THM] THENL [
-	Cases_on `n` THENL [
-		METIS_TAC [],
-		FULL_SIMP_TAC arith_ss [transform_def,LET_THM]],
-	Cases_on `n` THENL [
-		METIS_TAC [],
-		FULL_SIMP_TAC arith_ss [transform_def,LET_THM]]]);
-		 
+val LT_def = Define `LT w =  transform LTFun 127 w`;
 
+val invLT_def = Define `invLT w =  transform invLTFun 127 w`;
 
-		 
+(*desired properties of transform*)
 
-val LT_def = Define
-`LT w =  transform LTFun word128$HB w`;
+val transform_inv1_w128 = Q.store_thm(
+ "transform_inv1_w128",
+ `!to d w transFun.
+     to < 128 /\
+      d < 128 /\
+     to > d
+     ==>
+     ~((transform transFun d w) ' to)`,
+  Induct_on `d` THEN
+  SRW_TAC [ARITH_ss,WORD_BIT_EQ_ss] [transform_def,LET_THM]);
 
+val transform_inv2_w128 = Q.store_thm(
+ "transform_inv2_w128",
+ `!to d w transFun.
+     to < 128 /\
+      d < 128 /\
+     to <= d
+     ==>
+     ((transform transFun d w) ' to = selParity w (transFun to))`,
+ Induct_on `d` THEN
+  SRW_TAC [ARITH_ss,WORD_BIT_EQ_ss] [transform_def,LET_THM] THEN
+  `d < 128` by DECIDE_TAC THEN
+  Cases_on `to <= d` THEN
+  ASM_SIMP_TAC arith_ss [] THEN
+  `to = SUC d` by DECIDE_TAC THEN
+  ASM_SIMP_TAC arith_ss [transform_inv1_w128]);
+    
+(* the composite of two linear transformations *)       
 
-val invLT_def = Define
-`invLT w =  transform invLTFun word128$HB w`;
+val transCompose_def = Define `transCompose f1 f2 = \x. FLAT (MAP f1 (f2 x))`;
 
-(*desired properties of transform*) 
-val transform_inv1_w128=Q.store_thm(
-"transform_inv1_w128",
-`!to d w transFun.
-	 to < word128$WL /\ 
-         d < word128$WL /\
-	 to >d 
-	 ==>
-	 ~(word128$WORD_BIT to (transform transFun d w))`, 
+(* a transform function is legal *)
 
-Induct_on `d` THEN 
-RW_TAC arith_ss [transform_def,LET_THM] THEN
-RW_TAC arith_ss [word128Theory.WORD_BIT_BOOLOPS,word128Theory.WORD_BIT_LSL,
-                 word128Theory.WORD_BIT_def,word_1_bit128,w2n_zero128,
-		 BIT_ZERO,w2n_zero128 ]);
+val transInRange_def = Define
+ `transInRange transFun =
+    !i. i < 128 ==> ALL_EL (\x. x < 128) (transFun i)`;
 
+val LTFunInRange = Q.store_thm(
+ "LTFunInRange",
+ `transInRange LTFun`,
+ SIMP_TAC std_ss [transInRange_def] THEN CONV_TAC (time row_conv));
 
-val transform_inv2_w128=Q.store_thm(
-"transform_inv2_w128",
-`!to d w transFun.
-	 to < word128$WL /\ 
-         d < word128$WL /\
-	 to <=d 
-	 ==>
-	 (word128$WORD_BIT to (transform transFun d w) 
-	  = selParity w (transFun to))`,
+val invLTFunInRange = Q.store_thm(
+ "invLTFunInRange",
+ `transInRange invLTFun`,
+ SIMP_TAC std_ss [transInRange_def] THEN CONV_TAC (time row_conv));
 
+(* desired properties of composite of linear transformations *)
 
-Induct_on `d` THEN 
-RW_TAC arith_ss [transform_def,LET_THM] THENL [
-	FULL_SIMP_TAC arith_ss [word128Theory.WORD_BIT_def,
-	                        w2n_one128,BIT_def, BITS_THM ],
-	FULL_SIMP_TAC arith_ss [word128Theory.WORD_BIT_def, 
-	                        w2n_zero128,BIT_def, BITS_THM ],
-	Cases_on `to <=d`  THEN Cases_on `to=d` THENL [
-		RW_TAC arith_ss [word128Theory.WORD_BIT_BOOLOPS,
-		                 word128Theory.WORD_BIT_LSL],
-		RW_TAC arith_ss [word128Theory.WORD_BIT_BOOLOPS,
-		                 word128Theory.WORD_BIT_LSL],
-		FULL_SIMP_TAC arith_ss [],
-		`to = SUC d` by RW_TAC arith_ss [] THEN
-		FULL_SIMP_TAC arith_ss [word128Theory.WORD_BIT_BOOLOPS,
-		                        word128Theory.WORD_BIT_LSL,
-					word128Theory.WORD_BIT_def,
-					w2n_one128,BIT_def, BITS_THM]],
-		FULL_SIMP_TAC arith_ss [word128Theory.WORD_BIT_BOOLOPS,
-		                        word128Theory.WORD_BIT_def, 
-					w2n_zero128, BIT_ZERO,
-					DECIDE ``SUC x<y==>x<y``] THEN
-		Cases_on `to<=d` THENL [
-			FULL_SIMP_TAC arith_ss [],
-			`to>d /\ (to = SUC d)` 
-				by METIS_TAC [DECIDE ``~(x<=y) /\ 
-					               x <= SUC y=(x=SUC y) /\
-						       (x>y)``] THEN
-			FULL_SIMP_TAC arith_ss [GSYM word128Theory.WORD_BIT_def,
-			                        transform_inv1_w128]]]
-);
+val transformComposeLemma = Q.store_thm(
+ "transformComposeLemma",
+ `!transFun1 transL2 w.
+    transInRange transFun1  /\
+    ALL_EL (\x. x < 128) transL2
+    ==>
+    (selParity (transform transFun1 127 w) transL2
+     = selParity w (FLAT (MAP transFun1 transL2)))`,
+ Induct_on `transL2` THEN
+ FULL_SIMP_TAC list_ss
+   [MAP,FLAT,selParity_def,transform_def,selParityAppend,transform_inv2_w128]);
 
+val transformComposeBit = Q.store_thm(
+ "transformComposeBit",
+ `!i transFun1 transFun2 w.
+    i < 128                 /\  
+    transInRange transFun1  /\
+    transInRange transFun2 
+    ==>
+    ((transform transFun2 127 (transform transFun1 127 w)) ' i =
+     (transform (transCompose transFun1 transFun2) 127 w) ' i)`,
+ RW_TAC arith_ss [transCompose_def,transInRange_def,transform_inv2_w128,
+                  transformComposeLemma]);   
 
-(*the composite of two linear transformations*)		
-val transCompose_def=Define
-`transCompose f1 f2 = \x. FLAT (MAP f1 (f2 x))`;
+val transformComposeWord = Q.store_thm(
+ "transformComposeWord",
+ `!transFun1 transFun2 w.
+    transInRange transFun1  /\
+    transInRange transFun2 
+    ==>
+    (transform transFun2 127 (transform transFun1 127 w) =
+     transform (transCompose transFun1 transFun2) 127 w)`,
+ SRW_TAC [WORD_BIT_EQ_ss] [transformComposeBit]);
 
-(*a transform function is legal*)
-val transInRange_def=Define
- `transInRange transFun = 
-!i. i < word128$WL==> ALL_EL (\x. x < word128$WL) (transFun i)`;
+val TL128_eq_makeTL128 = save_thm(
+ "TL128_eq_makeTL128", SYM (EVAL ``makeTL 128``));
+         
+(* the intermediate values of the composite of the two given linear
+   transformation functions, used to speed up the verification *)
 
-val LTFunInRange=Q.store_thm(
-"LTFunInRange",
-`transInRange LTFun`,
-
-SIMP_TAC std_ss [transInRange_def,word128Theory.WL_def,word128Theory.HB_def] THEN
-CONV_TAC (time row_conv));
-
-val invLTFunInRange=Q.store_thm(
-"invLTFunInRange",
-`transInRange invLTFun`,
-
-SIMP_TAC std_ss [transInRange_def,word128Theory.WL_def,word128Theory.HB_def] THEN
-CONV_TAC (time row_conv));
-
-(*desired properties of composite of linear transformations*) 
-val transformComposeLemma=Q.store_thm(
-"transformComposeLemma",
-`!transFun1 transL2 w.
-	transInRange transFun1  /\
-	ALL_EL (\x. x < word128$WL) transL2
-	==>
-	(selParity (transform transFun1 word128$HB w) transL2
-	 = selParity w (FLAT (MAP transFun1 transL2)))`,
-
-Induct_on `transL2` THEN 
-FULL_SIMP_TAC list_ss [MAP,FLAT,selParity_def,transform_def,selParityAppend,
-                       word128Theory.WL_def,word128Theory.HB_def,
-		       transform_inv2_w128]); 
-
-val transformComposeBit=Q.store_thm(
-"transformComposeBit",
-`!i transFun1 transFun2 w.
-	i < word128$WL          /\   
-	transInRange transFun1  /\
-	transInRange transFun2  
-	==>
-	(word128$WORD_BIT i (transform transFun2 word128$HB 
-	                               (transform transFun1 word128$HB w))
-	 = word128$WORD_BIT i (transform (transCompose transFun1 transFun2)
-	                                 word128$HB w))`,
-
-RW_TAC arith_ss [transCompose_def,transInRange_def,transform_inv2_w128,
-                 word128Theory.WL_def,word128Theory.HB_def,
-		 transformComposeLemma]);	
-
-val transformComposeWord=Q.store_thm(
-"transformComposeWord",
-`!transFun1 transFun2 w.
-	transInRange transFun1  /\
-	transInRange transFun2  
-	==>
-	(transform transFun2 word128$HB (transform transFun1 word128$HB w) 
-	 = transform (transCompose transFun1 transFun2) word128$HB w)`,
-	
-RW_TAC std_ss[GSYM word128Theory.WORD_EQ,transformComposeBit]);
-
-
-
-val TL128_eq_makeTL128=Q.store_thm(
-"TL128_eq_makeTL128",
-`T::T::T::T::T::T::T::T::T::T::T::T::T::T::T::T::T::T::T::T::T::T::T::T::T::T::
-  T::T::T::T::T::T::T::T::T::T::T::T::T::T::T::T::T::T::T::T::T::T::T::T::T::T::
-  T::T::T::T::T::T::T::T::T::T::T::T::T::T::T::T::T::T::T::T::T::T::T::T::T::T::
-  T::T::T::T::T::T::T::T::T::T::T::T::T::T::T::T::T::T::T::T::T::T::T::T::T::T::
-  T::T::T::T::T::T::T::T::T::T::T::T::T::T::T::T::T::T::T::T::T::T::T::T::[]
-  =makeTL 128`,
-
-EVAL_TAC);	  
-	      
-(*the intermediate values of the composite of the two given linear transformation functions,
-used to speed up the verification*)
 val Res_def = Define `Res i = FLAT (MAP LTFun (invLTFun i))`;
+
 (*load "numSyntax";
 quietdec := true;
 open numSyntax;
 quietdec := false;*)
-val ResTable = 
-  LIST_CONJ
-           (map EVAL (map (fn i => ``Res ^(term_of_int i)``) (upto 0 127)));
 
-val _=computeLib.add_thms[ResTable] computeLib.the_compset;
+val ResTable =
+  LIST_CONJ (map EVAL (map (fn i => ``Res ^(term_of_int i)``) (upto 0 127)));
 
-		
-(*parity check is the same as counting EVEN or ODD.
-countEvenL and countEven is the two equivalent description,
-while countEvenL reduce a layer of loop*)
-val countL_def=Define
-`(countL l []=l) /\
- (countL l (h::t)=let x=makeL h 
+val _ = computeLib.add_thms [ResTable] computeLib.the_compset;
+       
+(* parity check is the same as counting EVEN or ODD.
+   countEvenL and countEven is the two equivalent description,
+   while countEvenL reduce a layer of loop *)
+
+val countL_def = Define
+`(countL l []= l) /\
+ (countL l (h::t) = let x = makeL h
                   in
-                  let tmp=zipXor x l 
-		  in 
+                  let tmp = zipXor x l
+          in
                   countL tmp t)`;
 
+val countEvenL_def = Define`
+ countEvenL tl =
+   countL 
+     [T; T; T; T; T; T; T; T; T; T; T; T; T; T; T; T; T; T; T; T; T; T; T;
+       T; T; T; T; T; T; T; T; T; T; T; T; T; T; T; T; T; T; T; T; T; T; T;
+       T; T; T; T; T; T; T; T; T; T; T; T; T; T; T; T; T; T; T; T; T; T; T;
+       T; T; T; T; T; T; T; T; T; T; T; T; T; T; T; T; T; T; T; T; T; T; T;
+       T; T; T; T; T; T; T; T; T; T; T; T; T; T; T; T; T; T; T; T; T; T; T;
+       T; T; T; T; T; T; T; T; T; T; T; T; T] tl`;
+         
+val countEvenL_LT_facts = Q.store_thm(
+ "countEvenL_LT_facts",
+ `!i.
+    i < 128
+    ==>
+        (countEvenL (Res i) = countEvenL [i]) `,
+ SIMP_TAC std_ss [] THEN CONV_TAC (time row_conv) THEN REWRITE_TAC []);   
 
-val countEvenL_def=Define
-`countEvenL tl 
- = countL (T::T::T::T::T::T::T::T::T::T::T::T::T::T::T::T::T::T::
-           T::T::T::T::T::T::T::T::T::T::T::T::T::T::T::T::T::T::
-	   T::T::T::T::T::T::T::T::T::T::T::T::T::T::T::T::T::T::
-	   T::T::T::T::T::T::T::T::T::T::T::T::T::T::T::T::T::T::
-	   T::T::T::T::T::T::T::T::T::T::T::T::T::T::T::T::T::T::
-	   T::T::T::T::T::T::T::T::T::T::T::T::T::T::T::T::T::T::
-	   T::T::T::T::T::T::T::T::T::T::T::T::T::T::T::T::T::T::
-	   T::T::[]) 
-	  tl`;
-	      
-	
-val countEvenL_LT_facts=Q.store_thm(
-"countEvenL_LT_facts",
-`!i. 
-	i<word128$WL 
-	==>
-        (countEvenL  (Res i)= countEvenL  [i]) `,
+val countEven_def = Define`
+ (countEven x [] = T) /\
+ (countEven x (h::t) = boolXor (x = h) (countEven x t))`;
 
-SIMP_TAC std_ss [word128Theory.WL_def,word128Theory.HB_def] THEN
-CONV_TAC (time row_conv) THEN
-REWRITE_TAC []);	
+val countL_fact = Q.store_thm(
+ "countL_fact",
+ `!i al h tl.
+    i < LENGTH al  /\
+    h < LENGTH al  /\
+    ALL_EL (\x. x < LENGTH al) tl
+    ==>
+    (EL i (countL (zipXor (makeL h) al) tl) =
+     boolXor (i = h) (EL i (countL al tl)))`,
+ Induct_on `tl` THEN
+ RW_TAC list_ss [countL_def,LET_THM,zipXor_makeL,
+                 zipXor_makeL_COMM,LENGTH_zipXor,boolXorComm3]);
 
+val Res_fact = Q.store_thm(
+ "Res_fact",
+ `!i.
+    i < 128
+    ==>
+    ALL_EL (\x. x < 128) (Res i)`,
+ SIMP_TAC std_ss [] THEN CONV_TAC (time row_conv));
 
+(* equivalence between countEven and countEvenL *)   
 
-val countEven_def=Define
-`(countEven x [] =T) /\
- (countEven x (h::t)= boolXor (x=h) (countEven x t))`;
+val countEvenL_countEven_eq = Q.store_thm(
+ "countEvenL_countEven_eq",
+ `!i tl.
+    i < 128 /\
+    ALL_EL (\x. x < 128) tl     
+    ==>
+    (EL i (countEvenL tl) = countEven i tl)`,
+ SIMP_TAC std_ss [] THEN
+ Induct_on `tl` THENL [
+   FULL_SIMP_TAC arith_ss [countEvenL_def,countEven_def,countL_def,
+                           TL128_eq_makeTL128,makeTL_fact],
+   
+   FULL_SIMP_TAC std_ss [ALL_EL,countEvenL_def,countEven_def,countL_def,
+                         LET_THM,TL128_eq_makeTL128,makeTL_fact,
+                         zipXor_makeL_COMM,LENGTH_zipXor,boolXorComm3,
+                         LENGTH_makeTL] THEN
+   FULL_SIMP_TAC std_ss [countEven_def,countL_fact,countEvenL_def,
+                         TL128_eq_makeTL128,LENGTH_makeTL]]);   
 
-val countL_fact=Q.store_thm(
-"countL_fact",
-`!i al h tl. 
-	i < LENGTH al  /\
-	h < LENGTH al  /\
-	ALL_EL (\x. x < LENGTH al) tl
-	==>
-	(EL i (countL (zipXor (makeL h) al) tl) = 
-	 boolXor (i=h) (EL i (countL al tl)))`,
+val LTFun_invLTFun_fact = Q.store_thm(
+ "LTFun_invLTFun_fact",
+ `!i.
+    i < 128
+    ==>
+    !j.
+         j < 128
+         ==>
+         (countEven j ((transCompose LTFun invLTFun) i)
+          = countEven j [i])`,
+ RW_TAC std_ss [GSYM Res_def, transCompose_def, GSYM countEvenL_countEven_eq,
+                countEvenL_LT_facts,Res_fact,ALL_EL]);
 
-Induct_on `tl` THEN 
-RW_TAC list_ss [countL_def,LET_THM,zipXor_makeL,
-                zipXor_makeL_COMM,LENGTH_zipXor,boolXorComm3]);
+(* desired properties of countEven *)
 
-
-
-val Res_fact=Q.store_thm(
-"Res_fact",
-`!i.
-	i < word128$WL
-	==>
-	ALL_EL (\x. x < word128$WL) (Res i)`,
-
-SIMP_TAC std_ss [word128Theory.WL_def,word128Theory.HB_def] THEN
-CONV_TAC (time row_conv));
-
-(*equivalence between countEven and countEvenL*)	
-
-
-val countEvenL_countEven_eq=Q.store_thm(
-"countEvenL_countEven_eq",
-`!i tl. 
-	i < word128$WL /\
-	ALL_EL (\x. x < word128$WL) tl      
-	==>
-	(EL i (countEvenL tl)=countEven i tl)`,
-	
-SIMP_TAC std_ss [word128Theory.WL_def,word128Theory.HB_def] THEN
-Induct_on `tl` THENL [
-	FULL_SIMP_TAC arith_ss [countEvenL_def,countEven_def,countL_def,
-	                        TL128_eq_makeTL128,makeTL_fact],
-	
-	FULL_SIMP_TAC std_ss [ALL_EL,countEvenL_def,countEven_def,countL_def,
-	                      LET_THM,TL128_eq_makeTL128,makeTL_fact,
-			      zipXor_makeL_COMM,LENGTH_zipXor,boolXorComm3,
-			      LENGTH_makeTL] THEN
-	FULL_SIMP_TAC std_ss [countEven_def,countL_fact,countEvenL_def,
-	                      TL128_eq_makeTL128,LENGTH_makeTL]]);	
-
-
-
-
-val LTFun_invLTFun_fact=Q.store_thm(
-"LTFun_invLTFun_fact",
-`!i. 
-	i<word128$WL 
-	==>
-	!j.
-		 j<word128$WL
-		 ==>
-		 (countEven j ((transCompose LTFun invLTFun) i) 
-		  = countEven j [i])`,
-
-RW_TAC std_ss [GSYM Res_def, transCompose_def,
-               GSYM countEvenL_countEven_eq,countEvenL_LT_facts,Res_fact,ALL_EL]);
-
-(*desired properties of countEven*) 
-
-val countEven_filter1=Q.store_thm(
-"countEven_filter1",
-`!i L d transL.
-	LENGTH transL <= L /\
-	i < d+1  /\
-	ALL_EL (\x. x < d+1) transL
-	
-	==>
-	countEven i (FILTER (\x. ~(x = i)) transL)`,	
-	
-Induct_on `L` THEN 
-RW_TAC arith_ss [countEven_def,ALL_EL,LENGTH_NIL,FILTER] THEN 
-Cases_on `transL` THEN 
-RW_TAC arith_ss [countEven_def,ALL_EL,LENGTH_NIL,FILTER] THEN  
-FULL_SIMP_TAC list_ss [boolXor_def] THEN
-METIS_TAC []);	
-			         
+val countEven_filter1 = Q.store_thm(
+ "countEven_filter1",
+ `!i L d transL.
+    LENGTH transL <= L /\
+    i < d+1  /\
+    ALL_EL (\x. x < d+1) transL
+   
+    ==>
+    countEven i (FILTER (\x. ~(x = i)) transL)`,   
+ Induct_on `L` THEN
+ RW_TAC arith_ss [countEven_def,ALL_EL,LENGTH_NIL,FILTER] THEN
+ Cases_on `transL` THEN
+ RW_TAC arith_ss [countEven_def,ALL_EL,LENGTH_NIL,FILTER] THEN 
+ FULL_SIMP_TAC list_ss [boolXor_def] THEN
+ METIS_TAC []);   
 
 
-val countEven_filter2=Q.store_thm(
-"countEven_filter2",
-`!i k L d transL.
-	LENGTH transL <= L /\
-	i < d+1  /\
-	k < d+1  /\
-	ALL_EL (\x. x < d+1) transL
-	==>
-	(countEven k (FILTER (\x. ~(x = i)) transL)
-	 = if k=i 
-	      then T
-	      else countEven k transL)`,
+val countEven_filter2 = Q.store_thm(
+ "countEven_filter2",
+ `!i k L d transL.
+    LENGTH transL <= L /\
+    i < d+1  /\
+    k < d+1  /\
+    ALL_EL (\x. x < d+1) transL
+    ==>
+    (countEven k (FILTER (\x. ~(x = i)) transL)
+     = if k = i
+          then T
+          else countEven k transL)`,
+ Induct_on `L` THEN
+ RW_TAC arith_ss [countEven_def,ALL_EL,LENGTH_NIL,FILTER] THEN
+ Cases_on `transL` THEN
+ FULL_SIMP_TAC list_ss [countEven_def,ALL_EL,LENGTH_NIL,FILTER]THEN
+ Cases_on `k = i` THEN Cases_on `h = i` THEN
+ RW_TAC std_ss [boolXor_def,countEven_def] THEN
+ METIS_TAC []);
+   
+val countEven_filter3 = Q.store_thm(
+ "countEven_filter3",
+ `!i k L d transL1 transL2.
+    LENGTH transL1 <= L /\
+    LENGTH transL2 <= L /\
+    (!j. j < d+1 ==> (countEven j transL1 = countEven j transL2)) /\
+    i < d+1  /\
+    k < d+1  /\
+    ALL_EL (\x. x < d+1) transL1 /\
+    ALL_EL (\x. x < d+1) transL2
+    ==>
+    (countEven k (FILTER (\x. ~(x = i)) transL1) =
+     countEven k (FILTER (\x. ~(x = i)) transL2))`,  
+ RW_TAC std_ss [] THEN METIS_TAC [countEven_filter2]);
 
-		
-Induct_on `L` THEN 
-RW_TAC arith_ss [countEven_def,ALL_EL,LENGTH_NIL,FILTER] THEN
-Cases_on `transL` THEN
-FULL_SIMP_TAC list_ss [countEven_def,ALL_EL,LENGTH_NIL,FILTER]THEN
-Cases_on `k=i` THEN Cases_on `h=i` THENL [
-	METIS_TAC [boolXor_def,countEven_def],
-	RW_TAC std_ss [boolXor_def,countEven_def] THEN 
-	METIS_TAC [],
-	RW_TAC std_ss [boolXor_def,countEven_def] THEN 
-	METIS_TAC [],
-	METIS_TAC [boolXor_def,countEven_def]]);
-	
-val countEven_filter3=Q.store_thm(
-"countEven_filter3",
-`!i k L d transL1 transL2.
-	LENGTH transL1 <= L /\
-	LENGTH transL2 <= L /\
-	(!j. j < d+1 ==> (countEven j transL1 = countEven j transL2)) /\
-	i < d+1  /\
-	k < d+1  /\
-	ALL_EL (\x. x < d+1) transL1 /\
-	ALL_EL (\x. x < d+1) transL2
-	==>
-	(countEven k (FILTER (\x. ~(x = i)) transL1) 
-	 = countEven k (FILTER (\x. ~(x = i)) transL2))`,   
+(* desired properties of selParity *)    
 
-RW_TAC std_ss [] THEN METIS_TAC [countEven_filter2]);
+val selParity_filter = Q.store_thm(
+ "selParity_filter",
+ `!i transL w.
+    i < 128 /\
+    ALL_EL (\x. x < 128) transL
+    ==>
+    (selParity w transL
+     = if countEven i transL
+          then  selParity w (FILTER (\x. ~(x = i)) transL)
+          else  boolXor (w ' i) (selParity w (FILTER (\x. ~(x = i)) transL)))`,
+ Induct_on `transL`  THEN1 METIS_TAC [FILTER,countEven_def] THEN
+   SRW_TAC [] [selParity_def,countEven_def,FILTER,ALL_EL] THEN
+   FULL_SIMP_TAC std_ss [boolXor_def] THEN METIS_TAC []);
 
+(*equivalence between two position list used in selParity*)
 
+val selParity_eq1 = Q.store_thm(
+ "selParity_eq1",
+ `!L transL1 transL2 w.
+    ALL_EL (\x. x < 128) transL1 /\
+    ALL_EL (\x. x < 128) transL2 /\
+    LENGTH transL1 <= L /\
+    LENGTH transL2 <= L /\
+    (!j. j < 128 ==> (countEven j transL1 = countEven j transL2 ))
+    ==>
+    (selParity w transL1  = selParity w transL2)`,
+ Induct_on `L` THEN
+ RW_TAC arith_ss [boolXor_def,countEven_def,selParity_def,LENGTH_NIL] THEN
+ Cases_on `transL1` THEN Cases_on `transL2` THENL [
+    RW_TAC arith_ss [selParity_def],
+    `h < 128` by FULL_SIMP_TAC list_ss [ALL_EL] THEN
+    `!j. j < 128 ==>
+      countEven j (FILTER (\x. ~(x = h)) (h::t)) = countEven h (h::t)`
+      by METIS_TAC [countEven_def, countEven_filter2,
+                    numLib.num_CONV ``128``, ADD1] THEN
+    `!j:num. countEven j []` by METIS_TAC [countEven_def] THEN
+    `!j. j < 128 ==> countEven j (FILTER (\x. ~(x = h)) (h::t))`
+      by METIS_TAC [countEven_def] THEN
+    FULL_SIMP_TAC bool_ss [FILTER] THEN
+    `LENGTH (FILTER (\x. ~(x = h)) t) <= L`
+      by (FULL_SIMP_TAC list_ss [] THEN
+          METIS_TAC [LENGTH_FILTER, LESS_EQ_TRANS]) THEN
+    `LENGTH ([]:num list) <= L` by RW_TAC arith_ss [LENGTH] THEN
+    `ALL_EL (\x. x < 128) t` by FULL_SIMP_TAC list_ss [ALL_EL] THEN
+    `!j. j < 128 ==> (countEven j [] = countEven j (FILTER (\x. ~(x = h)) t))`
+       by METIS_TAC [] THEN
+    `ALL_EL (\x. x < 128) (FILTER (\x. ~(x = h)) t)`
+       by METIS_TAC [ALL_EL_FILTER] THEN
+    `selParity w [] = selParity w (FILTER (\x. ~(x = h)) t)`
+       by METIS_TAC [] THEN
+     `countEven h (h::t)` by METIS_TAC [] THEN
+     `~countEven h t`
+       by FULL_SIMP_TAC std_ss [countEven_def,boolXor_def] THEN
+     METIS_TAC [selParity_filter, boolXor_def, selParity_def, countEven_def],
+    `h < 128` by FULL_SIMP_TAC list_ss [ALL_EL] THEN
+    `!j. j < 128 ==>
+      countEven j (FILTER (\x. ~(x = h)) (h::t)) = countEven h (h::t)`
+      by METIS_TAC [countEven_def, countEven_filter2,
+                    numLib.num_CONV ``128``, ADD1] THEN
+    `!j:num. countEven j []` by METIS_TAC [countEven_def] THEN
+    `!j. j < 128 ==> countEven j (FILTER (\x. ~(x = h)) (h::t))`
+      by METIS_TAC [countEven_def] THEN
+    FULL_SIMP_TAC bool_ss [FILTER] THEN
+    `LENGTH (FILTER (\x. ~(x = h)) t) <= L`
+      by (FULL_SIMP_TAC list_ss [] THEN
+          METIS_TAC [LENGTH_FILTER, LESS_EQ_TRANS]) THEN
+    `LENGTH ([]:num list) <= L` by RW_TAC arith_ss [LENGTH] THEN
+    `ALL_EL (\x. x < 128) t` by FULL_SIMP_TAC list_ss [ALL_EL] THEN
+    `!j. j < 128 ==> (countEven j [] = countEven j (FILTER (\x. ~(x = h)) t))`
+       by METIS_TAC [] THEN
+    `ALL_EL (\x. x < 128) (FILTER (\x. ~(x = h)) t)`
+       by METIS_TAC [ALL_EL_FILTER] THEN
+    `selParity w [] = selParity w (FILTER (\x. ~(x = h)) t)`
+       by METIS_TAC [] THEN
+     `countEven h (h::t)` by METIS_TAC [] THEN
+     `~countEven h t`
+       by FULL_SIMP_TAC std_ss [countEven_def,boolXor_def] THEN
+     METIS_TAC [selParity_filter, boolXor_def, selParity_def, countEven_def],
+    `(h < 128) /\ (h' < 128)` by FULL_SIMP_TAC std_ss [ALL_EL] THEN
+    `!j. j < 128 ==>
+        (countEven j (FILTER (\x. ~(x = h')) (h::t)) =
+         countEven j (FILTER (\x. ~(x = h')) (h'::t')))`
+         by METIS_TAC [countEven_def, numLib.num_CONV ``128``, ADD1,
+                       countEven_filter3] THEN
+    `ALL_EL (\x. x < 128) (FILTER (\x. ~(x = h')) (h::t)) /\
+     ALL_EL (\x. x < 128) (FILTER (\x. ~(x = h')) (h'::t'))`
+        by METIS_TAC [ALL_EL_FILTER] THEN
+    `LENGTH (FILTER (\x. ~(x = h')) (h::t)) <= LENGTH (h::t) /\
+     LENGTH (FILTER (\x. ~(x = h')) (h'::t')) <= LENGTH (h'::t')`
+        by FULL_SIMP_TAC arith_ss [LENGTH_FILTER] THEN
+    `LENGTH (FILTER (\x. ~(x = h')) (h'::t')) <= SUC L /\
+     LENGTH (FILTER (\x. ~(x = h')) (h::t)) <= SUC L`
+        by FULL_SIMP_TAC arith_ss [] THEN
+    `!j. j < 128 ==>
+        (countEven j (FILTER (\x. ~(x = h)) (FILTER (\x. ~(x = h')) (h::t))) =
+         countEven j (FILTER (\x. ~(x = h)) (FILTER (\x. ~(x = h')) (h'::t'))))`
+        by METIS_TAC [countEven_filter3,ADD1,numLib.num_CONV ``128``] THEN
+    `(FILTER (\x. ~(x = h)) (FILTER (\x. ~(x = h')) (h::t)) =
+      FILTER (\x. ~(x = h)) (FILTER (\x. ~(x = h')) t)) /\
+     (FILTER (\x. ~(x = h)) (FILTER (\x. ~(x = h')) (h'::t')) =
+      FILTER (\x. ~(x = h)) (FILTER (\x. ~(x = h')) t'))`
+        by  RW_TAC list_ss [FILTER_COMM, FILTER] THEN
+    `ALL_EL (\x. x < 128)
+            (FILTER (\x. ~(x = h)) (FILTER (\x. ~(x = h')) (h'::t'))) /\
+     ALL_EL (\x. x < 128)
+            (FILTER (\x. ~(x = h)) (FILTER (\x. ~(x = h')) (h::t)))`
+        by METIS_TAC [ALL_EL_FILTER] THEN
+    `LENGTH (FILTER (\x. ~(x = h)) (FILTER (\x. ~(x = h')) t)) <= L /\
+     LENGTH (FILTER (\x. ~(x = h)) (FILTER (\x. ~(x = h')) t')) <= L`
+        by (FULL_SIMP_TAC list_ss [] THEN
+            METIS_TAC [LENGTH_FILTER, LESS_EQ_TRANS]) THEN
+    `selParity w (FILTER (\x. ~(x = h)) (FILTER (\x. ~(x = h')) (h::t))) =
+     selParity w (FILTER (\x. ~(x = h)) (FILTER (\x. ~(x = h')) (h'::t')))`
+        by METIS_TAC [] THEN
+    `(selParity w (h::t) =
+        if countEven h' (h::t)
+        then selParity w (FILTER (\x. ~(x = h')) (h::t))
+        else boolXor (w ' h') (selParity w (FILTER (\x. ~(x = h')) (h::t)))) /\
+     (selParity w (h'::t') =
+        if countEven h' (h'::t')
+        then selParity w (FILTER (\x. ~(x = h')) (h'::t'))
+        else boolXor (w ' h') (selParity w (FILTER (\x. ~(x = h')) (h'::t'))))`
+        by METIS_TAC [selParity_filter] THEN
+     `(selParity w (FILTER (\x. ~(x = h')) (h::t)) =
+        if countEven h (FILTER (\x. ~(x = h')) (h::t))
+        then selParity w (FILTER (\x. ~(x = h)) (FILTER (\x. ~(x = h')) (h::t)))
+        else boolXor (w ' h) (selParity w
+               (FILTER (\x. ~(x = h)) (FILTER (\x. ~(x = h')) (h::t))))) /\
+      (selParity w (FILTER (\x. ~(x = h')) (h'::t')) =
+        if countEven h (FILTER (\x. ~(x = h')) (h'::t'))
+        then selParity w (FILTER (\x. ~(x = h))
+                            (FILTER (\x. ~(x = h')) (h'::t')))
+        else boolXor (w ' h) (selParity w
+               (FILTER (\x. ~(x = h)) (FILTER (\x. ~(x = h')) (h'::t')))))`
+        by METIS_TAC [selParity_filter] THEN
+      Cases_on `countEven h' (h::t)` THEN
+      Cases_on `countEven h (h::t)` THEN
+      Cases_on `countEven h' (h'::t')` THEN
+      Cases_on `countEven h (h'::t')` THEN
+      FULL_SIMP_TAC std_ss [] THEN
+      METIS_TAC []]);
+   
+val selParity_eq2 = Q.store_thm(
+ "selParity_eq2",
+  `!transL1 transL2 w.
+    ALL_EL (\x. x < 128) transL1 /\
+    ALL_EL (\x. x < 128) transL2 /\
+    (!j.
+        j <  128 
+        ==>
+        (countEven j transL1 = countEven j transL2 ))
+    ==>
+    (selParity w transL1 = selParity w transL2)`,
+ RW_TAC std_ss [] THEN
+ Cases_on `LENGTH transL1 < LENGTH transL2` THENL [
+    `LENGTH transL1 <=  LENGTH transL2` by RW_TAC arith_ss [] THEN
+    `LENGTH transL2 <=  LENGTH transL2` by RW_TAC arith_ss [] THEN
+    METIS_TAC [selParity_eq1],
+    `LENGTH transL1 <=  LENGTH transL1` by RW_TAC arith_ss [] THEN
+    `LENGTH transL2 <=  LENGTH transL1` by RW_TAC arith_ss [] THEN
+    METIS_TAC [selParity_eq1]]);
 
-(*desired properties of selParity*)	 
-val selParity_filter=Q.store_thm(
-"selParity_filter",
-`!i transL w.
-	i< word128$WL /\
-	ALL_EL (\x. x < word128$WL) transL 
-	==>
-	(selParity w transL 
-	 = if countEven i transL 
-	      then  selParity w (FILTER (\x. ~(x=i)) transL)
-	      else  boolXor (word128$WORD_BIT i w) 
-	                    (selParity w (FILTER (\x. ~(x =i)) transL)))`,
+(* given linear transformations cancel each other *)   
 
-Induct_on `transL` THENL [
-	METIS_TAC [FILTER,countEven_def],
-	RW_TAC std_ss [selParity_def,FILTER,countEven_def,ALL_EL] THENL [
-		`(selParity w transL 
-		  = (if countEven i transL 
-		        then selParity w (FILTER (\x. ~(x = i)) transL)
-			else boolXor (WORD_BIT i w) 
-			             (selParity w 
-				                (FILTER (\x. ~(x = i))
-						        transL))))` 
-			by METIS_TAC [] THEN
-		FULL_SIMP_TAC std_ss [boolXor_def],
-		`(selParity w transL 
-		  = (if countEven h transL 
-		        then selParity w (FILTER (\x. ~(x = h)) transL)
-			else boolXor (WORD_BIT h w) 
-			             (selParity w 
-				                (FILTER (\x. ~(x = h))
-						        transL))))` 
-			by METIS_TAC [] THEN
-		FULL_SIMP_TAC std_ss [boolXorAssoc,boolXorFacts,boolXorComm] THEN
-		METIS_TAC [boolXorAssoc,boolXorFacts,boolXorComm,boolXor_def],
-		`(selParity w transL 
-		  = (if countEven i transL 
-		        then selParity w (FILTER (\x. ~(x = i)) transL)
-			else boolXor (WORD_BIT i w) 
-			             (selParity w 
-				                (FILTER (\x. ~(x = i))
-						 transL))))` 
-			by METIS_TAC [] THEN
-		FULL_SIMP_TAC std_ss [boolXorAssoc,boolXorComm,boolXor_def] THEN
-		METIS_TAC [boolXorAssoc,boolXorFacts,boolXorComm,boolXor_def],	
-		`(selParity w transL 
-		  = (if countEven h transL 
-		        then selParity w (FILTER (\x. ~(x = h)) transL)
-			else boolXor (WORD_BIT h w) 
-			             (selParity w 
-				                (FILTER (\x. ~(x = h))
-						 transL))))` 
-			by METIS_TAC [] THEN
-		FULL_SIMP_TAC std_ss [boolXorAssoc,boolXorFacts,
-		                      boolXorComm,boolXor_def]]]);	
-		
+val invLT_LT_cancel = Q.store_thm(
+ "invLT_LT_cancel",
+ `!w. invLT (LT w) = w`,
+ SRW_TAC [fcpLib.FCP_ss]
+   [invLT_def,LT_def,transformComposeWord,LTFunInRange,invLTFunInRange] THEN
+ `w ' i = selParity w [i]` by RW_TAC std_ss [selParity_def,boolXor_def] THEN
+ FULL_SIMP_TAC arith_ss [transform_inv2_w128] THEN
+ `ALL_EL (\x. x < 128) (transCompose LTFun invLTFun i)`
+   by FULL_SIMP_TAC arith_ss [GSYM Res_def,transCompose_def] THENL [
+    `!i. i < 128 ==> ALL_EL (\x. x < 128) (Res i)`
+       by METIS_TAC [Res_fact] THEN
+    FULL_SIMP_TAC arith_ss [],
+    `ALL_EL (\x. x < 128) [i]` by RW_TAC list_ss [ALL_EL] THEN
+    RW_TAC arith_ss [LTFun_invLTFun_fact,selParity_eq2]]);   
 
-(*equivalence between two position list used in selParity*) 
-
-
-val selParity_eq1=Q.store_thm(
-"selParity_eq1",
-`!L transL1 transL2 w.
-	ALL_EL (\x. x < word128$WL) transL1 /\ 
-	ALL_EL (\x. x < word128$WL) transL2 /\
-	LENGTH transL1 <= L /\ 
-	LENGTH transL2 <= L /\
-	(!j. j <  word128$WL  ==>(countEven j transL1= countEven j transL2 )) 
-	==> 
-	( selParity w transL1  =selParity w transL2)`,
-
-Induct_on `L` THEN
-RW_TAC arith_ss [boolXor_def,countEven_def,selParity_def,LENGTH_NIL] THEN
-Cases_on `transL1` THEN Cases_on `transL2` THENL [
-	RW_TAC arith_ss [selParity_def],
-	`h < word128$WL` by FULL_SIMP_TAC list_ss [ALL_EL] THEN
-	`!j. 
-		j < word128$WL 
-		==> 
-		(countEven j (FILTER (\x. ~(x = h)) (h::t)) 
-		 = countEven j (h::t))` by RW_TAC std_ss [] THENL [
-		Cases_on `j=h` THEN
-		METIS_TAC [countEven_def, countEven_filter2,
-		           word128Theory.WL_def, DECIDE ``SUC x = x +1``],
-		`!j:num. countEven j []` by METIS_TAC [countEven_def] THEN
-		`!j. 
-			j < word128$WL 
-			==> 
-			countEven j (FILTER (\x. ~(x = h)) (h::t))` 
-			by METIS_TAC [] THEN
-		FULL_SIMP_TAC bool_ss [FILTER] THEN
-		`LENGTH (FILTER (\x. ~(x = h)) t)<=L` 
-			by FULL_SIMP_TAC list_ss [] THENL [
-			`LENGTH (FILTER (\x. ~(x = h)) t)<=LENGTH t` 
-				by FULL_SIMP_TAC list_ss [LENGTH_FILTER] THEN
-			FULL_SIMP_TAC arith_ss [],
-			`LENGTH ([]:num list)<=L` 
-				by RW_TAC arith_ss [LENGTH] THEN
-			`ALL_EL (\x. x < word128$WL) t` 
-				by FULL_SIMP_TAC list_ss [ALL_EL] THEN
-			`!j. 
-				j < word128$WL 
-				==> 
-				(countEven j [] 
-				 = countEven j (FILTER (\x. ~(x = h)) t) )`
-				 by METIS_TAC [] THEN
-			`ALL_EL (\x. x < word128$WL) (FILTER (\x. ~(x = h)) t)`
-				by METIS_TAC [ALL_EL_FILTER] THEN
-			`selParity w [] = selParity w  (FILTER (\x. ~(x = h)) t)`
-				by METIS_TAC [] THEN
-			`h < word128$WL` by FULL_SIMP_TAC std_ss [ALL_EL] THEN
-			`countEven h (h::t)` by METIS_TAC [] THEN
-			`~countEven h t` 
-				by FULL_SIMP_TAC std_ss
-				                 [countEven_def,boolXor_def] THEN
-			`selParity w t 
-			 = if countEven h t
-			      then selParity w (FILTER (\x. ~(x=h)) t) 
-			      else boolXor (word128$WORD_BIT h w) 
-			                   (selParity w 
-					              (FILTER (\x. ~(x =h)) t))`
-				by METIS_TAC [selParity_filter] THEN
-			FULL_SIMP_TAC std_ss [boolXor_def,selParity_def]]],
-	`h < word128$WL` by FULL_SIMP_TAC list_ss [ALL_EL] THEN
-	`!j. 
-		j < word128$WL 
-		==> 
-		(countEven j (FILTER (\x. ~(x = h)) (h::t)) 
-		 = countEven j (h::t))` by RW_TAC std_ss [] THENL [
-		Cases_on `j=h` THEN
-		METIS_TAC [countEven_def, countEven_filter2,word128Theory.WL_def,
-		           DECIDE ``SUC x = x +1``],
-		`!j:num. countEven j []` by METIS_TAC [countEven_def] THEN
-		`!j. 
-			j < word128$WL 
-			==> 
-			countEven j (FILTER (\x. ~(x = h)) (h::t))` 
-			by METIS_TAC [] THEN
-		FULL_SIMP_TAC bool_ss [FILTER] THEN
-		`LENGTH (FILTER (\x. ~(x = h)) t)<=L` 
-			by FULL_SIMP_TAC list_ss [] THENL [
-			`LENGTH (FILTER (\x. ~(x = h)) t)<=LENGTH t` 
-				by FULL_SIMP_TAC list_ss [LENGTH_FILTER] THEN
-			FULL_SIMP_TAC arith_ss [],
-			`LENGTH ([]:num list)<=L` by RW_TAC arith_ss [LENGTH] THEN
-			`ALL_EL (\x. x < word128$WL) t` 
-				by FULL_SIMP_TAC list_ss [ALL_EL] THEN
-			`!j. 
-				j < word128$WL 
-				==> 
-				(countEven j [] 
-				 = countEven j (FILTER (\x. ~(x = h)) t))`
-				 by METIS_TAC [] THEN
-			`ALL_EL (\x. x < word128$WL) (FILTER (\x. ~(x = h)) t)`
-				by METIS_TAC [ALL_EL_FILTER] THEN
-			`selParity w [] = selParity w (FILTER (\x. ~(x = h)) t)`
-				by METIS_TAC [] THEN
-			`h < word128$WL` by FULL_SIMP_TAC std_ss [ALL_EL] THEN
-			`countEven h (h::t)` by METIS_TAC [] THEN
-			`~countEven h t` 
-				by FULL_SIMP_TAC std_ss
-					         [countEven_def,boolXor_def] THEN
-			`selParity w t 
-			 = if countEven h t 
-			      then selParity w (FILTER (\x. ~(x=h)) t)
-			      else boolXor (word128$WORD_BIT h w) 
-			                   (selParity w 
-					              (FILTER (\x. ~(x =h)) t))` 
-				by METIS_TAC [selParity_filter] THEN
-			FULL_SIMP_TAC std_ss [boolXor_def,selParity_def]]],
-		
-	`(h < word128$WL) /\ (h' < word128$WL)` 
-		by FULL_SIMP_TAC std_ss [ALL_EL] THEN
-	`!j. 
-		j < word128$WL 
-		==> 
-		(countEven j (FILTER (\x. ~(x = h')) (h::t)) 
-		 = countEven j (FILTER (\x. ~(x = h')) (h'::t')))` 
-		 by METIS_TAC [countEven_filter3,word128Theory.WL_def,
-		               DECIDE ``SUC x = x +1``] THEN
-	`ALL_EL (\x. x < word128$WL) (FILTER (\x. ~(x = h')) (h::t))` 
-		by METIS_TAC [ALL_EL_FILTER] THEN
-	`ALL_EL (\x. x < word128$WL) (FILTER (\x. ~(x = h')) (h'::t'))`
-		by METIS_TAC [ALL_EL_FILTER] THEN 
-	`LENGTH (FILTER (\x. ~(x = h')) (h::t))<=LENGTH (h::t)` 
-		by FULL_SIMP_TAC arith_ss [LENGTH_FILTER] THEN
-	`LENGTH (FILTER (\x. ~(x = h')) (h::t)) <=SUC L` 
-		by FULL_SIMP_TAC arith_ss [] THEN
-	`LENGTH (FILTER (\x. ~(x = h')) (h'::t'))<=LENGTH (h'::t')` 
-		by FULL_SIMP_TAC arith_ss [LENGTH_FILTER] THEN
-	`LENGTH (FILTER (\x. ~(x = h')) (h'::t')) <=SUC L` 
-		by FULL_SIMP_TAC arith_ss [] THEN
-	`!j. 
-		j < word128$WL 
-		==> 
-		(countEven j (FILTER (\x. ~(x = h)) 
-		                     (FILTER (\x. ~(x = h')) (h::t))) 
-		 = countEven j (FILTER (\x. ~(x = h))
-		                       (FILTER (\x. ~(x = h')) (h'::t'))))` 
-		by METIS_TAC [countEven_filter3,word128Theory.WL_def,
-		              DECIDE ``SUC x = x +1``] THEN
-	`FILTER (\x. ~(x = h)) (FILTER (\x. ~(x = h')) (h::t))
-	 = FILTER (\x. ~(x = h)) (FILTER (\x. ~(x = h')) t)` 
-	 	by  RW_TAC list_ss [FILTER_COMM,FILTER] THEN
-	`FILTER (\x. ~(x = h)) (FILTER (\x. ~(x = h')) (h'::t'))
-	 = FILTER (\x. ~(x = h)) (FILTER (\x. ~(x = h')) t')` 
-		 by  RW_TAC list_ss [FILTER] THEN
-	`ALL_EL (\x. x < word128$WL) 
-	        (FILTER (\x. ~(x = h)) (FILTER (\x. ~(x = h')) (h'::t')))` 
-		by METIS_TAC [ALL_EL_FILTER] THEN
-	`ALL_EL (\x. x < word128$WL) 
-	        (FILTER (\x. ~(x = h)) (FILTER (\x. ~(x = h')) (h::t)))`
-		by METIS_TAC [ALL_EL_FILTER] THEN
-	`LENGTH ( FILTER (\x. ~(x = h)) (FILTER (\x. ~(x = h')) t)) <= L`
-		by FULL_SIMP_TAC list_ss [] THENL [
-		`LENGTH (FILTER (\x. ~(x = h)) 
-		                (FILTER (\x. ~(x = h')) t)) 
-		 <= LENGTH (FILTER (\x. ~(x = h')) t)` 
-			by METIS_TAC [LENGTH_FILTER] THEN
-		`LENGTH (FILTER (\x. ~(x = h')) t) <= LENGTH t` 
-			by METIS_TAC [LENGTH_FILTER] THEN
-		METIS_TAC [LESS_EQ_TRANS],
-		`LENGTH ( FILTER (\x. ~(x = h)) 
-		                 (FILTER (\x. ~(x = h')) t')) 
-		 <= L` by FULL_SIMP_TAC list_ss [] THENL [
-			`LENGTH (FILTER (\x. ~(x = h)) 
-			                (FILTER (\x. ~(x = h')) t')) 
-			 <= LENGTH (FILTER (\x. ~(x = h')) t')` 
-				by METIS_TAC [LENGTH_FILTER] THEN
-			`LENGTH (FILTER (\x. ~(x = h')) t') 
-			 <= LENGTH t'` by METIS_TAC [LENGTH_FILTER] THEN
-			METIS_TAC [LESS_EQ_TRANS],
-			`selParity w 
-			           (FILTER (\x. ~(x = h)) 
-				           (FILTER (\x. ~(x = h')) (h::t))) 
-			 = selParity w 
-				     (FILTER (\x. ~(x = h)) 
-				             (FILTER (\x. ~(x = h')) (h'::t')))` 
-				by METIS_TAC [] THEN
-			`selParity w (h::t) 
-			 = if countEven h' (h::t) 
-			      then selParity w 
-			                     (FILTER (\x. ~(x=h')) (h::t)) 
-			      else boolXor (word128$WORD_BIT h' w)
-				           (selParity w 
-					              (FILTER (\x. ~(x =h'))
-						              (h::t)))` 
-				by METIS_TAC [selParity_filter] THEN
-			`selParity w (h'::t') 
-			 = if countEven h' (h'::t') 
-			      then selParity w (FILTER (\x. ~(x=h')) (h'::t'))
-			      else  boolXor (word128$WORD_BIT h' w) 
-			                    (selParity w 
-					               (FILTER (\x. ~(x =h'))
-						               (h'::t')))` 
-				by METIS_TAC [selParity_filter] THEN
-			`selParity w (FILTER (\x. ~(x=h')) (h::t)) 
-			 = if countEven h (FILTER (\x. ~(x=h')) (h::t)) 
-			      then selParity w 
-			           (FILTER (\x. ~(x=h)) 
-				           (FILTER (\x. ~(x=h')) (h::t)))
-			      else  boolXor (word128$WORD_BIT h w) 
-			                    (selParity w 
-					               (FILTER (\x. ~(x =h))
-						               (FILTER (\x. ~(x=h'))
-							               (h::t))))` 
-				by METIS_TAC [selParity_filter] THEN
-			`selParity w (FILTER (\x. ~(x=h')) (h'::t')) 
-			 = if countEven h (FILTER (\x. ~(x=h')) (h'::t')) 
-			      then selParity w 
-			                     (FILTER (\x. ~(x=h)) 
-					             (FILTER (\x. ~(x=h')) (h'::t')))
-			      else  boolXor (word128$WORD_BIT h w) 
-			                    (selParity w 
-					               (FILTER (\x. ~(x =h)) 
-						               (FILTER (\x. ~(x=h'))
-							               (h'::t'))))`
-				by METIS_TAC [selParity_filter] THEN
-			Cases_on `countEven h' (h::t)` THEN 
-			Cases_on `countEven h (h::t)` THEN 
-			Cases_on `countEven h' (h'::t')` THEN 
-			Cases_on `countEven h (h'::t')` THENL [
-				FULL_SIMP_TAC std_ss [],
-				FULL_SIMP_TAC std_ss [],
-				METIS_TAC [],
-				METIS_TAC [],
-				METIS_TAC [],
-				FULL_SIMP_TAC std_ss [],
-				METIS_TAC [],
-				METIS_TAC [],
-				METIS_TAC [],
-				METIS_TAC [],
-				FULL_SIMP_TAC std_ss [],
-				METIS_TAC [],
-				METIS_TAC [],
-				METIS_TAC [],
-				METIS_TAC [],
-				FULL_SIMP_TAC std_ss []]]]]);
-		       
-	
-	
-val selParity_eq2=Q.store_thm(
-"selParity_eq2",
-`!transL1 transL2 w.
-	ALL_EL (\x. x < word128$WL) transL1 /\ 
-	ALL_EL (\x. x < word128$WL) transL2 /\
-	(!j. 
-		j <  word128$WL  
-		==>
-		(countEven j transL1= countEven j transL2 )) 
-	==> 
-	(selParity w transL1  =selParity w transL2)`,
-	
-RW_TAC std_ss [] THEN
-Cases_on `LENGTH transL1 < LENGTH transL2` THENL [
-	`LENGTH transL1 <=  LENGTH transL2` by RW_TAC arith_ss [] THEN
-	`LENGTH transL2 <=  LENGTH transL2` by RW_TAC arith_ss [] THEN
-	METIS_TAC [selParity_eq1],
-	`LENGTH transL1 <=  LENGTH transL1` by RW_TAC arith_ss [] THEN
-	`LENGTH transL2 <=  LENGTH transL1` by RW_TAC arith_ss [] THEN
-	METIS_TAC [selParity_eq1]]);
-	
-
-(*given linear transformations cancel each other*)	
-val invLT_LT_cancel=Q.store_thm(
-"invLT_LT_cancel",
-`!w.
-	invLT (LT w) = w `,
-
-
-RW_TAC std_ss [GSYM WORD_EQ,invLT_def,LT_def,transformComposeWord,
-               LTFunInRange,invLTFunInRange] THEN
-`WORD_BIT x w= selParity w [x]` by RW_TAC std_ss [selParity_def,boolXor_def] THEN
-FULL_SIMP_TAC arith_ss [transform_inv2_w128,word128Theory.HB_def,
-                        word128Theory.WL_def] THEN
-`ALL_EL (\x. x < word128$WL) (transCompose LTFun invLTFun x)` 
-	by FULL_SIMP_TAC arith_ss [GSYM Res_def,transCompose_def,
-	                           word128Theory.WL_def,word128Theory.HB_def] THENL [
-	`!i.
-		i < word128$WL
-		==>
-		ALL_EL (\x. x < word128$WL) (Res i)` 
-		by METIS_TAC [Res_fact] THEN
-	FULL_SIMP_TAC arith_ss [word128Theory.WL_def,word128Theory.HB_def],
-	 `ALL_EL (\x. x < word128$WL) [x]` 
-	 	by RW_TAC list_ss [ALL_EL,word128Theory.WL_def,
-		                   word128Theory.HB_def] THEN
-	  RW_TAC arith_ss [LTFun_invLTFun_fact,selParity_eq2,
-	                   word128Theory.WL_def,word128Theory.HB_def]]);	
-
-
-
-val _ = export_theory();	
+val _ = export_theory();   
