examples/Crypto/Serpent/Reference/Serpent_Reference_UtilityScript.sml
@@ -1,593 +1,445 @@
-open HolKernel Parse boolLib bossLib listTheory rich_listTheory bitsTheory
-     markerTheory metisLib pairTheory arithmeticTheory word4Theory 
-     word8Theory word32Theory word128Theory word256Theory 
-     word4Lib word8Lib word32Lib word128Lib word256Lib metisLib;
+open HolKernel Parse boolLib bossLib listTheory rich_listTheory bitTheory
+     markerTheory pairTheory arithmeticTheory wordsTheory wordsLib;
 
 val _ = new_theory "Serpent_Reference_Utility";
 
-(*trivial stuff about word128 *)
-val bit_num_val_bound=Q.store_thm(
-"bit_num_val_bound",
-`!w n.
-	BIT n w ==> w >= 2 ** n`,
-		
-RW_TAC arith_ss [BIT_def, BITS_THM] THEN
-CCONTR_TAC THEN
-FULL_SIMP_TAC arith_ss [DECIDE ``SUC n - n = 1n``, DECIDE``~(x >= y) = x<y:num``,
-                        LESS_DIV_EQ_ZERO]
-); 
+(* XOR *)
 
-val w2n_zero128 = Q.store_thm (
-"w2n_zero128",
-`word128$w2n 0w= 0`,
+val boolXor_def = Define `boolXor (x:bool) y = ~(x= y)`;
 
-EVAL_TAC);
-			
-val w2n_one128 = Q.store_thm ( 
-"w2n_one128", 
-`(w2n:word128->num) 1w= 1`,
-			
-EVAL_TAC); 			
+val boolXorComm = Q.store_thm(
+ "boolXorComm",
+ `!x y. boolXor x y = boolXor y x`,
+ METIS_TAC [boolXor_def]);
 
-val word_1_bit_0=Q.store_thm(
-"word_1_bit_0",
-`word128$WORD_BIT 0 (1w:word128)`,
+val boolXorAssoc = Q.store_thm(
+ "boolXorAssoc",
+ `!x y z. boolXor z (boolXor x y) = boolXor (boolXor z x) y`,
+ METIS_TAC [boolXor_def]);
 
-EVAL_TAC);
-
-
-val word_1_bit128=Q.store_thm(
-"word_1_bit128",
-`!n.
-	n>0 /\
-	n< word128$WL
-	==>
-	 ~(word128$WORD_BIT n (1w:word128))`,
-		
-CCONTR_TAC THEN
-FULL_SIMP_TAC bool_ss [word128Theory.WORD_BIT_def] THEN
-`word128$w2n 1w= 1` by METIS_TAC [w2n_one128] THEN
-`1 >=2**n` by METIS_TAC [bit_num_val_bound] THEN
-`~(2 ** n=0)` by FULL_SIMP_TAC arith_ss [TWOEXP_NOT_ZERO] THEN
-`2**n=1` by RW_TAC arith_ss [] THEN
-`(2=1) \/ (n=0)` by METIS_TAC [EXP_EQ_1] THEN 
-FULL_SIMP_TAC arith_ss []
-);     
-
-
-(*XOR
-*)
-val boolXor_def= Define
-`boolXor (x:bool) y = ~(x=y)`;
-
-val boolXorComm=Q.store_thm(
-"boolXorComm",
-` !x y. 
-	boolXor x y = boolXor y x`,
-
-METIS_TAC [boolXor_def]);
-
-val boolXorAssoc=Q.store_thm(
-"boolXorAssoc",
-` !x y z. 
-	boolXor z (boolXor x y) = boolXor (boolXor z x) y`,
-
-METIS_TAC [boolXor_def]);
-
-val boolXorFacts=Q.store_thm(
-"boolXorFacts",
-`(!x.(boolXor x x) = F) /\
+val boolXorFacts = Q.store_thm(
+ "boolXorFacts",
+ `(!x.(boolXor x x) = F) /\
   (!x.(boolXor x T) = ~x) /\
   (!x.(boolXor x F) = x) `,
+ METIS_TAC [boolXor_def]);
 
-METIS_TAC [boolXor_def]);
+val boolXorComm3 = Q.store_thm(
+ "boolXorComm3",
+ `!x y z. boolXor x (boolXor y z) = boolXor y (boolXor x z)`,
+  Cases_on `x` THEN Cases_on `y` THEN Cases_on `z` THEN
+  RW_TAC std_ss [boolXor_def]);
 
-val boolXorComm3=Q.store_thm(
-"boolXorComm3",
-`! x y z. 
-	boolXor x (boolXor y z) = boolXor y (boolXor x z)`,
+(* trivial stuff about list *)
 
-Cases_on `x` THEN Cases_on `y` THEN Cases_on `z` THEN
-RW_TAC std_ss [boolXor_def]);
-	
-(*trivial stuff about list
-*)	
-val ALL_EL_FILTER=Q.store_thm(
-"ALL_EL_FILTER",
-`!p q l. 
-	ALL_EL p l
-	==> 
-	ALL_EL p (FILTER q l)`,
+val ALL_EL_FILTER = Q.store_thm(
+ "ALL_EL_FILTER",
+ `!p q l.
+    ALL_EL p l
+    ==>
+    ALL_EL p (FILTER q l)`,
+ Induct_on `l` THEN RW_TAC list_ss []);
 
-Induct_on `l` THEN
-RW_TAC list_ss []);	
-	
-val LENGTH_NIL_LEQ =Q.store_thm(
-"LENGTH_NIL_LEQ",
-`!n. 
-	LENGTH [] <= n`,
+val LENGTH_NIL_LEQ = Q.store_thm(
+ "LENGTH_NIL_LEQ",
+ `!n. LENGTH [] <= n`,
+ RW_TAC list_ss []);
 
-RW_TAC list_ss []);
-	  
-val LENGTH_FILTER=Q.store_thm(
-"LENGTH_FILTER",
-`!l p. 
-	LENGTH (FILTER p l) <= LENGTH l`,
+val LENGTH_FILTER = Q.store_thm(
+ "LENGTH_FILTER",
+ `!l p. LENGTH (FILTER p l) <= LENGTH l`,
+ Induct_on `l` THEN
+ RW_TAC list_ss [] THEN
+ `LENGTH l <=  SUC (LENGTH l)` by RW_TAC arith_ss [] THEN
+ METIS_TAC [LESS_EQ_TRANS]);
 
-Induct_on `l` THEN 
-RW_TAC list_ss [] THEN 
-`LENGTH l <=  SUC (LENGTH l)` by RW_TAC arith_ss [] THEN
-METIS_TAC [LESS_EQ_TRANS]);
-	
-	
-(*make a list of "T" of length n*)
-val makeTL_def =Define
-`(makeTL 0 =  []) /\
+(* make a list of "T" of length n*)
 
+val makeTL_def = Define`
+ (makeTL 0 =  []) /\
  (makeTL (SUC n) = T::(makeTL n))`;
 
 val LENGTH_makeTL = Q.store_thm(
-"LENGTH_makeTL",
-`!n.
-	LENGTH (makeTL n) = n`,
-	
-Induct_on `n` THENL [
-	RW_TAC list_ss [makeTL_def],
-	RW_TAC list_ss [makeTL_def]]);
-	
+ "LENGTH_makeTL",
+ `!n. LENGTH (makeTL n) = n`,
+ Induct_on `n` THEN RW_TAC list_ss [makeTL_def]);
 
-val makeTL_fact=Q.store_thm(
-"makeTL_fact",
-`!i n. 
-	i<n
-	==>
-	EL i (makeTL n)`,
+val makeTL_fact = Q.store_thm(
+ "makeTL_fact",
+ `!i n.
+    i<n
+    ==>
+    EL i (makeTL n)`,
+ Induct_on `n` THENL [
+   RW_TAC arith_ss [],
+   Cases_on `i` THEN
+   RW_TAC list_ss [makeTL_def]]);
 
-Induct_on `n` THENL [
-	RW_TAC arith_ss [],
-	Cases_on `i` THEN
-	RW_TAC list_ss [makeTL_def]]);		
+(* XOR on bool lists in ZIP fashion *)
 
-(*XOR on bool lists in ZIP fashion
-*)		
-val zipXor_def =Define 
-`(zipXor [] l =l) /\
+val zipXor_def = Define`
+ (zipXor [] l = l) /\
+ (zipXor (xh::xt) (ah::at) = (boolXor xh ah)::zipXor xt at)   /\
+ (zipXor (xh::xt) [] = [])`;
 
-(zipXor (xh::xt) (ah::at) = (boolXor xh ah)::zipXor xt at)   /\
-(zipXor (xh::xt) [] = [])`;
+val zipXor_fact = Q.store_thm(
+ "zipXor_fact",
+ `!l. zipXor l [] = [] `,
+ Cases_on `l` THEN
+ RW_TAC list_ss [zipXor_def]);
 
-val zipXor_fact=Q.store_thm(
-"zipXor_fact",
-`!l. 
-	zipXor l [] = [] `,
+val LENGTH_zipXor = Q.store_thm(
+ "LENGTH_zipXor",
+ `!l1 l2. LENGTH (zipXor l1 l2) = LENGTH l2`,
+ Induct_on `l2` THENL [
+   Cases_on `l1` THEN
+   RW_TAC list_ss [zipXor_def],
+   Cases_on `l1` THEN
+   RW_TAC list_ss [zipXor_def]]);
 
-Cases_on `l` THEN
-RW_TAC list_ss [zipXor_def]);
-	
-val LENGTH_zipXor=Q.store_thm(
-"LENGTH_zipXor",
-`!l1 l2.
-	LENGTH (zipXor l1 l2) = LENGTH l2`,
+val makeL_def = Define`
+ (makeL 0 = [T]) /\
+ (makeL (SUC n) = F::makeL n)`;
 
-Induct_on `l2` THENL [
-	Cases_on `l1` THEN
-	RW_TAC list_ss [zipXor_def],
-	Cases_on `l1` THEN
-	RW_TAC list_ss [zipXor_def]]);
+val zipXor_makeL_COMM = Q.store_thm(
+ "zipXor_makeL_COMM",
+ `!i n1 n2 l.
+     zipXor (makeL n2) (zipXor (makeL n1) al) =
+     zipXor (makeL n1) (zipXor (makeL n2) al)`,
+ Induct_on `al` THENL [
+   RW_TAC list_ss [zipXor_fact],
+   Cases_on `n1` THEN Cases_on `n2` THEN
+   RW_TAC list_ss [makeL_def,zipXor_def,boolXor_def]]);
 
+val zipXor_makeL = Q.store_thm(
+ "zipXor_makeL",
+ `!i al h tl.
+    i < LENGTH al  /\
+    h < LENGTH al
+    ==>
+    (EL i (zipXor (makeL h) al) = boolXor (i = h) (EL i al))`,
+ Induct_on `h` THENL [
+   RW_TAC list_ss [zipXor_def,makeL_def] THEN
+   Cases_on `al` THEN
+   FULL_SIMP_TAC list_ss [zipXor_def,boolXor_def] THEN
+   Cases_on `i` THEN
+   RW_TAC list_ss [],
+   RW_TAC list_ss [makeL_def] THEN
+   Cases_on `al` THEN
+   RW_TAC list_ss [zipXor_def,boolXor_def] THEN
+   Cases_on `i` THEN
+   FULL_SIMP_TAC list_ss [boolXor_def]]);
 
-	  
-val makeL_def=Define
-`(makeL 0 = [T]) /\
-(makeL (SUC n) = F::makeL n)`;
+val MAP_ID = Q.store_thm(
+ "MAP_ID",
+ `!l f.
+    ALL_EL (\x. f x = x) l
+    ==>
+    (MAP f l = l)`,
+ Induct_on `l` THEN
+ RW_TAC list_ss []);
 
+(* housemade FIRSTN and BUTLASTN for easy evaluation*)
 
-val zipXor_makeL_COMM=Q.store_thm(
-"zipXor_makeL_COMM",
-`! i n1 n2 l.
-	 zipXor (makeL n2) (zipXor (makeL n1) al)
-	 = zipXor (makeL n1) (zipXor (makeL n2) al)`,
-	 
-Induct_on `al` THENL [
-	RW_TAC list_ss [zipXor_fact],
-	Cases_on `n1` THEN Cases_on `n2` THEN
-	RW_TAC list_ss [makeL_def,zipXor_def,boolXor_def]]);		
-		
-val zipXor_makeL=Q.store_thm(
-"zipXor_makeL",
- `!i al h tl. 
-	i < LENGTH al  /\
-	h < LENGTH al  
-	==>
-	(EL i (zipXor (makeL h) al) = boolXor (i=h) (EL i al))`,
-	
-Induct_on `h` THENL [
-	RW_TAC list_ss [zipXor_def,makeL_def] THEN
-	Cases_on `al` THEN 
-	FULL_SIMP_TAC list_ss [zipXor_def,boolXor_def] THEN
-	Cases_on `i` THEN
-	RW_TAC list_ss [],
-	RW_TAC list_ss [makeL_def] THEN
-	Cases_on `al` THEN
-	RW_TAC list_ss [zipXor_def,boolXor_def] THEN
-	Cases_on `i` THEN
-	FULL_SIMP_TAC list_ss [boolXor_def]]);					
-
-		
-		
-val MAP_ID=Q.store_thm(
-"MAP_ID",
-`!l f. 
-	ALL_EL (\x. f x =x) l
-	==>
-	(MAP f l=l)`, 
-	
-Induct_on `l` THEN
-RW_TAC list_ss []);
-	  		
-(*housemade FIRSTN and BUTLASTN for easy evaluation*)
-val (myFIRSTN_def,myFIRSTN_termi) =Defn.tstore_defn(
+val (myFIRSTN_def,myFIRSTN_termi) = Defn.tstore_defn(
  Defn.Hol_defn "myFIRSTN"
-`myFIRSTN n l = if n=0 then []
-else if l=[] then []
-else (HD l)::(myFIRSTN (n-1) (TL l))`,
+ `myFIRSTN n l =
+    if n = 0 then []
+    else if l =[] then []
+    else (HD l)::(myFIRSTN (n-1) (TL l))`,
+ WF_REL_TAC `measure (LENGTH o SND)` THEN
+ RW_TAC list_ss [] THEN
+ Cases_on `l` THENL [
+   FULL_SIMP_TAC list_ss [],
+   RW_TAC list_ss []]);
 
-WF_REL_TAC `measure (LENGTH o SND)` THEN
-RW_TAC list_ss [] THEN
-Cases_on `l` THENL [
-	FULL_SIMP_TAC list_ss [],
-	RW_TAC list_ss []]);
+val myBUTLASTN_def = Define`
+ myBUTLASTN n l = let len = LENGTH l in
+   if len>= n then myFIRSTN (LENGTH l-n) l
+   else []`;
 
-val myBUTLASTN_def = Define
-`myBUTLASTN n l = let len=LENGTH l in
-if len>=n then myFIRSTN (LENGTH l-n) l
-else []
-`;
+val LENGTH_myFIRSTN = Q.store_thm(
+ "LENGTH_myFIRSTN",
+ `!n l.
+    n <= LENGTH l
+    ==>
+    (LENGTH (myFIRSTN n l) = n)`,
+ Induct_on `n` THENL [
+   RW_TAC list_ss [] THEN
+   `myFIRSTN 0 l =[]` by METIS_TAC  [myFIRSTN_def] THEN
+   RW_TAC list_ss [],
+   RW_TAC list_ss [] THEN
+   Cases_on `l` THENL [
+     FULL_SIMP_TAC list_ss [],
+     `~(SUC n = 0)` by RW_TAC arith_ss [] THEN
+     `~((h::t) =[])` by RW_TAC list_ss [] THEN
+     `myFIRSTN (SUC n) (h::t)= (HD (h::t))::(myFIRSTN (SUC n-1) (TL (h::t)))`
+      by  METIS_TAC  [myFIRSTN_def] THEN
+      FULL_SIMP_TAC list_ss []]]);
 
-val LENGTH_myFIRSTN=Q.store_thm(
-"LENGTH_myFIRSTN",
-`!n l. 
-	n <= LENGTH l 
-	==> 
-	(LENGTH (myFIRSTN n l) = n)`,
-
-Induct_on `n` THENL [
-	RW_TAC list_ss [] THEN
-	`myFIRSTN 0 l=[]` by METIS_TAC  [myFIRSTN_def] THEN
-	RW_TAC list_ss [],
-	RW_TAC list_ss [] THEN
-	Cases_on `l` THENL [
-		FULL_SIMP_TAC list_ss [],
-		`~(SUC n=0)` by RW_TAC arith_ss [] THEN
-		`~((h::t) =[])` by RW_TAC list_ss [] THEN
-		`myFIRSTN (SUC n) (h::t)= (HD (h::t))::(myFIRSTN (SUC n-1) (TL (h::t)))` by  METIS_TAC  [myFIRSTN_def] THEN
-		FULL_SIMP_TAC list_ss []]]);
-	
-
-
-
-val LENGTH_myBUTLASTN=Q.store_thm(
-"LENGTH_myBUTLASTN",
-`!n l. 
-	n <= LENGTH l 
-	==> 
-	(LENGTH (myBUTLASTN n l) = LENGTH l - n)`,
-
-RW_TAC arith_ss [myBUTLASTN_def,LENGTH_myFIRSTN,LET_THM]);	
-	   
-	
-		
-
-(*conversion between different words,
-EL 0 is the MS in all split result,
-the bit ordering is perserved
-*)
-
-val word128to32l_def =Define 
-`word128to32l (w128:word128) = 
- [word32$n2w (w2n (w128 >>> 96)); word32$n2w (w2n ((w128 <<32) >>> 96));
-  word32$n2w (w2n ((w128<<64) >>> 96)); word32$n2w (w2n ((w128<<96) >>> 96))]`;
-
-val word32to8l_def =Define 
-`word32to8l (w32:word32) = 
- [word8$n2w (w2n (w32 >>> 24)); word8$n2w (w2n ((w32 <<8) >>> 24));
-  word8$n2w (w2n ((w32<<16) >>> 24)); word8$n2w (w2n ((w32<<24) >>> 24))]`;
+val LENGTH_myBUTLASTN = Q.store_thm(
+ "LENGTH_myBUTLASTN",
+ `!n l.
+    n <= LENGTH l
+    ==>
+    (LENGTH (myBUTLASTN n l) = LENGTH l - n)`,
+ RW_TAC arith_ss [myBUTLASTN_def,LENGTH_myFIRSTN,LET_THM]);
 
 
-val word8to4l_def =Define 
-`word8to4l(w8:word8) = 
- [word4$n2w (w2n (w8 >>> 4)); word4$n2w (w2n ((w8 <<4) >>> 4))]`;
+(* conversion between different words, EL 0 is the MS in all split result,
+   the bit ordering is perserved *)
 
-val word32to4l_def=Define
-`word32to4l w32= FLAT (MAP word8to4l (word32to8l w32))`;
+val _ = wordsLib.guess_lengths();
+val _ = wordsLib.mk_word_size 128;
+val _ = wordsLib.mk_word_size 256;
 
-val word4to32_def = Define
-`word4to32 (w4:word4)= word32$n2w (w2n w4)`;
+val word128to32l_def = Define`
+ word128to32l (w:word128) =
+ [(127 >< 96) w; (95 >< 64) w; (63 >< 32) w; (31 >< 0) w]`;
 
-val word4to128_def = Define
-`word4to128 (w4:word4)= word128$n2w (w2n w4)`;
+val word32to8l_def = Define`
+ word32to8l (w:word32) =
+ [(31 >< 24) w; (23 >< 16) w; (15 >< 8) w; (7 >< 0) w]`;
 
-val word32to128_def = Define
- `word32to128 (w32:word32)= word128$n2w (w2n w32)`;
+val word8to4l_def = Define`
+ word8to4l(w:word8) =
+ [(7 >< 4) w; (3 >< 0) w]`;
 
-val word256to128l = Define
-`word256to128l (w256:word256) = 
- [word128$n2w (w2n (w256 >>> 128)); word128$n2w  (w2n ((w256 <<128) >>> 128))]`;
+val word32to4l_def = Define`
+ word32to4l w = FLAT (MAP word8to4l (word32to8l w))`;
 
-val word256to32l_def = Define
-`word256to32l (w256:word256) = FLAT ( MAP word128to32l (word256to128l w256))`;
- (*input is in MSNibble....LSNibble
-in each Nibble, MSBit..LSBit
-input is of 32 nibbles
-*)
+val word4to32_def = Define `word4to32 = w2w:word4->word32`;
+val word4to128_def = Define `word4to128 = w2w:word4->word128`;
+val word32to128_def = Define `word32to128 = w2w:word32->word128`;
 
-(*convert a word4 list to a num
-LSW,,,,,MSW*)
-val revWord4ltoNum_def=Define
-`(revWord4ltoNum [] = 0) /\
-(revWord4ltoNum (h::t) = (word4$w2n h+ (revWord4ltoNum t)*16))`;
+val word256to128l = Define`
+ word256to128l (w:word256) =
+ [(255 >< 128) w; (127 >< 0) w]`;
 
+val word256to32l_def = Define`
+ word256to32l (w:word256) = FLAT (MAP word128to32l (word256to128l w))`;
 
-(*convert a num to a word4 list,
-the length of list is controled by a parameter,
-the length provides a MOD 
-LSW,,,,,MSW*)
-val numtoRevWord4l_def =Define
-`(numtoRevWord4l 0 n = []) /\
-(numtoRevWord4l (SUC m) n = word4$n2w (  n MOD 16)::(numtoRevWord4l m (n DIV 16)))`;
+(* input is in MSNibble....LSNibble in each Nibble, MSBit..LSBit input is
+   of 32 nibbles *)
 
-val numtoRevWord4lEval=Q.store_thm(
-"numtoRevWord4lEval",
-`!n m. 
-	numtoRevWord4l m n =
-	if m=0 then []
-	else  word4$n2w (  n MOD 16)::(numtoRevWord4l (m-1) (n DIV 16))`,
+(* convert a word4 list to a num LSW,,,,,MSW *)
 
+val revWord4ltoNum_def = Define`
+ (revWord4ltoNum ([]:word4 list) = 0) /\
+ (revWord4ltoNum (h::t) = (w2n h + (revWord4ltoNum t) * 16))`;
 
-RW_TAC arith_ss [numtoRevWord4l_def] THEN
-Cases_on `m` THENL [
-	METIS_TAC [],
-	FULL_SIMP_TAC arith_ss [numtoRevWord4l_def]]);
-	
+(* convert a num to a word4 list, the length of list is controled by a
+   parameter, the length provides a MOD LSW,,,,,MSW *)
 
-(*the length provides a MOD *)
-val revWord4ltoNumRange=Q.store_thm(
-"revWord4ltoNumRange",
-`!n l. 
-	LENGTH l <= n ==> revWord4ltoNum l < 2 ** (4*n)`,
-	
-Induct_on `l` THENL [
-	METIS_TAC [ revWord4ltoNum_def,ZERO_LESS_EXP,DECIDE ``2 = SUC 1``],
-	RW_TAC list_ss [ revWord4ltoNum_def] THEN
-	Cases_on `n` THENL [
-		FULL_SIMP_TAC arith_ss [],
-		`4* SUC n'=4+ 4*n'` by RW_TAC arith_ss [] THEN
-		`word4$w2n h < 2**word4$WL` by METIS_TAC  [word4Theory.w2n_LT] THEN
-		FULL_SIMP_TAC std_ss [EXP_ADD,word4Theory.WL_def,word4Theory.HB_def] THEN
-		FULL_SIMP_TAC list_ss [] THEN
-		`revWord4ltoNum  l < 2 ** (4 * n') ` by METIS_TAC [] THEN
-		`SUC ( revWord4ltoNum l) <= 2 ** (4 * n')` by METIS_TAC [LESS_EQ] THEN
-		`16+16* (revWord4ltoNum l)<= 16*2 ** (4 * n')` by RW_TAC arith_ss [] THEN
-		FULL_SIMP_TAC arith_ss []]]);
-		
-val LENGTH_numtoRevWord4l=Q.store_thm(
-"LENGTH_numtoRevWord4l",
-`!wl n. 
-	LENGTH (numtoRevWord4l n wl) =n`,
+val numtoRevWord4l_def = Define`
+ (numtoRevWord4l 0 n = [] : word4 list) /\
+ (numtoRevWord4l (SUC m) n = n2w (n MOD 16)::(numtoRevWord4l m (n DIV 16)))`;
 
-Induct_on `n` THEN
-RW_TAC list_ss [numtoRevWord4l_def]);
-	
-	
+val numtoRevWord4lEval = Q.store_thm(
+ "numtoRevWord4lEval",
+ `!n m.
+    numtoRevWord4l m n =
+    if m = 0 then []
+    else n2w (n MOD 16)::(numtoRevWord4l (m-1) (n DIV 16))`,
+ RW_TAC arith_ss [numtoRevWord4l_def] THEN
+ Cases_on `m` THENL [
+   METIS_TAC [],
+   FULL_SIMP_TAC arith_ss [numtoRevWord4l_def]]);
 
-	  
-(*the conversions between a num and word4 list are reversible*)        
-val numtoRevWord4l_conversion=Q.store_thm(
-"numtoRevWord4l_conversion",
-`!n wl. 
-	(n=LENGTH wl)
-	==>
-	( numtoRevWord4l n (revWord4ltoNum wl) =wl)`,
+(* the length provides a MOD *)
 
-Induct_on `wl` THEN
-RW_TAC list_ss [revWord4ltoNum_def,numtoRevWord4l_def] THENL [
-	`word4$w2n h < 2**word4$WL` by METIS_TAC  [word4Theory.w2n_LT] THEN
-	FULL_SIMP_TAC arith_ss [MOD_MULT,word4Theory.WL_def,
-	                        word4Theory.HB_def]  THEN
-	`(revWord4ltoNum wl * 16+word4$w2n h) MOD 16 =word4$w2n h` 
-		by METIS_TAC [MOD_MULT] THEN
-	 FULL_SIMP_TAC arith_ss [word4Theory.w2n_ELIM], 
-	`(revWord4ltoNum wl * 16) MOD 16=0 ` 
-		by METIS_TAC [MOD_EQ_0,DECIDE ``0<16``] THEN
-	`word4$w2n h < 2**word4$WL` by METIS_TAC  [word4Theory.w2n_LT] THEN 
-	 FULL_SIMP_TAC arith_ss [ADD_DIV_RWT,LESS_DIV_EQ_ZERO,MULT_DIV,
-	                         word4Theory.WL_def,word4Theory.HB_def]]); 
-		 
-val revWord4ltoNum_conversion=Q.store_thm(
-"revWord4ltoNum_conversion",
-`!n len.
-	n < 2**(4*len)
-	==>
-	(revWord4ltoNum  (numtoRevWord4l len n) =n)`,	
+val revWord4ltoNumRange = Q.store_thm(
+ "revWord4ltoNumRange",
+ `!n l.
+    LENGTH l <= n ==> revWord4ltoNum l < 2 ** (4 * n)`,
+ Induct_on `l` THENL [
+   METIS_TAC [ revWord4ltoNum_def,ZERO_LESS_EXP,DECIDE ``2 = SUC 1``],
+   RW_TAC list_ss [revWord4ltoNum_def] THEN
+   Cases_on `n` THENL [
+     FULL_SIMP_TAC arith_ss [],
+     `4 * SUC n' = 4 + 4 * n'` by RW_TAC arith_ss [] THEN
+     `w2n h < 16` by WORD_DECIDE_TAC THEN
+     FULL_SIMP_TAC std_ss [EXP_ADD] THEN
+     FULL_SIMP_TAC list_ss [] THEN
+     `revWord4ltoNum l < 2 ** (4 * n') ` by METIS_TAC [] THEN
+     `SUC (revWord4ltoNum l) <= 2 ** (4 * n')` by METIS_TAC [LESS_EQ] THEN
+     `16+16* (revWord4ltoNum l)<= 16* 2 ** (4 * n')` by RW_TAC arith_ss [] THEN
+     FULL_SIMP_TAC arith_ss []]]);
 
-Induct_on `len` THEN
-RW_TAC list_ss [revWord4ltoNum_def,numtoRevWord4l_def] THEN
-`n DIV 16 <=2 ** (4 * SUC len) DIV 16` by RW_TAC arith_ss [DIV_LE_MONOTONE] THEN
-`n = n DIV 16 * 16 + n MOD 16` by METIS_TAC [DIVISION,DECIDE ``0<16``] THEN
-`2 ** (4 * SUC len) = 2**(4*len)*16` 
-	by FULL_SIMP_TAC std_ss [DECIDE ``4*SUC len=4*len +4``,EXP_ADD] THEN
-FULL_SIMP_TAC std_ss [MULT_DIV] THEN
-`n DIV 16 *16<= 2 ** (4 * len)*16` by RW_TAC arith_ss [] THEN
-Cases_on ` n DIV 16 = 2 ** (4 * len) ` THEN Cases_on `n MOD 16=0` THEN
-FULL_SIMP_TAC arith_ss [word4Theory.w2n_EVAL,word4Theory.MOD_WL_def,
-                        word4Theory.WL_def,word4Theory.HB_def]);
-		        
+val LENGTH_numtoRevWord4l = Q.store_thm(
+ "LENGTH_numtoRevWord4l",
+ `!wl n.
+    LENGTH (numtoRevWord4l n wl) = n`,
+ Induct_on `n` THEN
+ RW_TAC list_ss [numtoRevWord4l_def]);
 
-(*the conversions between a word128 and word4 list*)				 	
-val word4ltow128_def = Define
-`word4ltow128 w4l=word128$n2w (revWord4ltoNum (REVERSE w4l))`;
+(* the conversions between a num and word4 list are reversible *)
 
-val word128tow4l_def= Define
-`word128tow4l w128 = REVERSE (numtoRevWord4l 32 (word128$w2n w128))`;
+val numtoRevWord4l_conversion = Q.store_thm(
+ "numtoRevWord4l_conversion",
+ `!n wl.
+    (n = LENGTH wl)
+    ==>
+    (numtoRevWord4l n (revWord4ltoNum wl) = wl)`,
+ Induct_on `wl` THEN
+ RW_TAC list_ss [revWord4ltoNum_def,numtoRevWord4l_def] THEN
+ `w2n h < 16` by WORD_DECIDE_TAC THENL [
+    `(16 * revWord4ltoNum wl + w2n h) MOD 16 = w2n h`
+        by METIS_TAC [MOD_MULT, MULT_COMM] THEN
+    SRW_TAC [] [],
+    `(revWord4ltoNum wl * 16) MOD 16 = 0 `
+        by METIS_TAC [MOD_EQ_0,DECIDE ``0<16``] THEN
+     FULL_SIMP_TAC arith_ss [ADD_DIV_RWT,LESS_DIV_EQ_ZERO,
+       ONCE_REWRITE_RULE [MULT_COMM] MULT_DIV]]);
 
+val revWord4ltoNum_conversion = Q.store_thm(
+ "revWord4ltoNum_conversion",
+ `!n len.
+    n < 2 ** (4 * len)
+    ==>
+    (revWord4ltoNum  (numtoRevWord4l len n) = n)`,
+ Induct_on `len` THEN
+ RW_TAC list_ss [revWord4ltoNum_def,numtoRevWord4l_def] THEN
+ `n DIV 16 <= 2 ** (4 * SUC len) DIV 16`
+   by RW_TAC arith_ss [DIV_LE_MONOTONE] THEN
+ `n = n DIV 16 * 16 + n MOD 16` by METIS_TAC [DIVISION,DECIDE ``0<16``] THEN
+ `2 ** (4 * SUC len) = 2**(4* len)*16`
+   by FULL_SIMP_TAC std_ss [DECIDE ``4* SUC len = 4*len +4``,EXP_ADD] THEN
+ FULL_SIMP_TAC std_ss [MULT_DIV] THEN
+ `n DIV 16 * 16<= 2 ** (4 * len)*16` by RW_TAC arith_ss [] THEN
+ Cases_on ` n DIV 16 = 2 ** (4 * len) ` THEN
+  Cases_on `n MOD 16 = 0` THEN
+ FULL_SIMP_TAC (srw_ss()++ARITH_ss) []);
 
+(* the conversions between a word128 and word4 list*)
 
-val LENGTH_word128tow4l=Q.store_thm(
-"LENGTH_word128tow4l",
-`!w.
-	LENGTH (word128tow4l w) =32`,
+val word4ltow128_def = Define`
+ word4ltow128 w4l = n2w (revWord4ltoNum (REVERSE w4l)) : word128`;
 
-RW_TAC std_ss [word128tow4l_def,LENGTH_REVERSE,LENGTH_numtoRevWord4l]);
+val word128tow4l_def = Define`
+ word128tow4l (w:word128) = REVERSE (numtoRevWord4l 32 (w2n w))`;
 
-(*the conversions between a word128 and word4 list are reversible*)
-val word128tow4l_conversion=Q.store_thm(
-"word128tow4l_conversion",
-`!l. (LENGTH l =32) ==> (word128tow4l (word4ltow128 l) =l)`,
+val LENGTH_word128tow4l = Q.store_thm(
+ "LENGTH_word128tow4l",
+ `!w.  LENGTH (word128tow4l w) = 32`,
+ RW_TAC std_ss [word128tow4l_def,LENGTH_REVERSE,LENGTH_numtoRevWord4l]);
 
-RW_TAC arith_ss [word128tow4l_def,word4ltow128_def,word128Theory.w2n_EVAL,
-                 word128Theory.MOD_WL_def,word128Theory.WL_def,
-		 word128Theory.HB_def] THEN
-`LENGTH (REVERSE l) <=32` by RW_TAC list_ss [LENGTH_REVERSE] THEN
-`revWord4ltoNum (REVERSE l) < 2 ** (4*32)` by METIS_TAC [revWord4ltoNumRange] THEN
-FULL_SIMP_TAC arith_ss [LESS_MOD] THEN
-`LENGTH (REVERSE l) =32` by RW_TAC list_ss [LENGTH_REVERSE] THEN
-`numtoRevWord4l 32 (revWord4ltoNum (REVERSE l)) = REVERSE l` 
-	by METIS_TAC [numtoRevWord4l_conversion] THEN
-METIS_TAC [REVERSE_REVERSE]);
+(* the conversions between a word128 and word4 list are reversible*)
 
-val word4ltow128_conversion=Q.store_thm(
-"word4ltow128_conversion",
-`!w128.
-	word4ltow128 (word128tow4l w128) = w128`,
+val word128tow4l_conversion = Q.store_thm(
+ "word128tow4l_conversion",
+ `!l. (LENGTH l = 32) ==> (word128tow4l (word4ltow128 l) =l)`,
+ SRW_TAC [] [word128tow4l_def,word4ltow128_def] THEN
+ `LENGTH (REVERSE l) <= 32` by RW_TAC list_ss [LENGTH_REVERSE] THEN
+ `revWord4ltoNum (REVERSE l) < 2 ** (4* 32)`
+   by METIS_TAC [revWord4ltoNumRange] THEN
+ FULL_SIMP_TAC arith_ss [LESS_MOD] THEN
+ `LENGTH (REVERSE l) = 32` by RW_TAC list_ss [LENGTH_REVERSE] THEN
+ `numtoRevWord4l 32 (revWord4ltoNum (REVERSE l)) = REVERSE l`
+   by METIS_TAC [numtoRevWord4l_conversion] THEN
+ METIS_TAC [REVERSE_REVERSE]);
 
-RW_TAC arith_ss [word4ltow128_def,word128tow4l_def,REVERSE_REVERSE] THEN
-`word128$w2n w128 < 2 **word128$WL` by METIS_TAC [word128Theory.w2n_LT] THEN
-FULL_SIMP_TAC arith_ss [word128Theory.WL_def,word128Theory.HB_def,
-                        revWord4ltoNum_conversion,word128Theory.w2n_ELIM]);
-
-
-	 
+val word4ltow128_conversion = Q.store_thm(
+ "word4ltow128_conversion",
+ `!w.  word4ltow128 (word128tow4l w) = w`,
+ RW_TAC arith_ss [word4ltow128_def,word128tow4l_def,REVERSE_REVERSE] THEN
+ `w2n w < 2 ** 128` by WORD_DECIDE_TAC THEN
+ FULL_SIMP_TAC (srw_ss()) [revWord4ltoNum_conversion]);
 
 val word256to32lLength = Q.store_thm (
-"word256to32lLength",
-`!w. 
-	LENGTH (word256to32l w) =8`,
+ "word256to32lLength",
+ `!w.  LENGTH (word256to32l w) = 8`,
+ EVAL_TAC THEN METIS_TAC []);
 
-EVAL_TAC THEN METIS_TAC []);
+(* instantiate explicit list given the length *)
 
+val LENGTH_GREATER_EQ_CONS = Q.store_thm(
+ "LENGTH_GREATER_EQ_CONS",
+ `!l n.
+    (LENGTH l >= SUC n)
+    ==>
+    ?x l'. (LENGTH l' >= n) /\ (l = x::l')`,
+ Induct_on `l` THEN RW_TAC list_ss []);
 
-(*instantiate explicit list given the length
-*) 
+val listInstGreaterEq2 = Q.store_thm(
+ "listInstGreaterEq2",
+ `!l.
+    (LENGTH l >= 2)
+    ==>
+    ?v_1 v_2 t. l = (v_1::v_2::t)`,
+ REWRITE_TAC [REDEPTH_CONV numLib.num_CONV ``2``] THEN
+ METIS_TAC  [LENGTH_GREATER_EQ_CONS, LENGTH_NIL]);
 
-val LENGTH_GREATER_EQ_CONS=Q.store_thm(
-"LENGTH_GREATER_EQ_CONS",
-`!l n. 
-	(LENGTH l >=SUC n) 
-	==>
-	?x l'. (LENGTH l' >= n) /\ (l = x::l')`,
+val listInstEq2 = Q.store_thm(
+ "listInstEq2",
+ `!l.
+    (LENGTH l = 2)
+    ==>
+    ?w_1 w_2. l = (w_1::w_2::[])`,
+ METIS_TAC [LENGTH_CONS, LENGTH_NIL, REDEPTH_CONV numLib.num_CONV ``2``]);
 
-Induct_on `l` THEN
-RW_TAC list_ss []);
-	  
-val listInstGreaterEq2=Q.store_thm(
-"listInstGreaterEq2",
-`!l. 
-	(LENGTH l>=2) 
-	==> 
-	?v_1 v_2 t. l = (v_1::v_2::t)`,
-	     
-REWRITE_TAC [DECIDE ``2 = SUC (SUC 0)``] THEN
-METIS_TAC  [LENGTH_GREATER_EQ_CONS, LENGTH_NIL]);	  
+val listInstGreaterEq4 = Q.store_thm(
+ "listInstGreaterEq4",
+ `!l.
+    (LENGTH l >= 4)
+    ==>
+    ?v_1 v_2 v_3 v_4 t. l = (v_1::v_2::v_3::v_4::t)`,
+ REWRITE_TAC [REDEPTH_CONV numLib.num_CONV ``4``] THEN
+ METIS_TAC  [LENGTH_GREATER_EQ_CONS, LENGTH_NIL]);
 
-val listInstEq2=Q.store_thm(
-"listInstEq2",
-`!l. 
-	(LENGTH l=2) 
-	==> 
-	?w_1 w_2. l = (w_1::w_2::[])`,
-	
-REWRITE_TAC [LENGTH_CONS, LENGTH_NIL, DECIDE ``2 = SUC (SUC 0)``] THEN
-METIS_TAC []);
+val listInstEq4 = Q.store_thm(
+ "listInstEq4",
+ `!l.
+    (LENGTH l = 4)
+    ==>
+    ?w_1 w_2 w_3 w_4. l = (w_1::w_2::w_3::w_4::[])`,
+ REWRITE_TAC [LENGTH_CONS, LENGTH_NIL, REDEPTH_CONV numLib.num_CONV ``4``] THEN
+ METIS_TAC []);
 
+val listInstGreaterEq8 = Q.store_thm(
+ "listInstGreaterEq8",
+ `!l.
+    (LENGTH l >= 8)
+    ==>
+    ?v_1 v_2 v_3 v_4 v_5 v_6 v_7 v_8 t. l =
+    (v_1::v_2::v_3::v_4::v_5::v_6::v_7::v_8::t)`,
+ REWRITE_TAC [REDEPTH_CONV numLib.num_CONV ``8``] THEN
+ METIS_TAC  [LENGTH_GREATER_EQ_CONS, LENGTH_NIL]);
 
-val listInstGreaterEq4=Q.store_thm(
-"listInstGreaterEq4",
-`!l. 
-	(LENGTH l>=4) 
-	==> 
-	?v_1 v_2 v_3 v_4 t. l = (v_1::v_2::v_3::v_4::t)`,
-	
-REWRITE_TAC [DECIDE ``4 = SUC  (SUC  (SUC (SUC 0)))``] THEN
-METIS_TAC  [LENGTH_GREATER_EQ_CONS, LENGTH_NIL]);	  
+val listInstEq8 = Q.store_thm(
+ "listInstEq8",
+ `!l.
+    (LENGTH l = 8)
+    ==>
+    ?w_1 w_2 w_3 w_4 w_5 w_6 w_7 w_8. l =
+    (w_1::w_2::w_3::w_4::w_5::w_6::w_7::w_8::[])`,
+ REWRITE_TAC [LENGTH_CONS, LENGTH_NIL, REDEPTH_CONV numLib.num_CONV ``8``] THEN
+ METIS_TAC []);
 
-val listInstEq4=Q.store_thm(
-"listInstEq4",
-`!l. 
-	(LENGTH l=4) 
-	==> 
-	?w_1 w_2 w_3 w_4. l = (w_1::w_2::w_3::w_4::[])`,
-
-REWRITE_TAC [LENGTH_CONS, LENGTH_NIL, DECIDE ``4 = SUC (SUC (SUC (SUC 0)))``] THEN
-METIS_TAC []);
-     	  
-val listInstGreaterEq8=Q.store_thm(
-"listInstGreaterEq8",
-`!l. 
-	(LENGTH l>=8) 
-	==> 
-	?v_1 v_2 v_3 v_4 v_5 v_6 v_7 v_8 t. l =
-	(v_1::v_2::v_3::v_4::v_5::v_6::v_7::v_8::t)`,
-	     
-REWRITE_TAC [DECIDE ``8 = SUC (SUC (SUC (SUC (SUC (SUC (SUC (SUC 0)))))))``] THEN
-METIS_TAC  [LENGTH_GREATER_EQ_CONS, LENGTH_NIL]);	
-	        
-val listInstEq8=Q.store_thm(
-"listInstEq8",
-`!l. 
-	(LENGTH l=8) 
-	==> 
-	?w_1 w_2 w_3 w_4 w_5 w_6 w_7 w_8. l =
-	(w_1::w_2::w_3::w_4::w_5::w_6::w_7::w_8::[])`,
-
-REWRITE_TAC [LENGTH_CONS, LENGTH_NIL, DECIDE ``8 = SUC (SUC (SUC (SUC (SUC (SUC (SUC (SUC 0)))))))``] THEN
-METIS_TAC []);
-
-
-val listInstEq32 =Q.store_thm(
-"listInstEq32",
-` !l.
-	(LENGTH l = 32) ==>
+val listInstEq32 = Q.store_thm(
+ "listInstEq32",
+ ` !l.
+    (LENGTH l = 32) ==>
         ?v_0 v_1 v_2 v_3 v_4 v_5 v_6 v_7 v_8 v_9 v_10 v_11 v_12 v_13 v_14
          v_15 v_16 v_17 v_18 v_19 v_20 v_21 v_22 v_23 v_24 v_25 v_26 v_27
          v_28 v_29 v_30 v_31.
-        l =[v_0; v_1; v_2; v_3; v_4; v_5; v_6; v_7; v_8; v_9; v_10; v_11;
-           v_12; v_13; v_14; v_15; v_16; v_17; v_18; v_19; v_20; v_21; v_22;
-           v_23; v_24; v_25; v_26; v_27; v_28; v_29; v_30; v_31]`,
+        l = [v_0; v_1; v_2; v_3; v_4; v_5; v_6; v_7; v_8; v_9; v_10; v_11;
+             v_12; v_13; v_14; v_15; v_16; v_17; v_18; v_19; v_20; v_21; v_22;
+             v_23; v_24; v_25; v_26; v_27; v_28; v_29; v_30; v_31]`,
+ REWRITE_TAC [LENGTH_CONS, LENGTH_NIL, REDEPTH_CONV numLib.num_CONV ``32``] THEN
+ METIS_TAC []);
 
-REWRITE_TAC [LENGTH_CONS, LENGTH_NIL, 
-             DECIDE ``32 = SUC (SUC (SUC (SUC (SUC (SUC (SUC (SUC (SUC (SUC 
-	            (SUC (SUC (SUC (SUC (SUC (SUC (SUC (SUC (SUC (SUC (SUC 
-		    (SUC (SUC (SUC (SUC (SUC (SUC (SUC (SUC (SUC (SUC (SUC
-		     0))))))))))))))))))))))))))))))) ``] THEN
-METIS_TAC []); 
-
-val listInstEq33 =Q.store_thm(
-"listInstEq33", 
-` !l.
-	(LENGTH l = 33) ==>
+val listInstEq33 = Q.store_thm(
+ "listInstEq33",
+ `!l.
+    (LENGTH l = 33) ==>
         ?v_0 v_1 v_2 v_3 v_4 v_5 v_6 v_7 v_8 v_9 v_10 v_11 v_12 v_13 v_14
            v_15 v_16 v_17 v_18 v_19 v_20 v_21 v_22 v_23 v_24 v_25 v_26 v_27
            v_28 v_29 v_30 v_31 v_32.
-        l =[v_0; v_1; v_2; v_3; v_4; v_5; v_6; v_7; v_8; v_9; v_10; v_11;
-           v_12; v_13; v_14; v_15; v_16; v_17; v_18; v_19; v_20; v_21; v_22;
-           v_23; v_24; v_25; v_26; v_27; v_28; v_29; v_30; v_31; v_32]`,
-
-REWRITE_TAC [LENGTH_CONS, LENGTH_NIL, 
-             DECIDE ``33 = SUC (SUC (SUC (SUC (SUC (SUC (SUC (SUC (SUC (SUC
-	            (SUC (SUC (SUC (SUC (SUC (SUC (SUC (SUC (SUC (SUC (SUC 
-		    (SUC (SUC (SUC (SUC (SUC (SUC (SUC (SUC (SUC (SUC (SUC 
-		    (SUC 0)))))))))))))))))))))))))))))))) ``] THEN
-METIS_TAC []); 
-
+        l = [v_0; v_1; v_2; v_3; v_4; v_5; v_6; v_7; v_8; v_9; v_10; v_11;
+             v_12; v_13; v_14; v_15; v_16; v_17; v_18; v_19; v_20; v_21; v_22;
+             v_23; v_24; v_25; v_26; v_27; v_28; v_29; v_30; v_31; v_32]`,
+ REWRITE_TAC [LENGTH_CONS, LENGTH_NIL, REDEPTH_CONV numLib.num_CONV ``33``] THEN
+ METIS_TAC []);
 
 val _ = export_theory();
