examples/Crypto/IDEA/ideaScript.sml
@@ -1,13 +1,12 @@
 (* For interactive use
-app load ["word16Lib", "metisLib", "intLib","ideaMultTheory"];
+app load ["wordsLib", "intLib","ideaMultTheory"];
 quietdec := true;
-open word16Lib word16Theory metisLib pairTheory 
-     intLib integerTheory ideaMultTheory;
+open wordsLib wordsTheory pairTheory intLib integerTheory ideaMultTheory;
 quietdec := false;
 *)
 
 open HolKernel Parse boolLib bossLib
-     word16Lib word16Theory metisLib pairTheory 
+     wordsLib wordsTheory pairTheory
      intLib integerTheory ideaMultTheory;
 
 val RESTR_EVAL_TAC = computeLib.RESTR_EVAL_TAC;
@@ -30,11 +29,11 @@ val _ = type_abbrev("Block",    ``:word16 # word16 # word16 # word16``);
 val _ = type_abbrev("OddKey",   ``:word16 # word16 # word16 # word16``);
 val _ = type_abbrev("EvenKey",  ``:word16 # word16``);
 
-val _ = type_abbrev("InputKey", 
-        ``:word16 # word16 # word16 # word16 # 
+val _ = type_abbrev("InputKey",
+        ``:word16 # word16 # word16 # word16 #
            word16 # word16 # word16 # word16``);
 
-val _ = type_abbrev ("OddKeySched", 
+val _ = type_abbrev ("OddKeySched",
         ``:OddKey#OddKey#OddKey#OddKey#
            OddKey#OddKey#OddKey#OddKey#OddKey``);
 
@@ -50,92 +49,87 @@ val FORALL_BLOCK = Q.store_thm
  SIMP_TAC std_ss [FORALL_PROD]);
 
 val FORALL_ODDKEYSCHED = Q.prove
-(`(!x:OddKeySched. Q x) = !k1 k2 k3 k4 k5 k6 k7 k8 k9. 
+(`(!x:OddKeySched. Q x) = !k1 k2 k3 k4 k5 k6 k7 k8 k9.
                         Q(k1,k2,k3,k4,k5,k6,k7,k8,k9)`,
  EQ_TAC THEN RW_TAC std_ss [] THEN
- `?a1 a2 a3 a4 a5 a6 a7 a8 a9. 
+ `?a1 a2 a3 a4 a5 a6 a7 a8 a9.
      x = (a1,a2,a3,a4,a5,a6,a7,a8,a9)`
    by METIS_TAC [ABS_PAIR_THM]
  THEN ASM_REWRITE_TAC[]);
 
 val FORALL_EVENKEYSCHED = Q.prove
-(`(!x:EvenKeySched. Q x) = !k1 k2 k3 k4 k5 k6 k7 k8. 
+(`(!x:EvenKeySched. Q x) = !k1 k2 k3 k4 k5 k6 k7 k8.
                         Q(k1,k2,k3,k4,k5,k6,k7,k8)`,
  EQ_TAC THEN RW_TAC std_ss [] THEN
- `?a1 a2 a3 a4 a5 a6 a7 a8. 
+ `?a1 a2 a3 a4 a5 a6 a7 a8.
      x = (a1,a2,a3,a4,a5,a6,a7,a8)`
    by METIS_TAC [ABS_PAIR_THM]
  THEN ASM_REWRITE_TAC[]);
 
 val FORALL_EVENKEY = Q.prove
-(`(!x:EvenKey. Q x) = !kw1 kw2. 
+(`(!x:EvenKey. Q x) = !kw1 kw2.
                         Q(kw1,kw2)`,
  EQ_TAC THEN RW_TAC std_ss [] THEN
- `?a1 a2. 
+ `?a1 a2.
      x = (a1,a2)`
    by METIS_TAC [ABS_PAIR_THM]
  THEN ASM_REWRITE_TAC[]);
 
 val FORALL_ODDKEY = Q.prove
-(`(!x:OddKey. Q x) = !kw1 kw2 kw3 kw4. 
+(`(!x:OddKey. Q x) = !kw1 kw2 kw3 kw4.
                         Q(kw1,kw2,kw3,kw4)`,
  EQ_TAC THEN RW_TAC std_ss [] THEN
- `?a1 a2 a3 a4. 
+ `?a1 a2 a3 a4.
      x = (a1,a2,a3,a4)`
    by METIS_TAC [ABS_PAIR_THM]
  THEN ASM_REWRITE_TAC[]);
 
 val ZeroOddKey_def =  Define `ZeroOddKey = (0w,0w,0w,0w) : OddKey`;
 val ZeroEvenKey_def =  Define `ZeroEvenKey = (0w,0w) : EvenKey`;
-val ZeroOddKeys_def = 
- Define
-      `ZeroOddKeys = (ZeroOddKey,ZeroOddKey,ZeroOddKey,ZeroOddKey,ZeroOddKey,
-                      ZeroOddKey,ZeroOddKey,ZeroOddKey,ZeroOddKey) : OddKeySched`;
-val ZeroEvenKeys_def = 
- Define
-      `ZeroEvenKeys = (ZeroEvenKey,ZeroEvenKey,ZeroEvenKey,ZeroEvenKey,
-                       ZeroEvenKey,ZeroEvenKey,ZeroEvenKey,ZeroEvenKey) : EvenKeySched`;
+val ZeroOddKeys_def = Define
+  `ZeroOddKeys = (ZeroOddKey,ZeroOddKey,ZeroOddKey,ZeroOddKey,ZeroOddKey,
+                  ZeroOddKey,ZeroOddKey,ZeroOddKey,ZeroOddKey) : OddKeySched`;
+val ZeroEvenKeys_def = Define
+  `ZeroEvenKeys = (ZeroEvenKey,ZeroEvenKey,ZeroEvenKey,ZeroEvenKey,
+                   ZeroEvenKey,ZeroEvenKey,ZeroEvenKey,ZeroEvenKey) : EvenKeySched`;
 
 (*---Use Both Additive and Multiplicative Inverses Now---*)
-val InverseKey_def = 
- Define 
-   `InverseKey (k1,k2,k3,k4) = (winv k1, ~k3, ~k2, winv k4) : OddKey`;
+val InverseKey_def =
+ Define
+   `InverseKey (k1,k2,k3,k4) = (winv k1, $- k3, $- k2, winv k4) : OddKey`;
 
-val InverseKeys_def = 
+val InverseKeys_def =
  Define
    `InverseKeys (ok1,ok2,ok3,ok4,ok5,ok6,ok7,ok8,ok9) =
                 (InverseKey ok9,InverseKey ok8,InverseKey ok7,InverseKey ok6,
                  InverseKey ok5,InverseKey ok4,InverseKey ok3,InverseKey ok2,
                  InverseKey ok1) : OddKeySched`;
 
-val ReverseKeys_def = 
+val ReverseKeys_def =
  Define
    `ReverseKeys (ek1,ek2,ek3,ek4,ek5,ek6,ek7,ek8) =
                 (ek8,ek7,ek6,ek5,ek4,ek3,ek2,ek1) : EvenKeySched`;
 
-val RotateOddKeys_def = 
+val RotateOddKeys_def =
  Define
    `RotateOddKeys (k1,k2,k3,k4,k5,k6,k7,k8,k9) =
             (k2,k3,k4,k5,k6,k7,k8,k9,k1) : OddKeySched`;
 
-val RotateEvenKeys_def = 
+val RotateEvenKeys_def =
  Define
    `RotateEvenKeys (k1,k2,k3,k4,k5,k6,k7,k8) =
             (k2,k3,k4,k5,k6,k7,k8,k1) : EvenKeySched`;
 
 (*-1st and 4th are multiplications now-*)
-val OddRound_def = 
- Define 
+val OddRound_def =
+ Define
    `OddRound ((Ka, Kb, Kc, Kd):OddKey) ((Xa, Xb, Xc, Xd):Block) =
           (Xa wmul Ka, Xc + Kc, Xb + Kb,Xd wmul Kd) :Block`;
 
 val OddRound_Lemma1 = Q.store_thm
 ("OddRound_Lemma1",
- `!w1:word16 w2:word16. w1 + w2 + ~w2 = w1`,
- SIMP_TAC std_ss [WORD_ADD_COMM] THEN
- SIMP_TAC std_ss [WORD_ADD_ASSOC] THEN 
- ONCE_REWRITE_TAC [WORD_ADD_COMM] THEN
- SIMP_TAC std_ss [WORD_ADD_ASSOC, WORD_ADD_RINV, WORD_ADD]);
+ `!w1:word16 w2:word16. w1 + w2 + $- w2 = w1`,
+ SRW_TAC [] []);
 
 val OddRound_Inversion = Q.store_thm
 ("OddRound_Inversion",
@@ -144,48 +138,18 @@ val OddRound_Inversion = Q.store_thm
  ARW [InverseKey_def, OddRound_def] THEN
  ARW [wmul_ASSOC, wmul_Theorem, wmul_Mul1, OddRound_Lemma1]);
 
-val Mangler1_def = Define `Mangler1 ((Yin:word16), (Zin:word16), (Ke:word16), (Kf:word16)) = ((Ke * Yin) + Zin) * Kf`;
-val Mangler2_def = Define `Mangler2 ((Yin:word16), (Ke:word16), (Yout:word16)) = (Ke * Yin) + Yout`;
+val Mangler1_def = Define`
+ Mangler1 ((Yin:word16), (Zin:word16), (Ke:word16), (Kf:word16)) =
+   ((Ke * Yin) + Zin) * Kf`;
 
-val Mangler1_Lemma1 = Q.store_thm
-("Mangler1_Lemma1",
- `!w1 w2 w3 w4 w5 w6. w5 # Mangler1 (w1, w2, w3, w4) # (w6 # Mangler1 (w1, w2, w3, w4)) = w5 # w6`,
- SIMP_TAC std_ss [WORD_EOR_ASSOC] THEN 
- SIMP_TAC std_ss [WORD_EOR_COMM] THEN
- SIMP_TAC std_ss [WORD_EOR_ASSOC] THEN 
- ONCE_REWRITE_TAC [WORD_EOR_COMM] THEN
- SIMP_TAC std_ss [WORD_EOR_ASSOC, WORD_EOR_INV, WORD_EOR_ID]);
-
-val Mangler1_Lemma2 = Q.store_thm
-("Mangler1_Lemma2",
- `!w1 w2 w3 w4 w5. w5 # Mangler1 (w1, w2, w3, w4) # Mangler1 (w1, w2, w3, w4) = w5`,
- SIMP_TAC std_ss [WORD_EOR_COMM] THEN 
- SIMP_TAC std_ss [WORD_EOR_ASSOC] THEN
- ONCE_REWRITE_TAC [WORD_EOR_COMM] THEN
- SIMP_TAC std_ss [WORD_EOR_ASSOC, WORD_EOR_INV, WORD_EOR_ID]);
-
-val Mangler2_Lemma1 = Q.store_thm
-("Mangler2_Lemma1",
- `!w1 w2 w3 w4 w5. w4 # Mangler2 (w1, w2, w3) # (w5 # Mangler2 (w1, w2, w3)) = w4 # w5`,
- SIMP_TAC std_ss [WORD_EOR_ASSOC] THEN 
- SIMP_TAC std_ss [WORD_EOR_COMM] THEN
- SIMP_TAC std_ss [WORD_EOR_ASSOC] THEN 
- ONCE_REWRITE_TAC [WORD_EOR_COMM] THEN
- SIMP_TAC std_ss [WORD_EOR_ASSOC, WORD_EOR_INV, WORD_EOR_ID]);
-
-val Mangler2_Lemma2 = Q.store_thm
-("Mangler2_Lemma2",
- `!w1 w2 w3 w4. w4 # Mangler2 (w1, w2, w3) # Mangler2 (w1, w2, w3) = w4`,
- SIMP_TAC std_ss [WORD_EOR_COMM] THEN 
- SIMP_TAC std_ss [WORD_EOR_ASSOC] THEN
- ONCE_REWRITE_TAC [WORD_EOR_COMM] THEN
- SIMP_TAC std_ss [WORD_EOR_ASSOC, WORD_EOR_INV, WORD_EOR_ID]);
+val Mangler2_def = Define`
+  Mangler2 ((Yin:word16), (Ke:word16), (Yout:word16)) = (Ke * Yin) + Yout`;
 
 val EvenRound_def = Define
- `EvenRound ((Ke, Kf):EvenKey) ((Xa, Xb, Xc, Xd):Block) = 
-   let Yout =  Mangler1 ((Xa # Xb), (Xc # Xd), Ke, Kf) in
-     let Zout = Mangler2 ((Xa # Xb), Ke, Yout) in 
-       (Xa # Yout, Xb # Yout, Xc # Zout, Xd # Zout):Block`;
+ `EvenRound ((Ke, Kf):EvenKey) ((Xa, Xb, Xc, Xd):Block) =
+   let Yout =  Mangler1 ((Xa ?? Xb), (Xc ?? Xd), Ke, Kf) in
+     let Zout = Mangler2 ((Xa ?? Xb), Ke, Yout) in
+       (Xa ?? Yout, Xb ?? Yout, Xc ?? Zout, Xd ?? Zout):Block`;
 
 val [Mangler1] = decls "Mangler1";
 val [Mangler2] = decls "Mangler2";
@@ -193,26 +157,23 @@ val [Mangler2] = decls "Mangler2";
 val EvenRound_Inversion = Q.store_thm
 ("EvenRound_Inversion",
  `!s:Block k:EvenKey. EvenRound k (EvenRound k s) = s`,
- SIMP_TAC std_ss [FORALL_BLOCK, FORALL_EVENKEY] THEN
- RESTR_EVAL_TAC [Mangler1, Mangler2] THEN
- SIMP_TAC std_ss [Mangler1_Lemma1, Mangler1_Lemma2, Mangler2_Lemma1, Mangler2_Lemma2]);
+  SIMP_TAC std_ss [FORALL_BLOCK, FORALL_EVENKEY] THEN
+  RESTR_EVAL_TAC [Mangler1, Mangler2] THEN
+  SRW_TAC [] []);
 
-val (Round_def,Round_ind) = 
-  Defn.tprove 
-    (Hol_defn 
-      "Round"
-      `Round n (oddkeys: OddKeySched) (evenkeys: EvenKeySched) (state:Block) = 
+val Round_def =
+  tDefine "Round"
+    `Round n (oddkeys: OddKeySched) (evenkeys: EvenKeySched) (state:Block) =
       if (n = 0) then
         state
       else
         if (EVEN n) then
-          Round (n-1) oddkeys (RotateEvenKeys evenkeys) (EvenRound (FST evenkeys) state)
-        else 
-          Round (n-1) (RotateOddKeys oddkeys) evenkeys (OddRound (FST oddkeys) state)`,    
-   WF_REL_TAC `measure (FST)`
-   THEN CONJ_TAC
-   THEN REPEAT PairRules.PGEN_TAC
-   THEN SRW_TAC[ARITH_ss][]);
+          Round (n-1) oddkeys (RotateEvenKeys evenkeys)
+            (EvenRound (FST evenkeys) state)
+        else
+          Round (n-1) (RotateOddKeys oddkeys) evenkeys
+            (OddRound (FST oddkeys) state)`
+  (WF_REL_TAC `measure (FST)` THEN RW_TAC arith_ss [ELIM_UNCURRY]);
 
 val IdeaFwd_def = Define `IdeaFwd oddkeys evenkeys= Round 17 oddkeys evenkeys`;
 
@@ -221,62 +182,61 @@ val [EvenRound] = decls "EvenRound";
 
 val IDEA_LEMMA = Q.store_thm
 ("IDEA_LEMMA",
- `!plaintext:Block oddkeys:OddKeySched evenkeys:EvenKeySched. 
-     IdeaFwd (InverseKeys oddkeys) (ReverseKeys evenkeys) (IdeaFwd oddkeys evenkeys plaintext) = plaintext`,
- SIMP_TAC std_ss [FORALL_ODDKEYSCHED, FORALL_EVENKEYSCHED] THEN 
- RESTR_EVAL_TAC [OddRound, EvenRound] THEN 
+ `!plaintext:Block oddkeys:OddKeySched evenkeys:EvenKeySched.
+     IdeaFwd (InverseKeys oddkeys) (ReverseKeys evenkeys)
+       (IdeaFwd oddkeys evenkeys plaintext) = plaintext`,
+ SIMP_TAC std_ss [FORALL_ODDKEYSCHED, FORALL_EVENKEYSCHED] THEN
+ RESTR_EVAL_TAC [OddRound, EvenRound] THEN
  SIMP_TAC std_ss [OddRound_Inversion, EvenRound_Inversion]);
 
-val (MakeEnKeys_def,MakeEnKeys_ind) = 
-  Defn.tprove 
-    (Hol_defn 
-      "MakeEnKeys"
-      `MakeEnKeys n (K8::K7::K6::K5::K4::K3::K2::K1::rst) = 
-      let (NK1, NK2, NK3, NK4, NK5, NK6, NK7, NK8) = 
-        ((K2<<9) # (K3>>>7), (K3<<9) # (K4>>>7), 
-         (K4<<9) # (K5>>>7), (K5<<9) # (K6>>>7), 
-         (K6<<9) # (K7>>>7), (K7<<9) # (K8>>>7), 
-         (K8<<9) # (K1>>>7), (K1<<9) # (K2>>>7)) 
-      in 
+val MakeEnKeys_def =
+  tDefine "MakeEnKeys"
+   `MakeEnKeys n (K8::K7::K6::K5::K4::K3::K2::K1::rst) =
+      let (NK1, NK2, NK3, NK4, NK5, NK6, NK7, NK8) =
+        ((K2<<9) ?? (K3>>>7), (K3<<9) ?? (K4>>>7),
+         (K4<<9) ?? (K5>>>7), (K5<<9) ?? (K6>>>7),
+         (K6<<9) ?? (K7>>>7), (K7<<9) ?? (K8>>>7),
+         (K8<<9) ?? (K1>>>7), (K1<<9) ?? (K2>>>7))
+      in
         if n = 0 then
           (NK4::NK3::NK2::NK1::K8::K7::K6::K5::K4::K3::K2::K1::rst)
-        else 
+        else
           MakeEnKeys (n-1) (NK8::NK7::NK6::NK5::NK4::NK3::NK2::NK1
-                           ::K8::K7::K6::K5::K4::K3::K2::K1::rst)`,
-   WF_REL_TAC `measure (FST)`);
+                           ::K8::K7::K6::K5::K4::K3::K2::K1::rst)`
+   (WF_REL_TAC `measure (FST)`);
 
 val MakeKeys_def = Define
-   `MakeKeys ((K1, K2, K3, K4, K5, K6, K7, K8):InputKey)  = 
+   `MakeKeys ((K1, K2, K3, K4, K5, K6, K7, K8):InputKey)  =
       MakeEnKeys 6 [K8;K7;K6;K5;K4;K3;K2;K1]`;
 
-val ListToOddKeys_def = 
+val ListToOddKeys_def =
  Define
   `(ListToOddKeys [] oddkeys = oddkeys) /\
-   (ListToOddKeys ((k1::k2::k3::k4::k5::k6::t): word16 list) 
+   (ListToOddKeys ((k1::k2::k3::k4::k5::k6::t): word16 list)
         ((ok1,ok2,ok3,ok4,ok5,ok6,ok7,ok8,ok9): OddKeySched)  =
     ListToOddKeys t ((k1,k2,k3,k4),ok1,ok2,ok3,ok4,ok5,ok6,ok7,ok8))   /\
-   (ListToOddKeys ((k1::k2::k3::k4::t): word16 list) 
+   (ListToOddKeys ((k1::k2::k3::k4::t): word16 list)
                ((ok1,ok2,ok3,ok4,ok5,ok6,ok7,ok8,ok9): OddKeySched) =
     ListToOddKeys t ((k1,k2,k3,k4),ok1,ok2,ok3,ok4,ok5,ok6,ok7,ok8))`;
 
-val ListToEvenKeys_def = 
+val ListToEvenKeys_def =
  Define
   `(ListToEvenKeys [] evenkeys = evenkeys) /\
-   (ListToEvenKeys ((k1::k2::k3::k4::k5::k6::t): word16 list) 
+   (ListToEvenKeys ((k1::k2::k3::k4::k5::k6::t): word16 list)
             ((ek1,ek2,ek3,ek4,ek5,ek6,ek7,ek8): EvenKeySched) =
     ListToEvenKeys t ((k5,k6),ek1,ek2,ek3,ek4,ek5,ek6,ek7))`;
 
-val IDEA_def = Define `IDEA key = 
+val IDEA_def = Define `IDEA key =
   let oddkeys = ListToOddKeys (MakeKeys key) ZeroOddKeys in
-  let evenkeys = ListToEvenKeys (MakeKeys key) ZeroEvenKeys in 
-    (IdeaFwd oddkeys evenkeys, IdeaFwd (InverseKeys oddkeys) (ReverseKeys evenkeys))`;
-
+  let evenkeys = ListToEvenKeys (MakeKeys key) ZeroEvenKeys in
+    (IdeaFwd oddkeys evenkeys, IdeaFwd (InverseKeys oddkeys)
+    (ReverseKeys evenkeys))`;
 
 val IDEA_CORRECT = Q.store_thm
   ("IDEA_CORRECT",
-   `!key plaintext. 
-      ((encrypt,decrypt) = IDEA key) 
-      ==> 
+   `!key plaintext.
+      ((encrypt,decrypt) = IDEA key)
+      ==>
        (decrypt (encrypt plaintext) = plaintext)`,
  RW_TAC std_ss [IDEA_def,LET_THM,IDEA_LEMMA]);
 
