examples/Crypto/Serpent/Reference/Serpent_Reference_KeyScheduleScript.sml
@@ -1,44 +1,44 @@
-open HolKernel Parse boolLib bossLib listTheory rich_listTheory bitsTheory
-     markerTheory metisLib pairTheory arithmeticTheory 
-     word4Theory word32Theory word256Theory word4Lib word32Lib word256Lib 
+open HolKernel Parse boolLib bossLib listTheory rich_listTheory bitTheory
+     markerTheory pairTheory arithmeticTheory wordsTheory wordsLib
      Serpent_Reference_UtilityTheory Serpent_Reference_SBoxTheory
      Serpent_Reference_PermutationTheory;
 
 val _ = new_theory "Serpent_Reference_KeySchedule";
 
 (*32 rounds*)
-val R_def=Define `R=32`;
 
-val PHI_def=Define `PHI=(n2w:num->word32) 0x9e3779b9`;
+val R_def = Define `R = 32`;
+
+val PHI_def = Define `PHI = 0x9e3779b9w : word32`;
 
 (*padding*)
+
 val short2longKey_def =
   Define 
    `short2longKey k kl = 
       let nw256 = (n2w:num->word256) (k MOD  (2**kl)) 
       in
-        nw256 | (1w<<kl)`;
+        nw256 !! (1w << kl)`;
 
 (*used in making preKey*)
-val (makeSubKeyBitSlice_def,makeSubKeyBitSlice_termi)=Defn.tstore_defn(
+
+val (makeSubKeyBitSlice_def,makeSubKeyBitSlice_termi) = Defn.tstore_defn(
 Hol_defn "makeSubKeyBitSlice"
 `makeSubKeyBitSlice (w_1::w_2::w_3::w_4::w_5::w_6::w_7::w_8::t) i 
- = let nl =((w_1 # w_3 #  w_5 # w_8 #PHI# (n2w:num->word32) (131-i)) #>> 
+ = let nl =((w_1 ?? w_3 ??  w_5 ?? w_8 ?? PHI ?? (n2w:num->word32) (131-i)) #>> 
             (32-11)) 
-	   ::(w_1::w_2::w_3::w_4::w_5::w_6::w_7::w_8::t) 
+       ::(w_1::w_2::w_3::w_4::w_5::w_6::w_7::w_8::t) 
    in
-   if i=0 
+   if i = 0 
       then nl
       else makeSubKeyBitSlice nl (i-1)`,
-
-WF_REL_TAC `measure SND`);
-
+  WF_REL_TAC `measure SND`);
 
 (*reversed preKey*)
-val makeRevPreKey_def= Define
-`makeRevPreKey longKey=let keySlices = word256to32l longKey in
- myBUTLASTN 8 (makeSubKeyBitSlice keySlices 131)`;
 
+val makeRevPreKey_def = Define
+`makeRevPreKey longKey = let keySlices = word256to32l longKey in
+ myBUTLASTN 8 (makeSubKeyBitSlice keySlices 131)`;
 
 (*in reverse order
 
@@ -46,163 +46,143 @@ round  from 31 to 0
 
 bitPos from 31 to 0
 
-(k3,k2,k1,k0) =(0w,0w,0w,0w) when bitPos=31
+(k3,k2,k1,k0) =(0w,0w,0w,0w) when bitPos = 31
 
 efficient
 A version with mainly bit shifts, rotation and bitwise operation has been tried, 
 it is slow
 *)
+
 val makeRoundKey_def = Define
-`makeRoundKey (w3:word32,w2:word32,w1:word32,w0:word32) (k3:word32,k2:word32,k1:word32,k0:word32) bitPos round= 
-let bitofw0 = if word32$WORD_BIT bitPos w0 then 1
-		else 0
-in
-let bitofw1 = if word32$WORD_BIT bitPos w1 then 2
-		else 0
-in
-let bitofw2 = if word32$WORD_BIT bitPos w2 then 4 
-		else 0
-in
-let bitofw3 = if word32$WORD_BIT bitPos w3 then 8
-		else 0
-in
-let subed=S (((R+3-round) MOD R) MOD 8) ( bitofw3+ bitofw2+ bitofw1+ bitofw0)
-in
+`makeRoundKey (w3:word32,w2:word32,w1:word32,w0:word32)
+   (k3:word32,k2:word32,k1:word32,k0:word32) bitPos round = 
+  let bitofw0 = if w0 ' bitPos then 1 else 0 in
+  let bitofw1 = if w1 ' bitPos then 2 else 0 in
+  let bitofw2 = if w2 ' bitPos then 4 else 0 in
+  let bitofw3 = if w3 ' bitPos then 8 else 0 in
+  let subed = S (((R+3-round) MOD R) MOD 8)
+                (bitofw3 + bitofw2 + bitofw1 + bitofw0)
+  in
+  let subedbitofw0 = if subed ' 0 then 2 ** bitPos else 0 in
+  let subedbitofw1 = if subed ' 1 then 2 ** bitPos else 0 in
+  let subedbitofw2 = if subed ' 2 then 2 ** bitPos else 0 in
+  let subedbitofw3 = if subed ' 3 then 2 ** bitPos else 0 in
+  let bitofk0 = subedbitofw0 + w2n k0 in
+  let bitofk1 = subedbitofw1 + w2n k1 in
+  let bitofk2 = subedbitofw2 + w2n k2 in
+  let bitofk3 = subedbitofw3 + w2n k3 in
+    if bitPos = 0 then
+     (n2w (bitofk3 * 2 ** 96 +
+           bitofk2 * 2 ** 64 +
+           bitofk1 * 2 ** 32 +
+           bitofk0) : word128)
+    else
+      makeRoundKey (w3,w2,w1,w0) 
+        (n2w bitofk3, n2w bitofk2, n2w bitofk1, n2w bitofk0) (bitPos-1) round`;
 
-let subedbitofw0 = if word4$WORD_BIT 0 subed then 2**bitPos
-		else 0
-in
-let subedbitofw1 = if word4$WORD_BIT 1 subed then 2**bitPos 
-		else 0
-in
-let subedbitofw2 = if word4$WORD_BIT 2 subed then  2**bitPos 
-		else 0
-in
-let subedbitofw3 = if word4$WORD_BIT 3 subed then  2**bitPos
-		else 0
-in
-let bitofk0= subedbitofw0 + w2n k0 in
-let bitofk1= subedbitofw1 + w2n k1 in
-let bitofk2= subedbitofw2 + w2n k2 in
-let bitofk3= subedbitofw3 + w2n k3 in
+(* EL 0 is the 128bit key for first round MSBit(127)...LSBit(0) for each key
+   initialize round with 32 still in reversed order here *)
 
-if bitPos =0 then  word128$n2w (bitofk3 *2**96+ bitofk2*2**64 + bitofk1*2**32+bitofk0)
-else makeRoundKey (w3,w2,w1,w0) 
-( word32$n2w bitofk3, word32$n2w bitofk2,word32$n2w bitofk1, word32$n2w bitofk0) (bitPos-1) round`;
-
-
-
-
-(*EL 0 is the 128bit key for first round
-MSBit(127)...LSBit(0) for each key
-initialize round with 32 
-still in reversed order here
-*)
-val makeRevSubKey_def =Define
-`(makeRevSubKey [] round = [])          /\
-(makeRevSubKey (w3::w2::w1::w0::t) round = let roundKey = makeRoundKey (w3,w2,w1,w0) (0w,0w,0w,0w) 31 round in
-roundKey::(makeRevSubKey t (round-1))) `;
-
+val makeRevSubKey_def = Define
+`(makeRevSubKey [] round = []) /\
+ (makeRevSubKey (w3::w2::w1::w0::t) round =
+   let roundKey = makeRoundKey (w3,w2,w1,w0) (0w,0w,0w,0w) 31 round in
+     roundKey::(makeRevSubKey t (round-1)))`;
 
 (*this is the key used in the optimized version*)
-val makeSubKey_def =Define
-` makeSubKey revPreKey = REVERSE ( makeRevSubKey revPreKey 32)`;
+
+val makeSubKey_def = Define
+ `makeSubKey revPreKey = REVERSE ( makeRevSubKey revPreKey 32)`;
 
 (*this is the key used in the reference version*)
-val makeSubKeyHat_def=Define
-`makeSubKeyHat subKey=MAP IP subKey`;
 
+val makeSubKeyHat_def = Define
+ `makeSubKeyHat subKey = MAP IP subKey`;
 
 val makeKeyHat_def = Define
-`makeKeyHat userKey kl=let longKey =short2longKey userKey kl in
-let revPreKey=makeRevPreKey longKey in
-let subKey= makeSubKey revPreKey in
-makeSubKeyHat subKey`;
+`makeKeyHat userKey kl =
+  let longKey = short2longKey userKey kl in
+  let revPreKey = makeRevPreKey longKey in
+  let subKey = makeSubKey revPreKey in
+    makeSubKeyHat subKey`;
 
-val makeSubKeyBitSliceLength=Q.store_thm(
+val makeSubKeyBitSliceLength = Q.store_thm(
 "makeSubKeyBitSliceLength",
 `!longKey n. 
-	(LENGTH longKey>=8)
-	==> 
-	(LENGTH (makeSubKeyBitSlice longKey n )= n+LENGTH longKey+1)`,
+    (LENGTH longKey>= 8)
+    ==> 
+    (LENGTH (makeSubKeyBitSlice longKey n) = n + LENGTH longKey + 1)`,
+  Induct_on `n` THENL [
+    FULL_SIMP_TAC list_ss [makeSubKeyBitSlice_def,LENGTH,Abbrev_def] THEN
+    RW_TAC std_ss [] THEN
+    `?v_1 v_2 v_3 v_4 v_5 v_6 v_7 v_8 t. 
+        longKey = (v_1::v_2::v_3::v_4::v_5::v_6::v_7::v_8::t)` 
+        by METIS_TAC [listInstGreaterEq8] THEN
+    FULL_SIMP_TAC list_ss [makeSubKeyBitSlice_def] THEN
+    METIS_TAC [LENGTH,SUC_ONE_ADD,ADD_COMM],
+    RW_TAC std_ss [] THEN
+    `?v_1 v_2 v_3 v_4 v_5 v_6 v_7 v_8 t. 
+        longKey = (v_1::v_2::v_3::v_4::v_5::v_6::v_7::v_8::t)` 
+        by METIS_TAC [listInstGreaterEq8] THEN
+    FULL_SIMP_TAC list_ss [makeSubKeyBitSlice_def] THEN
+    RW_TAC list_ss [] THEN
+    FULL_SIMP_TAC list_ss [Abbrev_def]]);
 
-Induct_on `n` THENL [
-	FULL_SIMP_TAC list_ss [makeSubKeyBitSlice_def,LENGTH,Abbrev_def] THEN
-	RW_TAC std_ss [] THEN
-	`?v_1 v_2 v_3 v_4 v_5 v_6 v_7 v_8 t. 
-		longKey= (v_1::v_2::v_3::v_4::v_5::v_6::v_7::v_8::t)` 
-		by METIS_TAC [listInstGreaterEq8] THEN
-	FULL_SIMP_TAC list_ss [makeSubKeyBitSlice_def] THEN
-	METIS_TAC [LENGTH,SUC_ONE_ADD,ADD_COMM],
-	RW_TAC std_ss [] THEN
-	`?v_1 v_2 v_3 v_4 v_5 v_6 v_7 v_8 t. 
-		longKey = (v_1::v_2::v_3::v_4::v_5::v_6::v_7::v_8::t)` 
-		by METIS_TAC [listInstGreaterEq8] THEN
-	FULL_SIMP_TAC list_ss [makeSubKeyBitSlice_def] THEN
-	RW_TAC list_ss [] THEN
-	FULL_SIMP_TAC list_ss [Abbrev_def]]);
-
-val makeRevPreKeyLength=Q.store_thm(
+val makeRevPreKeyLength = Q.store_thm(
 "makeRevPreKeyLength",
 `!userKey. 
-	LENGTH (makeRevPreKey userKey)=132`,
+    LENGTH (makeRevPreKey userKey) = 132`,
+  RW_TAC std_ss [makeRevPreKey_def,LET_THM] THEN
+  `LENGTH (word256to32l userKey)= 8` by METIS_TAC [word256to32lLength] THEN
+  `LENGTH (word256to32l userKey)>= 8` by RW_TAC arith_ss [] THEN
+  `LENGTH (makeSubKeyBitSlice (word256to32l userKey) 131)
+   = 131+LENGTH (word256to32l userKey) +1` 
+      by METIS_TAC [makeSubKeyBitSliceLength,LENGTH_REVERSE] THEN
+  `8 <= LENGTH (makeSubKeyBitSlice (word256to32l userKey) 131)` 
+      by FULL_SIMP_TAC arith_ss [] THEN
+  FULL_SIMP_TAC list_ss [LENGTH_myBUTLASTN,LENGTH_REVERSE]);
 
-RW_TAC std_ss [makeRevPreKey_def,LET_THM] THEN
-`LENGTH (word256to32l userKey)=8` by METIS_TAC [word256to32lLength] THEN
-`LENGTH (word256to32l userKey)>=8` by RW_TAC arith_ss [] THEN
-`LENGTH (makeSubKeyBitSlice (word256to32l userKey) 131)
- =131+LENGTH (word256to32l userKey) +1` 
-	by METIS_TAC [makeSubKeyBitSliceLength,LENGTH_REVERSE] THEN
-`8 <= LENGTH (makeSubKeyBitSlice (word256to32l userKey) 131)` 
-	by FULL_SIMP_TAC arith_ss [] THEN
-FULL_SIMP_TAC list_ss [LENGTH_myBUTLASTN,LENGTH_REVERSE]);
-
-
-
-val makeRevSubKeyLength=Q.store_thm(
+val makeRevSubKeyLength = Q.store_thm(
 "makeRevSubKeyLength",
 `!n revPreKey. 
-	(LENGTH revPreKey= 4 * (n+1)) ==>(LENGTH (makeRevSubKey revPreKey n) =n+1)`,
+    (LENGTH revPreKey = 4 * (n+1)) ==>
+    (LENGTH (makeRevSubKey revPreKey n) = n + 1)`,
+  Induct_on `n` THENL [
+    RW_TAC arith_ss [] THEN
+    `?w_1 w_2 w_3 w_4. 
+        revPreKey = (w_1::w_2::w_3::w_4::[])` 
+        by METIS_TAC [listInstEq4] THEN
+    FULL_SIMP_TAC list_ss [makeRevSubKey_def] THEN
+    RW_TAC std_ss [] THEN
+    FULL_SIMP_TAC list_ss [LENGTH,Abbrev_def],
+    `4 * (SUC n + 1) = 4 +  4 * (n + 1)` by RW_TAC arith_ss [] THEN
+    `4 * (SUC n + 1) >= 4` by  RW_TAC arith_ss [] THEN
+    RW_TAC std_ss [] THEN
+    `?v_1 v_2 v_3 v_4 t. 
+        revPreKey = (v_1::v_2::v_3::v_4::t)` 
+        by METIS_TAC [listInstGreaterEq4] THEN
+    `LENGTH t = 4 * (n + 1)` by FULL_SIMP_TAC list_ss [LENGTH] THEN
+    FULL_SIMP_TAC list_ss [makeRevSubKey_def,LET_THM]]);
 
-Induct_on `n` THENL [
-	RW_TAC arith_ss [] THEN
-	`?w_1 w_2 w_3 w_4. 
-		revPreKey = (w_1::w_2::w_3::w_4::[])` 
-		by METIS_TAC [listInstEq4] THEN
-	FULL_SIMP_TAC list_ss [makeRevSubKey_def] THEN
-	RW_TAC std_ss [] THEN
-	FULL_SIMP_TAC list_ss [LENGTH,Abbrev_def],
-	`4 * (SUC n + 1) = 4 +  4 * (n + 1)` by RW_TAC arith_ss [] THEN
-	`4 * (SUC n + 1) >=4` by  RW_TAC arith_ss [] THEN
-	RW_TAC std_ss [] THEN
-	`?v_1 v_2 v_3 v_4 t. 
-		revPreKey = (v_1::v_2::v_3::v_4::t)` 
-		by METIS_TAC [listInstGreaterEq4] THEN
-	`LENGTH t = 4 * (n + 1)` by FULL_SIMP_TAC list_ss [LENGTH] THEN
-	FULL_SIMP_TAC list_ss [makeRevSubKey_def,LET_THM]]);
-
-val makeSubKeyLength=Q.store_thm(
+val makeSubKeyLength = Q.store_thm(
 "makeSubKeyLength",
 `!revPreKey.
-	(LENGTH revPreKey= 132) ==>(LENGTH (makeSubKey revPreKey) =33)`,
+    (LENGTH revPreKey = 132) ==> (LENGTH (makeSubKey revPreKey) = 33)`,
+ RW_TAC list_ss [makeSubKey_def,makeRevSubKeyLength,LENGTH_REVERSE]);
 
-RW_TAC list_ss [makeSubKey_def,makeRevSubKeyLength,LENGTH_REVERSE]);
+(* the only property of key shecduling which matters for the functional
+   correctness of Serpent is the length of the generated key *)        
 
-
-(*the only property of key shecduling 
-which matters for the functional correctness of Serpent
-is the length of the generated key*)	    
-val makeKeyHatLength=Q.store_thm(
+val makeKeyHatLength = Q.store_thm(
 "makeKeyHatLength",
 `!userKey kl. 
-	LENGTH (makeKeyHat userKey kl) =33`,
-
-RW_TAC std_ss [makeKeyHat_def,makeSubKeyHat_def] THEN
-RW_TAC std_ss [LENGTH_MAP] THEN
-FULL_SIMP_TAC std_ss [Abbrev_def] THEN
-`LENGTH  (makeRevPreKey (short2longKey userKey kl))=132` 
-	by METIS_TAC [makeRevPreKeyLength] THEN
-`132=4*(32+1)` by EVAL_TAC THEN
-FULL_SIMP_TAC arith_ss [makeSubKeyLength]);
+    LENGTH (makeKeyHat userKey kl) = 33`,
+  RW_TAC std_ss [makeKeyHat_def,makeSubKeyHat_def] THEN
+  RW_TAC std_ss [LENGTH_MAP] THEN
+  FULL_SIMP_TAC std_ss [Abbrev_def] THEN
+  `LENGTH  (makeRevPreKey (short2longKey userKey kl))= 132` 
+      by METIS_TAC [makeRevPreKeyLength] THEN
+  `132 = 4*(32+1)` by EVAL_TAC THEN
+  FULL_SIMP_TAC arith_ss [makeSubKeyLength]);
 
 val _ = export_theory();
